PREFIX : <http://resource.geosciml.org/classifierscheme/cgi/2016.01/classification-method-used>
PREFIX cs: <http://resource.geosciml.org/classifierscheme/cgi/2016.01/classification-method-used>
PREFIX dt: <http://resource.geosciml.org/datatype/>
PREFIX rdf: <http://www.w3.org/1999/02/22-rdf-syntax-ns#>
PREFIX rdfs: <http://www.w3.org/2000/01/rdf-schema#>
PREFIX schema: <https://schema.org/>
PREFIX skos: <http://www.w3.org/2004/02/skos/core#>
PREFIX xsd: <http://www.w3.org/2001/XMLSchema#>

cs: 
    a skos:ConceptScheme ;
    schema:keywords <https://gcmd.earthdata.nasa.gov/kms/concept/e9f67a66-e9fc-435c-b720-ae32a2c3d8f5> ;
    schema:dateCreated "2014-03-19"^^xsd:date ;
    schema:creator <https://linked.data.gov.au/org/cgi-gtwg> ;
    schema:dateModified "2025-06-04"^^xsd:date ;
    schema:citation "The EarthResourceML standard"@en ;
    schema:publisher <https://linked.data.gov.au/org/cgi> ;
    schema:citation "https://earthresourceml.org"^^xsd:anyURI ;
    skos:changeNote "2014 - Original SKOS implementation, based on 2013-06 approved vocabulary from GTWG face-to-face meeting in St. Petersburg, Russia. SKOS-RDF generated from Excel workbook using GSML_SKOS_from_XLS_2013.xslt."@en,
        "2016-07-15 OLR - Reformat SKOS to migrate to new vocabulary server. No changes to concepts."@en,
        "2020-06-23 NJC Added properties to ensure vocab matched Geoscience Australia's vocab profile (http://linked.data.gov.au/def/ga-skos-profile). Just annotation properties, no new content. Agents (creator/publisher) now not text but RDF resource. Dates (create/modified) derived from editorial notes & existing date properties."@en ,
        "2025-06-04 NJC Updates metadata to meet the VocPub 5.1 profile"@en ;
    skos:definition "This concept scheme describes methods of classification for quantitative reporting of mineral resources, as defined by the CGI Geoscience Terminology Working Group. By extension, it includes all concepts in this conceptScheme, as well as concepts in any previous versions of the scheme. Designed for use in the \"classificationMethodUsed\" property in EarthResourceML OreMeasure elements."@en ;
    skos:editorialNote "This file contains the 2016 SKOS-RDF version of the CGI Mineral Resource Reporting Classification Method vocabulary. Compilation in Excel spreadsheet, and converted to SKOS using GSML_SKOS_fromXLS_2016.02.xslt."@en ;
    skos:hasTopConcept 
        :cim-standards,
        :crirsco-code,
        :iimch-code,
        :imm-reporting-code,
        :jorc-code,
        :ni-43-101,
        :non-compliant-resource-estimate,
        :perc-code,
        :peruvian-code,
        :russian-code,
        :samrec-code,
        :sec-guide,
        :sme-guide,
        :unfc-code ;
    skos:prefLabel "Mineral Resource Reporting Classification Method"@en .


<http://resource.geosciml.org/classifier/cgi/classification-method-used> a skos:Collection ;
    schema:citation "The original vocabulary - all its concepts"@en ;
    rdfs:isDefinedBy cs: ;
    skos:changeNote "2021-12-17 R.Heaven BGS Added alignments to INSPIRE registry codelists using new alignments created automatically using Levenshtein similarity threshold of 0.75."@en ;
    skos:definition "All the Concepts in this vocabulary"@en ;
    skos:inScheme cs: ;
    skos:member 
        :cim-standards,
        :crirsco-code,
        :iimch-code,
        :imm-reporting-code,
        :jorc-code,
        :ni-43-101,
        :non-compliant-resource-estimate,
        :perc-code,
        :peruvian-code,
        :russian-code,
        :samrec-code,
        :sec-guide,
        :sme-guide,
        :unfc-code ;
    skos:prefLabel "Mineral Resource Reporting Classification Method - All Concepts"@en .


:cim-standards a skos:Concept ;
    schema:citation "http://www.cim.org/splash/index.cfm"^^xsd:anyURI ;
    rdfs:isDefinedBy cs: ;
    skos:definition "The CIM Definition Standards on Mineral Resources and Reserves (CIM Definition Standards) establish definitions and guidelines for the reporting of exploration information, mineral resources and mineral reserves in Canada"@en ;
    skos:exactMatch <http://inspire.ec.europa.eu/codelist/ClassificationMethodUsedValue/CIMstandards> ;
    skos:inScheme cs: ;
    skos:notation "03.."^^dt:LocalHierarchyKey ;
    skos:prefLabel "CIM standards"@en ;
    skos:topConceptOf cs: 
.


:crirsco-code a skos:Concept ;
    schema:citation "www.crirsco.com"@en ;
    rdfs:isDefinedBy cs: ;
    skos:definition "The International Reporting Template (IRT) is a document that draws on the best of the CRIRSCO-style reporting standards, the JORC Code (Australasia), SAMREC Code (South Africa), Reporting Code (UK / Western Europe), CIM Guidelines (Canada), SME Guide (USA) and Certification Code (Chile). These reporting standards are recognised and adopted world-wide for market-related reporting and financial investment"@en ;
    skos:exactMatch <http://inspire.ec.europa.eu/codelist/ClassificationMethodUsedValue/CRIRSCOCode> ;
    skos:inScheme cs: ;
    skos:notation "09.."^^dt:LocalHierarchyKey ;
    skos:prefLabel "CRIRSCO Code"@en ;
    skos:topConceptOf cs: 
.


:iimch-code a skos:Concept ;
    schema:citation "http://www.cim.org/standards/documents/Block470_Doc26.pdf"^^xsd:anyURI ;
    rdfs:isDefinedBy cs: ;
    skos:definition "Certification Code for Exploration Prospects, Mineral Resources & Ore Reserves. This Code is the result of a Collaboration Agreement between the Institution of Mining Engineers of Chile (IIMCh) and the Ministry of Mining."@en ;
    skos:exactMatch <http://inspire.ec.europa.eu/codelist/ClassificationMethodUsedValue/IIMChCode> ;
    skos:inScheme cs: ;
    skos:notation "07.."^^dt:LocalHierarchyKey ;
    skos:prefLabel "IIMCh Code"@en ;
    skos:topConceptOf cs: 
.


:imm-reporting-code a skos:Concept ;
    schema:citation "http://www.iom3.org/"^^xsd:anyURI ;
    rdfs:isDefinedBy cs: ;
    skos:definition "The Code for Reporting of Mineral Resources and Mineral Reserves (the 'Reporting Code' or ‘the Code’) sets out minimum standards, recommendations and guidelines for Public Reporting of Mineral Exploration Results, Mineral Resources and Mineral Reserves in the United Kingdom, Ireland and Europe."@en ;
    skos:exactMatch <http://inspire.ec.europa.eu/codelist/ClassificationMethodUsedValue/IMMReportingCode> ;
    skos:inScheme cs: ;
    skos:notation "05.."^^dt:LocalHierarchyKey ;
    skos:prefLabel "IMM Reporting Code"@en ;
    skos:topConceptOf cs: 
.


:jorc-code a skos:Concept ;
    schema:citation "http://www.jorc.org"^^xsd:anyURI ;
    rdfs:isDefinedBy cs: ;
    skos:definition "The Australasian Code for Reporting of Exploration Results, Mineral Resources and Ore Reserves (the ‘JORC Code’ or ‘the Code’)"@en ;
    skos:exactMatch <http://inspire.ec.europa.eu/codelist/ClassificationMethodUsedValue/JORCcode> ;
    skos:inScheme cs: ;
    skos:notation "01.."^^dt:LocalHierarchyKey ;
    skos:prefLabel "JORC code"@en ;
    skos:topConceptOf cs: 
.


:ni-43-101 a skos:Concept ;
    schema:citation "http://www.cim.org/splash/index.cfm"^^xsd:anyURI ;
    rdfs:isDefinedBy cs: ;
    skos:definition "National Instrument 43-101 (the \"NI 43-101\" or the \"NI\") is a mineral resource classification scheme used for the public disclosure of information relating to mineral properties in Canada. The NI is a strict guideline for how public companies can disclose scientific and technical information about mineral projects on bourses supervised by the Canadian Securities Administrators"@en ;
    skos:exactMatch <http://inspire.ec.europa.eu/codelist/ClassificationMethodUsedValue/NI43-101> ;
    skos:inScheme cs: ;
    skos:notation "02.."^^dt:LocalHierarchyKey ;
    skos:prefLabel "NI 43-101"@en ;
    skos:topConceptOf cs: 
.


:non-compliant-resource-estimate a skos:Concept ;
    schema:citation "CGI/ERML 2.0 and USGS proposal"@en ;
    rdfs:isDefinedBy cs: ;
    skos:definition "Resource estimate that does not meet the standards of \"standard codes\" (e.g. JORC etc.). Generally these estimates are 'Historic\" in that they pre-date the standards however in some cases they do not."@en ;
    skos:inScheme cs: ;
    skos:notation "14.."^^dt:LocalHierarchyKey ;
    skos:prefLabel "Non compliant resource estimate"@en ;
    skos:topConceptOf cs: 
.


:perc-code a skos:Concept ;
    schema:citation "http://www.vmine.net/percreserves/"^^xsd:anyURI ;
    rdfs:isDefinedBy cs: ;
    skos:definition "The Pan European Reserves and Resources Reporting Committee (PERC) Code for Reporting of Exploration Results, Mineral Resources and Mineral Reserves (further referred to as ‘the Code’) sets out minimum standards, recommendations and guidelines for Public Reporting of Exploration Results, Mineral Resources and Mineral Reserves in the United Kingdom, Ireland and Europe."@en ;
    skos:exactMatch <http://inspire.ec.europa.eu/codelist/ClassificationMethodUsedValue/PERCCode> ;
    skos:inScheme cs: ;
    skos:notation "12.."^^dt:LocalHierarchyKey ;
    skos:prefLabel "PERC Code"@en ;
    skos:topConceptOf cs: 
.


:peruvian-code a skos:Concept ;
    schema:citation "http://www.bvl.com.pe/scr/english/doc-reglamentos/Code%20for%20reporting%20of%20minerals.pdf"^^xsd:anyURI ;
    rdfs:isDefinedBy cs: ;
    skos:definition "The Code for Reporting on Mineral Resources and Ore Reserves has the purpose to set out the minimum standards, recommendations and guidelines to be complied with the presentation of Public Reports which are the basis from which to have access to the Venture Capital Segment of the Lima Stock Exchange. These reports will sustain the results on mineral exploration, of Mineral Resources and Ore Reserves. This Code was prepared by a Joint Committee formed by members of the Lima Stock Exchange and by professionals dedicated to the exploration and evaluation of mineral resources. This Code is based on and follows the example of the 1999 JORC CODE of Australasia which was prepared to ensure compliance with its guidelines in every Public Report on mineral explorations and evaluation results, as well as with similar codes and translations in use such as Canada (CIMVal 2001), United States of America (US Bureau of Mines, USGS Circular 831, Principles of Resource and Reserve Classification for Minerals), South Africa (The SAMREC Code), England (The UKIMM), and Australia (The AusIMM The Valmin Code)."@en ;
    skos:exactMatch <http://inspire.ec.europa.eu/codelist/ClassificationMethodUsedValue/peruvianCode> ;
    skos:inScheme cs: ;
    skos:notation "08.."^^dt:LocalHierarchyKey ;
    skos:prefLabel "Peruvian Code"@en ;
    skos:topConceptOf cs: 
.


:russian-code a skos:Concept ;
    schema:citation "http://www.imcinvest.com/pdf/Russian_reserves_8.pdf"^^xsd:anyURI ;
    rdfs:isDefinedBy cs: ;
    skos:altLabel "NAEN Code"@en ;
    skos:definition "Currently effective in Russia is the Code approved by the Decree of the Ministry of Natural Resources, RF № 278 of 11 December, 2006. Full title of the Document: Classification of resources/reserves and prognostic resources of solid minerals."@en ;
    skos:exactMatch <http://inspire.ec.europa.eu/codelist/ClassificationMethodUsedValue/russianCode> ;
    skos:inScheme cs: ;
    skos:notation "13.."^^dt:LocalHierarchyKey ;
    skos:prefLabel "Russian Code"@en ;
    skos:topConceptOf cs: 
.


:samrec-code a skos:Concept ;
    schema:citation "www.samcode.co.za"@en ;
    rdfs:isDefinedBy cs: ;
    skos:definition "The South African Code for Reporting of Exploration Results, Mineral Resources and Mineral Reserves."@en ;
    skos:exactMatch <http://inspire.ec.europa.eu/codelist/ClassificationMethodUsedValue/SAMRECcode> ;
    skos:inScheme cs: ;
    skos:notation "04.."^^dt:LocalHierarchyKey ;
    skos:prefLabel "SAMREC code"@en ;
    skos:topConceptOf cs: 
.


:sec-guide a skos:Concept ;
    schema:citation "www.cim.org/standards/"@en ;
    rdfs:isDefinedBy cs: ;
    skos:definition "Description of Property by Issuers Engaged or to be Engaged in Significant Mining Operations. Developed by the United States Securities and Exchange Commission, this Guide contains the Commission's basic mining disclosure policy. It includes definitions and disclosure instructions that apply to all public mining entities and their public disclosure."@en ;
    skos:exactMatch <http://inspire.ec.europa.eu/codelist/ClassificationMethodUsedValue/SECGuide> ;
    skos:inScheme cs: ;
    skos:notation "11.."^^dt:LocalHierarchyKey ;
    skos:prefLabel "SEC Guide"@en ;
    skos:topConceptOf cs: 
.


:sme-guide a skos:Concept ;
    schema:citation "www.smenet.org"@en ;
    rdfs:isDefinedBy cs: ;
    skos:definition "A guide for reporting exploration information, mineral resources, and mineral reserves - USA"@en ;
    skos:exactMatch <http://inspire.ec.europa.eu/codelist/ClassificationMethodUsedValue/SMEGuide> ;
    skos:inScheme cs: ;
    skos:notation "06.."^^dt:LocalHierarchyKey ;
    skos:prefLabel "SME Guide"@en ;
    skos:topConceptOf cs: 
.


:unfc-code a skos:Concept ;
    schema:citation "http://www.unece.org/energy/se/reserves.html"^^xsd:anyURI ;
    rdfs:isDefinedBy cs: ;
    skos:definition "The United Nations Framework Classification for Fossil Energy and Mineral Reserves and Resources 2009 (UNFC-2009) is a universally applicable scheme for classifying/evaluating energy and mineral reserves and resources - it is the successor to UNFC-2004. Designed as an all-encompassing framework, it enables the incorporation and unification of existing national systems, while allowing their classification units and glossary to be retained. The principal objective of UNFC-2009 is to enhance international communication by providing a simple, user-friendly and uniform format for the reporting of energy reserves and resources, using market-based economic criteria. It has been developed to meet, to the extent possible, the needs of applications pertaining to international energy and mineral studies, government resource management functions, corporate business processes and financial reporting standards"@en ;
    skos:exactMatch <http://inspire.ec.europa.eu/codelist/ClassificationMethodUsedValue/UNFCCode> ;
    skos:inScheme cs: ;
    skos:notation "10.."^^dt:LocalHierarchyKey ;
    skos:prefLabel "UNFC Code"@en ;
    skos:topConceptOf cs: 
.
