PREFIX : <http://resource.geosciml.org/classifier/cgi/mine-status/>
PREFIX astatus: <https://linked.data.gov.au/def/reg-statuses/>
PREFIX cs:<http://resource.geosciml.org/classifierscheme/cgi/2016.01/mine-status>
PREFIX dt: <http://resource.geosciml.org/datatype/>
PREFIX rdfs: <http://www.w3.org/2000/01/rdf-schema#>
PREFIX schema: <https://schema.org/>
PREFIX skos: <http://www.w3.org/2004/02/skos/core#>
PREFIX xsd: <http://www.w3.org/2001/XMLSchema#>

cs:
    a skos:ConceptScheme ;
    schema:keywords <https://gcmd.earthdata.nasa.gov/kms/concept/e9f67a66-e9fc-435c-b720-ae32a2c3d8f5> ;
    schema:dateCreated "2016-11-29"^^xsd:date ;
    schema:creator <https://linked.data.gov.au/org/cgi-gtwg> ;
    schema:dateModified "2025-06-04"^^xsd:date ;
    schema:citation "The EarthResourceML standard"@en ;
    schema:publisher <https://linked.data.gov.au/org/cgi> ;
    schema:citation "https://earthresourceml.org"^^xsd:anyURI ;
    schema:status astatus:stable ;
    skos:changeNote
        "2013-11-29 SMR Original conversion to SKOS."@en,
        "2015-01-08 OLR Edits to fix typos and remove '201403' from rdf file name."@en,
        "2016-11-29 OLR Regenerate SKOS-RDF file as part of migration to new vocabulary server. No change to previous concepts definitions."@en,
        "2020-06-23 NJC Added properties to ensure vocab matched Geoscience Australia's vocab profile (http://linked.data.gov.au/def/ga-skos-profile). Just annotation properties, no new content. Agents (creator/publisher) now not text but RDF resource. Dates (create/modified) derived from editorial notes & existing date properties."@en,
        "2021-12-17 R.Heaven BGS Added prefLabel and altLabel in non English languages, obtained from previously determined alignments between @en labels in CGI and Multi-lingual Thesaurus of Geosciences (MulTG) and Asian Multi-lingual Thesaurus of Geosciences (AMTG). Note that specific language packs are required to render the fonts.  Known issues: @lo and @fi labels were incorrectly encoded in the digitised source datasets; they have been included regardless of this in case the encoding can be corrected."@en ,
        "2025-06-04 NJC Updates metadata to meet the VocPub 5.1 profile"@en ;
    skos:definition "This file contains the CGI Mine Status vocabulary, as defined by the IUGS Commission for Geoscience Information (CGI) Geoscience Terminology Working Group. The vocabulary defines the operating status of a mine at a specified date, or if no date is specified, the current opertaing status. By extension, this vocabulary includes all concepts in this conceptScheme, as well as concepts in any previous versions of the scheme."@en ;
    skos:editorialNote "This file contains the 2016 SKOS-RDF version of the CGI Mine Status vocabulary. Compilation and review in Google doc spreadsheet; adopted 2013-06 in St. Petersburg, Russia; converted to MS Excel XML for SKOS generation using SKOS_for_GA_from_XLS_2016.03.xslt"@en ;
    skos:hasTopConcept :not-operating,
        :operating,
        :under-development ;
    skos:prefLabel "Mine Status"@en
.


<http://resource.geosciml.org/classifier/cgi/mine-status>
    a skos:Collection ;
    schema:citation "The original vocabulary - all its concepts"@en ;
    skos:changeNote
        "2021-12-17 R.Heaven BGS Added alignments to INSPIRE registry codelists using new alignments created automatically using Levenshtein similarity threshold of 0.75."@en ;
    skos:definition "All the Concepts in this vocabulary"@en ;
    skos:member
        :abandoned,
        :care-and-maintenance,
        :closed,
        :construction,
        :feasibility,
        :historic,
        :not-operating,
        :operating,
        :operating-continuously,
        :operating-intermittently,
        :pending-approval,
        :retention,
        :under-development ;
    skos:prefLabel "Mine Status - All Concepts"@en
.


:not-operating
    a skos:Concept ;
    schema:citation "this vocabulary"@en ;
    rdfs:isDefinedBy cs: ;
    skos:definition "A mine has been operating and then closed or suspended"@en ;
    skos:exactMatch <http://inspire.ec.europa.eu/codelist/MineStatusValue/notOperating> ;
    skos:inScheme cs: ;
    skos:narrower
        :abandoned,
        :care-and-maintenance,
        :closed,
        :historic,
        :retention ;
    skos:notation "02.."^^dt:LocalHierarchyKey ;
    skos:prefLabel "not operating"@en ;
    skos:topConceptOf cs:
.


:operating
    a skos:Concept ;
    schema:citation "this vocabulary"@en ;
    rdfs:isDefinedBy cs: ;
    skos:definition "A mine is operating"@en ;
    skos:exactMatch <http://inspire.ec.europa.eu/codelist/MineStatusValue/operating> ;
    skos:inScheme cs: ;
    skos:narrower
        :operating-continuously,
        :operating-intermittently ;
    skos:notation "01.."^^dt:LocalHierarchyKey ;
    skos:prefLabel "operating"@en ;
    skos:topConceptOf cs:
.


:under-development
    a skos:Concept ;
    schema:citation "this vocabulary"@en ;
    rdfs:isDefinedBy cs: ;
    skos:definition "A mine is under development - e.g feasibilty"@en ;
    skos:exactMatch <http://inspire.ec.europa.eu/codelist/MineStatusValue/underDevelopment> ;
    skos:inScheme cs: ;
    skos:narrower
        :construction,
        :feasibility,
        :pending-approval ;
    skos:notation "03.."^^dt:LocalHierarchyKey ;
    skos:prefLabel "under development"@en ;
    skos:topConceptOf cs:
.


:abandoned
    a skos:Concept ;
    schema:citation "this vocabulary"@en ;
    rdfs:isDefinedBy cs: ;
    skos:broader :not-operating ;
    skos:definition "A mine is abandoned - one reason or another"@en ;
    skos:exactMatch <http://inspire.ec.europa.eu/codelist/MineStatusValue/abandoned> ;
    skos:inScheme cs: ;
    skos:notation "02.2.."^^dt:LocalHierarchyKey ;
    skos:prefLabel "abandoned"@en
.


:care-and-maintenance
    a skos:Concept ;
    schema:citation "this vocabulary"@en ;
    rdfs:isDefinedBy cs: ;
    skos:broader :not-operating ;
    skos:definition "A mine is under care and maintenance"@en ;
    skos:exactMatch <http://inspire.ec.europa.eu/codelist/MineStatusValue/careAndMaintenance> ;
    skos:inScheme cs: ;
    skos:notation "02.3.."^^dt:LocalHierarchyKey ;
    skos:prefLabel "care and maintenance"@en
.


:closed
    a skos:Concept ;
    schema:citation "this vocabulary"@en ;
    rdfs:isDefinedBy cs: ;
    skos:broader :not-operating ;
    skos:definition "A mine can be closed for several reasons, e.g. technical, economical or technico-economical. For example, it may be re-opened if the price of the exploited commodity increases."@en ;
    skos:exactMatch <http://inspire.ec.europa.eu/codelist/MineStatusValue/closed> ;
    skos:inScheme cs: ;
    skos:notation "02.1.."^^dt:LocalHierarchyKey ;
    skos:prefLabel "closed"@en
.


:construction
    a skos:Concept ;
    schema:citation "this vocabulary"@en ;
    rdfs:isDefinedBy cs: ;
    skos:altLabel
        "bangunan"@id,
        "tafsiran"@id,
        "建造"@ja,
        "pembinaan"@ms,
        "构造"@zh,
        "结构"@zh ;
    skos:broader :under-development ;
    skos:definition "A mine is under construction after obtaining licenses/permits"@en ;
    skos:exactMatch <http://inspire.ec.europa.eu/codelist/MineStatusValue/construction> ;
    skos:inScheme cs: ;
    skos:notation "03.1.."^^dt:LocalHierarchyKey ;
    skos:prefLabel
        "Ingenieurbau"@de,
        "construction"@en,
        "obra"@es,
        "rakentaminen"@fi,
        "ouvrage"@fr,
        "konstruksi"@id,
        "opera ingegneristica"@it,
        "建築"@ja,
        "sMNg;"@km,
        "건설"@ko,
        "¡¾­¡Ò¦É¾¤"@lo,
        "binaan"@ms,
        "sooruzhenie"@ru,
        "konstruktion"@sv,
        "การก่อสร้าง"@th,
        "xây dựng"@vi,
        "建造"@zh
.


:feasibility
    a skos:Concept ;
    schema:citation "Dictionnaire thématique des mines et carrières, SIM Editor."@en ;
    rdfs:isDefinedBy cs: ;
    skos:broader :under-development ;
    skos:definition "Technical economic study aimed at assessing the possibility to launching a mine venture."@en ;
    skos:exactMatch <http://inspire.ec.europa.eu/codelist/MineStatusValue/feasibility> ;
    skos:inScheme cs: ;
    skos:notation "03.3.."^^dt:LocalHierarchyKey ;
    skos:prefLabel "feasibility"@en
.


:historic
    a skos:Concept ;
    schema:citation "this vocabulary"@en ;
    rdfs:isDefinedBy cs: ;
    skos:broader :not-operating ;
    skos:definition "An 'old' mine which has been exploited before 1900, e.g. during Roman times, the Middle Ages, etc."@en ;
    skos:exactMatch <http://inspire.ec.europa.eu/codelist/MineStatusValue/historic> ;
    skos:inScheme cs: ;
    skos:notation "02.5.."^^dt:LocalHierarchyKey ;
    skos:prefLabel "historic"@en
.


:operating-continuously
    a skos:Concept ;
    schema:citation "this vocabulary"@en ;
    rdfs:isDefinedBy cs: ;
    skos:broader :operating ;
    skos:definition "A mine is operating continuously"@en ;
    skos:exactMatch <http://inspire.ec.europa.eu/codelist/MineStatusValue/operatingContinuously> ;
    skos:inScheme cs: ;
    skos:notation "01.1.."^^dt:LocalHierarchyKey ;
    skos:prefLabel "operating continuously"@en
.


:operating-intermittently
    a skos:Concept ;
    schema:citation "this vocabulary"@en ;
    rdfs:isDefinedBy cs: ;
    skos:broader :operating ;
    skos:definition "A mine is operating intermittently"@en ;
    skos:exactMatch <http://inspire.ec.europa.eu/codelist/MineStatusValue/operatingIntermittently> ;
    skos:inScheme cs: ;
    skos:notation "01.2.."^^dt:LocalHierarchyKey ;
    skos:prefLabel "operating intermittently"@en
.


:pending-approval
    a skos:Concept ;
    schema:citation "this vocabulary"@en ;
    rdfs:isDefinedBy cs: ;
    skos:broader :under-development ;
    skos:definition "Waiting for the exploitation authorization, generally given by a State Mining Engineering Department."@en ;
    skos:exactMatch <http://inspire.ec.europa.eu/codelist/MineStatusValue/pendingApproval> ;
    skos:inScheme cs: ;
    skos:notation "03.2.."^^dt:LocalHierarchyKey ;
    skos:prefLabel "pending approval"@en
.


:retention
    a skos:Concept ;
    schema:citation "this vocabulary"@en ;
    rdfs:isDefinedBy cs: ;
    skos:altLabel
        "保留"@zh ;
    skos:broader :not-operating ;
    skos:definition "A mine can be kept unexploited until the price of contained commodity(ies) makes it economical."@en ;
    skos:exactMatch <http://inspire.ec.europa.eu/codelist/MineStatusValue/retention> ;
    skos:inScheme cs: ;
    skos:notation "02.4.."^^dt:LocalHierarchyKey ;
    skos:prefLabel "Zurückhaltung"@de,
        "retention"@en,
        "retención"@es,
        "vedenpidätyskyky"@fi,
        "rétention"@fr,
        "penambatan"@id,
        "ritenzione"@it,
        "保持"@ja,
        "karXat;"@km,
        "보유"@ko,
        "£¸¾´£ö¤êö­"@lo,
        "tambatan"@ms,
        "retentsiya"@ru,
        "retention"@sv,
        "การคงไว้"@th,
        "lượng nước giữ lại"@vi,
        "滞留"@zh
.

