PREFIX : <http://resource.geosciml.org/classifier/cgi/mineral-deposit-model/>
PREFIX astatus: <https://linked.data.gov.au/def/reg-statuses/>
PREFIX cs:<http://resource.geosciml.org/classifierscheme/cgi/2023.11/mineral-deposit-model>
PREFIX dt: <http://resource.geosciml.org/datatype/>
PREFIX owl: <http://www.w3.org/2002/07/owl#>
PREFIX rdfs: <http://www.w3.org/2000/01/rdf-schema#>
PREFIX schema: <https://schema.org/>
PREFIX skos: <http://www.w3.org/2004/02/skos/core#>
PREFIX xsd: <http://www.w3.org/2001/XMLSchema#>

:abyssal-pegmatite-ree
    a skos:Concept ;
    rdfs:isDefinedBy cs: ;
    skos:broader :pegmatite ;
    skos:definition "Pegmatites within the upper amphibolite to low to high pressure granulite facies, concentrated in rare-earth elements (REE)."@en ;
    skos:inScheme cs: ;
    skos:notation "12.01.04"^^dt:LocalHierarchyKey ;
    skos:prefLabel "Abyssal pegmatite REE"@en ;
    schema:additionalType :DepositType ;
.

:albitite-hosted-uranium
    a skos:Concept ;
    rdfs:isDefinedBy cs: ;
    skos:broader :alkali-calcic ;
    skos:definition "Not yet available"@en ;
    skos:inScheme cs: ;
    skos:notation "09.01.02"^^dt:LocalHierarchyKey ;
    skos:prefLabel "Albitite-hosted uranium"@en ;
    schema:additionalType :DepositType ;
.

:algoma-type-banded-iron-formation
    a skos:Concept ;
    rdfs:isDefinedBy cs: ;
    skos:broader :volcanogenic ;
    skos:definition "Chemically precipitated iron formation composed of thinly banded chert and iron minerals, with associated volcanic rocks and greywackes. It is found along volcanic arcs, chiefly Archaen  in age."@en ;
    skos:inScheme cs: ;
    skos:notation "10.02.01"^^dt:LocalHierarchyKey ;
    skos:prefLabel "Algoma-type banded iron formation"@en ;
    schema:additionalType :DepositType ;
.

:alkalic-epithermal-gold-ag
    a skos:Concept ;
    rdfs:isDefinedBy cs: ;
    skos:broader :epithermal ;
    skos:definition "Alkalic type epithermal deposits are part of a family of epithermal deposits and considered a subset of low-sulfidation epithermal gold deposits. Related to alkaline igneous rocks and occur as disseminated breccia and vein hosted gold and silver."@en ;
    skos:inScheme cs: ;
    skos:notation "11.01.03"^^dt:LocalHierarchyKey ;
    skos:prefLabel "Alkalic epithermal gold ± Ag"@en ;
    schema:additionalType :DepositType ;
.

:anorthosite-conduit-nickel-copper-pge
    a skos:Concept ;
    rdfs:isDefinedBy cs: ;
    skos:broader :anorthosite-conduit ;
    skos:definition "An anorthosite conduit associated nickel-copper-platinum-group elements (PGE) deposit."@en ;
    skos:inScheme cs: ;
    skos:notation "12.13.01"^^dt:LocalHierarchyKey ;
    skos:prefLabel "Anorthosite conduit nickel-copper-PGE"@en ;
    schema:additionalType :DepositType ;
.

:anorthosite-massif-titanium
    a skos:Concept ;
    rdfs:isDefinedBy cs: ;
    skos:broader :anorthosite-massif ;
    skos:definition "A massif-type anorthosite hosted titanium deposit."@en ;
    skos:inScheme cs: ;
    skos:notation "12.12.01"^^dt:LocalHierarchyKey ;
    skos:prefLabel "Anorthosite massif titanium"@en ;
    schema:additionalType :DepositType ;
.

:apatite-intrusion-ree
    a skos:Concept ;
    rdfs:isDefinedBy cs: ;
    skos:broader :apatite-intrusion ;
    skos:definition "Rare earth element mineralisation hosted by massive apatite veins. Veins and mineralisation form via magmatic-hydrothermal fluids exsolved from an alkali melt crystallising in the mid-crust."@en ;
    skos:inScheme cs: ;
    skos:notation "12.05.01"^^dt:LocalHierarchyKey ;
    skos:prefLabel "Apatite intrusion REE"@en ;
    schema:additionalType :DepositType ;
.

:apatite-nepheline-titanite-intrusion
    a skos:Concept ;
    rdfs:isDefinedBy cs: ;
    skos:broader :magmatic ;
    skos:definition "Apatite-nepheline-titanite mineralisation associated with an alkaline intrusive complex. Stockwork orebodies are hosted by nepheline syenite or foyaite."@en ;
    skos:inScheme cs: ;
    skos:notation "12.04."^^dt:LocalHierarchyKey ;
    skos:prefLabel "Apatite-nepheline-titanite intrusion"@en ;
    schema:additionalType :DepositGroup ;
.

:arc-u-m-intrusion-nickel-copper-pge
    a skos:Concept ;
    rdfs:isDefinedBy cs: ;
    skos:broader :ultramafic-and-or-mafic-intrusion ;
    skos:definition "Ultramafic to mafic arc-related intrusions with approximate concentric zoning and nickel-copper-platinum group element mineralisation. "@en ;
    skos:inScheme cs: ;
    skos:notation "12.09.04"^^dt:LocalHierarchyKey ;
    skos:prefLabel "Arc U-M intrusion nickel-copper-PGE"@en ;
    schema:additionalType :DepositType ;
.

:arc-u-m-intrusion-titanium-vanadium
    a skos:Concept ;
    rdfs:isDefinedBy cs: ;
    skos:broader :ultramafic-and-or-mafic-intrusion ;
    skos:definition "Ultramafic to mafic arc-related intrusions with approximate concentric zoning and titanium-vanadium mineralisation. "@en ;
    skos:inScheme cs: ;
    skos:notation "12.09.03"^^dt:LocalHierarchyKey ;
    skos:prefLabel "Arc U-M intrusion titanium-vanadium"@en ;
    schema:additionalType :DepositType ;
.

:bauxite
    a skos:Concept ;
    rdfs:isDefinedBy cs: ;
    skos:broader :laterite ;
    skos:definition "A sedimentary rock and the primary ore for aluminium, containing 15-25% aluminium. Bauxite is formed by the surface weathering of clay rocks in humid tropical to sub-tropical regions."@en ;
    skos:inScheme cs: ;
    skos:notation "02.01.01"^^dt:LocalHierarchyKey ;
    skos:prefLabel "Bauxite"@en ;
    schema:additionalType :DepositType ;
.

:bimodal-felsic-vms
    a skos:Concept ;
    rdfs:isDefinedBy cs: ;
    skos:broader :volcanogenic-massive-sulfide-vms ;
    skos:definition "Copper-zinc-lead-Au-Ag deposits formed at or near the seafloor at incipient-rifted continental margin arcs and related back-arc rifts where circulating hydrothermal fluids driven by magmatic heat are quenched through mixing with bottom waters or porewaters. Massive sulfide lenses form in a variety of shapes and sizes; they may be podlike or sheetlike and are generally stratiform. These deposits have an association with felsic and bimodal volcanic lithologies."@en ;
    skos:inScheme cs: ;
    skos:notation "10.01.04"^^dt:LocalHierarchyKey ;
    skos:prefLabel "Bimodal-felsic VMS"@en ;
    schema:additionalType :DepositType ;
.

:bimodal-mafic-vms
    a skos:Concept ;
    rdfs:isDefinedBy cs: ;
    skos:broader :volcanogenic-massive-sulfide-vms ;
    skos:definition "Copper-zinc-lead-Au-Ag deposits formed at or near the seafloor at intraoceanic volcanic arcs and related back-arc rifts where circulating hydrothermal fluids driven by magmatic heat are quenched through mixing with bottom waters or porewaters. Massive sulfide lenses form in a variety of shapes and sizes; they may be podlike or sheetlike and are generally stratiform. These deposits have an association with mafic and bimodal volcanic lithologies."@en ;
    skos:inScheme cs: ;
    skos:notation "10.01.03"^^dt:LocalHierarchyKey ;
    skos:prefLabel "Bimodal-mafic VMS"@en ;
    schema:additionalType :DepositType ;
.

:black-shale-gold
    a skos:Concept ;
    rdfs:isDefinedBy cs: ;
    skos:broader :black-shale ;
    skos:definition "A black shale hosted gold deposit."@en ;
    skos:inScheme cs: ;
    skos:notation "05.01.03"^^dt:LocalHierarchyKey ;
    skos:prefLabel "Black shale gold"@en ;
    schema:additionalType :DepositType ;
.

:black-shale-nickel-mo-pge
    a skos:Concept ;
    rdfs:isDefinedBy cs: ;
    skos:broader :black-shale ;
    skos:definition "Thin (<3-10 cm) layers of pyrite, vaesite, jordisite, and sphalerite in black shale sub-basins with associated phosphatic chert and carbonate rocks. These form in anoxic environments in continental platform or successor basin settings."@en ;
    skos:inScheme cs: ;
    skos:notation "05.01.02"^^dt:LocalHierarchyKey ;
    skos:prefLabel "Black shale nickel ± Mo-PGE"@en ;
    schema:additionalType :DepositType ;
.

:black-shale-uranium
    a skos:Concept ;
    rdfs:isDefinedBy cs: ;
    skos:broader :black-shale ;
    skos:definition "A black shale hosted uranium deposit. Uranium accumulations can be stratiform or stockwork, and are at low or very low grades forming an unconventional uranium resource."@en ;
    skos:inScheme cs: ;
    skos:notation "05.01.01"^^dt:LocalHierarchyKey ;
    skos:prefLabel "Black shale uranium"@en ;
    schema:additionalType :DepositType ;
.

:black-shale-vanadium-mo-ni
    a skos:Concept ;
    rdfs:isDefinedBy cs: ;
    skos:broader :black-shale ;
    skos:definition "A black shale hosted vanadium, molybdenum, nickel deposit."@en ;
    skos:inScheme cs: ;
    skos:notation "05.01.04"^^dt:LocalHierarchyKey ;
    skos:prefLabel "Black shale vanadium ± Mo ± Ni"@en ;
    schema:additionalType :DepositType ;
.

:breccia-pipe-copper
    a skos:Concept ;
    rdfs:isDefinedBy cs: ;
    skos:broader :breccia-pipe ;
    skos:definition "Not yet available"@en ;
    skos:inScheme cs: ;
    skos:notation "11.03.04"^^dt:LocalHierarchyKey ;
    skos:prefLabel "Breccia pipe copper"@en ;
    schema:additionalType :DepositType ;
.

:breccia-pipe-gold
    a skos:Concept ;
    rdfs:isDefinedBy cs: ;
    skos:broader :breccia-pipe ;
    skos:definition "Not yet available"@en ;
    skos:inScheme cs: ;
    skos:notation "11.03.01"^^dt:LocalHierarchyKey ;
    skos:prefLabel "Breccia pipe gold"@en ;
    schema:additionalType :DepositType ;
.

:breccia-pipe-molybdenum
    a skos:Concept ;
    rdfs:isDefinedBy cs: ;
    skos:broader :breccia-pipe ;
    skos:definition "Not yet available"@en ;
    skos:inScheme cs: ;
    skos:notation "11.03.02"^^dt:LocalHierarchyKey ;
    skos:prefLabel "Breccia pipe molybdenum"@en ;
    schema:additionalType :DepositType ;
.

:breccia-pipe-ree
    a skos:Concept ;
    rdfs:isDefinedBy cs: ;
    skos:broader :breccia-pipe ;
    skos:definition "Not yet available"@en ;
    skos:inScheme cs: ;
    skos:notation "11.03.03"^^dt:LocalHierarchyKey ;
    skos:prefLabel "Breccia pipe REE"@en ;
    schema:additionalType :DepositType ;
.

:calcrete-uranium
    a skos:Concept ;
    rdfs:isDefinedBy cs: ;
    skos:broader :uranium ;
    skos:definition "A calcrete-hosted uranium deposit, where ores are disseminations, vug linings, fracture coatings, and encrustations in calcrete cemented sediments or evaporative calcrete horizons."@en ;
    skos:inScheme cs: ;
    skos:notation "03.03.04"^^dt:LocalHierarchyKey ;
    skos:prefLabel "Calcrete uranium"@en ;
    schema:additionalType :DepositType ;
.

:carbonate-uranium
    a skos:Concept ;
    rdfs:isDefinedBy cs: ;
    skos:broader :uranium ;
    skos:definition "A uranium deposit occurring in calcareous host rocks. These deposits comprise syn- and epigenetic ores forming in a variety of geological settings."@en ;
    skos:inScheme cs: ;
    skos:notation "03.03.02"^^dt:LocalHierarchyKey ;
    skos:prefLabel "Carbonate uranium"@en ;
    schema:additionalType :DepositType ;
.

:carbonatite-laterite-ree
    a skos:Concept ;
    rdfs:isDefinedBy cs: ;
    skos:broader :laterite ;
    skos:definition "A REE deposit formed by the lateritic weathering of carbonatities. Carbonatite-hosted REE deposits are the primary source of the world's REEs."@en ;
    skos:inScheme cs: ;
    skos:notation "02.01.05"^^dt:LocalHierarchyKey ;
    skos:prefLabel "Carbonatite laterite REE"@en ;
    schema:additionalType :DepositType ;
.

:carbonatite-niobium
    a skos:Concept ;
    rdfs:isDefinedBy cs: ;
    skos:broader :carbonatite ;
    skos:definition "A carbonatite hosted niobium deposit."@en ;
    skos:inScheme cs: ;
    skos:notation "12.02.01"^^dt:LocalHierarchyKey ;
    skos:prefLabel "Carbonatite niobium"@en ;
    schema:additionalType :DepositType ;
.

:carbonatite-ree
    a skos:Concept ;
    rdfs:isDefinedBy cs: ;
    skos:broader :carbonatite ;
    skos:definition "A carbonatite hosted rare eath element (REE) deposit."@en ;
    skos:inScheme cs: ;
    skos:notation "12.02.02"^^dt:LocalHierarchyKey ;
    skos:prefLabel "Carbonatite REE"@en ;
    schema:additionalType :DepositType ;
.

:carlin-type-gold
    a skos:Concept ;
    rdfs:isDefinedBy cs: ;
    skos:broader :carlin-type ;
    skos:definition "Gold occuring as microscopic particles (up to 30 micrometeres) that must be identified by chemical analysis as it is not recoverable by panning."@en ;
    skos:inScheme cs: ;
    skos:notation "11.04.01"^^dt:LocalHierarchyKey ;
    skos:prefLabel "Carlin-type gold"@en ;
    schema:additionalType :DepositType ;
.

:climax-type-porphyry-molybdenum
    a skos:Concept ;
    rdfs:isDefinedBy cs: ;
    skos:broader :porphyry ;
    skos:definition "Not yet available"@en ;
    skos:inScheme cs: ;
    skos:notation "11.08.04"^^dt:LocalHierarchyKey ;
    skos:prefLabel "Climax-type porphyry molybdenum"@en ;
    schema:additionalType :DepositType ;
.

:coal-peat-bog-uranium
    a skos:Concept ;
    rdfs:isDefinedBy cs: ;
    skos:broader :uranium ;
    skos:definition "Uranium accumulations in coal or peat-bogs. Accumulations in coal form are likely sourced from uranium-rich rocks that sometimes overly or are intercalated with the coal seams. Uranium in peat-bogs are sourced from adjacent uranium-enriched regions."@en ;
    skos:inScheme cs: ;
    skos:notation "03.03.03"^^dt:LocalHierarchyKey ;
    skos:prefLabel "Coal/peat/bog uranium"@en ;
    schema:additionalType :DepositType ;
.

:collapse-breccia-pipe-uranium
    a skos:Concept ;
    rdfs:isDefinedBy cs: ;
    skos:broader :collapse-breccia-pipe ;
    skos:definition "Uranium mineralization centred on vertical collapse breccia pipes. The pipes develop in marine platform carbonates and act as a permeable conduit for upward artesian flow of basinal brines. Mixing of basinal brines with uranium-bearing oxidising waters from sandstone aquifers forms disseminated, replacement, and fracture fill uranium mineralisation."@en ;
    skos:inScheme cs: ;
    skos:notation "06.02.01"^^dt:LocalHierarchyKey ;
    skos:prefLabel "Collapse breccia pipe uranium"@en ;
    schema:additionalType :DepositType ;
.

:crust-manganese
    a skos:Concept ;
    rdfs:isDefinedBy cs: ;
    skos:broader :manganese ;
    skos:definition "Manganese crusts form by the precipitation of manganese and iron oxides from cold, ambient ocean water on sediment-free, hard substrates in the deep ocean. They typically form at water depths 400-7000 m."@en ;
    skos:inScheme cs: ;
    skos:notation "05.04.04"^^dt:LocalHierarchyKey ;
    skos:prefLabel "Crust manganese"@en ;
    schema:additionalType :DepositType ;
.

:distal-disseminated-silver-gold
    a skos:Concept ;
    rdfs:isDefinedBy cs: ;
    skos:broader :distal-disseminated ;
    skos:definition "Carlin-type style Ag-Au deposits formed on the distal edges of magmatic-hydrotthermal systems, related to upper crustal instrusive complexes."@en ;
    skos:inScheme cs: ;
    skos:notation "11.05.01"^^dt:LocalHierarchyKey ;
    skos:prefLabel "Distal-disseminated silver-gold"@en ;
    schema:additionalType :DepositType ;
.

:epithermal-beryllium
    a skos:Concept ;
    rdfs:isDefinedBy cs: ;
    skos:broader :epithermal ;
    skos:definition "Not yet available"@en ;
    skos:inScheme cs: ;
    skos:notation "11.01.05"^^dt:LocalHierarchyKey ;
    skos:prefLabel "Epithermal beryllium"@en ;
    schema:additionalType :DepositType ;
.

:epithermal-mercury
    a skos:Concept ;
    rdfs:isDefinedBy cs: ;
    skos:broader :epithermal ;
    skos:definition "Mercury (Hg) deposit assocaited with epithermal system."@en ;
    skos:inScheme cs: ;
    skos:notation "11.01.04"^^dt:LocalHierarchyKey ;
    skos:prefLabel "Epithermal mercury"@en ;
    schema:additionalType :DepositType ;
.

:epithermal-uranium
    a skos:Concept ;
    rdfs:isDefinedBy cs: ;
    skos:broader :epithermal ;
    skos:definition "Not yet available"@en ;
    skos:inScheme cs: ;
    skos:notation "11.01.06"^^dt:LocalHierarchyKey ;
    skos:prefLabel "Epithermal uranium"@en ;
    schema:additionalType :DepositType ;
.

:epizonal-orogenic-antimony-gold
    a skos:Concept ;
    rdfs:isDefinedBy cs: ;
    skos:broader :orogenic ;
    skos:definition "Antimony-bearing quartz veins hosted in deformed metamorphic terranes, formed in collisional orogenic belts at depths of less than 6 km and temperatures 150-300C."@en ;
    skos:inScheme cs: ;
    skos:notation "07.01.04"^^dt:LocalHierarchyKey ;
    skos:prefLabel "Epizonal orogenic antimony ± gold"@en ;
    schema:additionalType :DepositType ;
.

:epizonal-orogenic-gold
    a skos:Concept ;
    rdfs:isDefinedBy cs: ;
    skos:broader :orogenic ;
    skos:definition "Gold-bearing quartz veins hosted in deformed metamorphic terranes, formed in collisional orogenic belts at depths of less than 6 km and temperatures 150-300C."@en ;
    skos:inScheme cs: ;
    skos:notation "07.01.03"^^dt:LocalHierarchyKey ;
    skos:prefLabel "Epizonal orogenic gold"@en ;
    schema:additionalType :DepositType ;
.

:epizonal-orogenic-mercury
    a skos:Concept ;
    rdfs:isDefinedBy cs: ;
    skos:broader :orogenic ;
    skos:definition "Mercury deposits hosted in deformed metamorphic terranes, formed in collisional orogenic belts at depths of less than 6 km and temperatures 150-300C. Cinnabar and stibnite are the dominant ore minerals with native mercury also occuring."@en ;
    skos:inScheme cs: ;
    skos:notation "07.01.05"^^dt:LocalHierarchyKey ;
    skos:prefLabel "Epizonal orogenic mercury"@en ;
    schema:additionalType :DepositType ;
.

:exotic-copper
    a skos:Concept ;
    rdfs:isDefinedBy cs: ;
    skos:broader :exotic ;
    skos:definition "A copper deposit resulting from release by chemical weathering of soluble minerals and concentration by lateral chemical gradients and transport through paleodrainage systems."@en ;
    skos:inScheme cs: ;
    skos:notation "03.01.01"^^dt:LocalHierarchyKey ;
    skos:prefLabel "Exotic copper"@en ;
    schema:additionalType :DepositType ;
.

:felsic-siliciclastic-vms
    a skos:Concept ;
    rdfs:isDefinedBy cs: ;
    skos:broader :volcanogenic-massive-sulfide-vms ;
    skos:definition "Copper-zinc-lead-Au-Ag deposits formed at or near the seafloor at mature epicontinental margin arcs and related back-arc rifts where circulating hydrothermal fluids driven by magmatic heat are quenched through mixing with bottom waters or porewaters. Massive sulfide lenses form in a variety of shapes and sizes; they may be podlike or sheetlike and are generally stratiform. These deposits have an association with felsic and siliciclastic lithologies."@en ;
    skos:inScheme cs: ;
    skos:notation "10.01.05"^^dt:LocalHierarchyKey ;
    skos:prefLabel "Felsic-siliciclastic VMS"@en ;
    schema:additionalType :DepositType ;
.

:ferroan-carbonate-polymetallic
    a skos:Concept ;
    rdfs:isDefinedBy cs: ;
    skos:broader :metasomatic-iron ;
    skos:definition "Not yet available"@en ;
    skos:inScheme cs: ;
    skos:notation "09.02.01"^^dt:LocalHierarchyKey ;
    skos:prefLabel "Ferroan carbonate polymetallic"@en ;
    schema:additionalType :DepositType ;
.

:fluvial-placer-diamond
    a skos:Concept ;
    rdfs:isDefinedBy cs: ;
    skos:broader :placer ;
    skos:definition "A diamond deposit formed by modern fluvial systems transporting and concentrating diamonds."@en ;
    skos:inScheme cs: ;
    skos:notation "01.01.04"^^dt:LocalHierarchyKey ;
    skos:prefLabel "Fluvial placer diamond"@en ;
    schema:additionalType :DepositType ;
.

:fluvial-placer-garnet
    a skos:Concept ;
    rdfs:isDefinedBy cs: ;
    skos:broader :placer ;
    skos:definition "A garnet deposit formed by modern fluvial systems transporting and concentrating grains of garnet."@en ;
    skos:inScheme cs: ;
    skos:notation "01.01.08"^^dt:LocalHierarchyKey ;
    skos:prefLabel "Fluvial placer garnet"@en ;
    schema:additionalType :DepositType ;
.

:fluvial-placer-gemstones
    a skos:Concept ;
    rdfs:isDefinedBy cs: ;
    skos:broader :placer ;
    skos:definition "A gemstone deposit formed by modern fluvial systems transporting and concentrating gemstones."@en ;
    skos:inScheme cs: ;
    skos:notation "01.01.09"^^dt:LocalHierarchyKey ;
    skos:prefLabel "Fluvial placer gemstones"@en ;
    schema:additionalType :DepositType ;
.

:fluvial-placer-gold
    a skos:Concept ;
    rdfs:isDefinedBy cs: ;
    skos:broader :placer ;
    skos:definition "A gold deposit formed by modern fluvial systems transporting and concentrating gold."@en ;
    skos:inScheme cs: ;
    skos:notation "01.01.11"^^dt:LocalHierarchyKey ;
    skos:prefLabel "Fluvial placer gold"@en ;
    schema:additionalType :DepositType ;
.

:fluvial-placer-niobium-tantalum
    a skos:Concept ;
    rdfs:isDefinedBy cs: ;
    skos:broader :placer ;
    skos:definition "A niobium-tantalum deposit formed by modern fluvial systems transporting and concentrating niobium-tantalum bearing minerals."@en ;
    skos:inScheme cs: ;
    skos:notation "01.01.10"^^dt:LocalHierarchyKey ;
    skos:prefLabel "Fluvial placer niobium-tantalum"@en ;
    schema:additionalType :DepositType ;
.

:fluvial-placer-pge
    a skos:Concept ;
    rdfs:isDefinedBy cs: ;
    skos:broader :placer ;
    skos:definition "A PGE deposit formed by modern fluvial systems transporting and concentrating PGE bearing minerals."@en ;
    skos:inScheme cs: ;
    skos:notation "01.01.06"^^dt:LocalHierarchyKey ;
    skos:prefLabel "Fluvial placer PGE"@en ;
    schema:additionalType :DepositType ;
.

:fluvial-placer-ree
    a skos:Concept ;
    rdfs:isDefinedBy cs: ;
    skos:broader :placer ;
    skos:definition "A REE deposit formed by modern fluvial systems transporting and concentrating REE bearing minerals."@en ;
    skos:inScheme cs: ;
    skos:notation "01.01.05"^^dt:LocalHierarchyKey ;
    skos:prefLabel "Fluvial placer REE"@en ;
    schema:additionalType :DepositType ;
.

:fluvial-placer-tin
    a skos:Concept ;
    rdfs:isDefinedBy cs: ;
    skos:broader :placer ;
    skos:definition "A tin deposit formed by modern rivers and streams transporting and concentrating tin bearing minerals."@en ;
    skos:inScheme cs: ;
    skos:notation "01.01.07"^^dt:LocalHierarchyKey ;
    skos:prefLabel "Fluvial placer tin"@en ;
    schema:additionalType :DepositType ;
.

:fluvial-placer-tungsten
    a skos:Concept ;
    rdfs:isDefinedBy cs: ;
    skos:broader :placer ;
    skos:definition "A tungsten deposit formed by modern fluvial systems transporting and concentrating tungsten bearing minerals."@en ;
    skos:inScheme cs: ;
    skos:notation "01.01.03"^^dt:LocalHierarchyKey ;
    skos:prefLabel "Fluvial placer tungsten"@en ;
    schema:additionalType :DepositType ;
.

:greisen-beryllium-li
    a skos:Concept ;
    rdfs:isDefinedBy cs: ;
    skos:broader :greisen ;
    skos:definition "Not yet available"@en ;
    skos:inScheme cs: ;
    skos:notation "11.09.03"^^dt:LocalHierarchyKey ;
    skos:prefLabel "Greisen beryllium ± Li"@en ;
    schema:additionalType :DepositType ;
.

:greisen-tin-w-mo
    a skos:Concept ;
    rdfs:isDefinedBy cs: ;
    skos:broader :greisen ;
    skos:definition "Not yet available"@en ;
    skos:inScheme cs: ;
    skos:notation "11.09.01"^^dt:LocalHierarchyKey ;
    skos:prefLabel "Greisen tin ± W, Mo"@en ;
    schema:additionalType :DepositType ;
.

:greisen-tungsten-molybdenum-bi
    a skos:Concept ;
    rdfs:isDefinedBy cs: ;
    skos:broader :greisen ;
    skos:definition "Not yet available"@en ;
    skos:inScheme cs: ;
    skos:notation "11.09.02"^^dt:LocalHierarchyKey ;
    skos:prefLabel "Greisen tungsten-molybdenum ± Bi"@en ;
    schema:additionalType :DepositType ;
.

:heavy-mineral-sands
    a skos:Concept ;
    rdfs:isDefinedBy cs: ;
    skos:broader :placer ;
    skos:definition "Old beach, river, or dune sands that contain concentrations of heavy minerals such as rutile, ilmenite, zircon and monazite. Heavy minerals are concentrated by wave and wind action."@en ;
    skos:inScheme cs: ;
    skos:notation "01.01.16"^^dt:LocalHierarchyKey ;
    skos:prefLabel "Heavy mineral sands"@en ;
    schema:additionalType :DepositType ;
.

:hematite-dominant-ioa
    a skos:Concept ;
    rdfs:isDefinedBy cs: ;
    skos:broader :ioa ;
    skos:definition "Iron oxide-apatite (IOA) deposits in which the dominant iron oxide mineralisation is hematite."@en ;
    skos:inScheme cs: ;
    skos:notation "09.04.01"^^dt:LocalHierarchyKey ;
    skos:prefLabel "Hematite-dominant IOA"@en ;
    schema:additionalType :DepositType ;
.

:hematite-dominant-iocg
    a skos:Concept ;
    rdfs:isDefinedBy cs: ;
    skos:broader :iocg ;
    skos:definition "Iron oxide copper-gold (IOCG) deposits in which the dominant iron oxide mineralisation is hematite."@en ;
    skos:inScheme cs: ;
    skos:notation "09.03.02"^^dt:LocalHierarchyKey ;
    skos:prefLabel "Hematite-dominant IOCG"@en ;
    schema:additionalType :DepositType ;
.

:high-sulfidation-epithermal-silver-gold-cu
    a skos:Concept ;
    rdfs:isDefinedBy cs: ;
    skos:broader :epithermal ;
    skos:definition "Epithermal deposits characterised by the high sulphidation (HS) state of the sulfide mineral assemblage. The primary products of HS deposits are gold with variable amounts of silver and copper and are a major source of these elements."@en ;
    skos:inScheme cs: ;
    skos:notation "11.01.01"^^dt:LocalHierarchyKey ;
    skos:prefLabel "High-sulfidation (HS) epithermal silver-gold ± Cu"@en ;
    schema:additionalType :DepositType ;
.

:hypozonal-orogenic-gold
    a skos:Concept ;
    rdfs:isDefinedBy cs: ;
    skos:broader :orogenic ;
    skos:definition "Gold-bearing quartz veins hosted in deformed metamorphic terranes, formed in collisional orogenic belts at depths greater than 12 km and temperatures exceeding 475C."@en ;
    skos:inScheme cs: ;
    skos:notation "07.01.01"^^dt:LocalHierarchyKey ;
    skos:prefLabel "Hypozonal orogenic gold"@en ;
    schema:additionalType :DepositType ;
.

:impact-u-m-intrusion-nickel-copper-pge
    a skos:Concept ;
    rdfs:isDefinedBy cs: ;
    skos:broader :ultramafic-and-or-mafic-intrusion ;
    skos:definition "Nickel-copper-PGE mineralisation associated with an impact structure. Meteorite impact with ultramafic to mafic crustal rocks generates a superheated melt sheet, dissolving all sulfides in the target rocks. During cooling the sulfides crystallise early and accumulate along the base of the melt sheet."@en ;
    skos:inScheme cs: ;
    skos:notation "12.09.01"^^dt:LocalHierarchyKey ;
    skos:prefLabel "Impact U-M intrusion nickel-copper-PGE"@en ;
    schema:additionalType :DepositType ;
.

:intermediate-sulfidation-epithermal-silver-gold-zn-pb-cu-sn-mn
    a skos:Concept ;
    rdfs:isDefinedBy cs: ;
    skos:broader :epithermal ;
    skos:definition "Epithermal deposits characterised by the intermediate sulphidation (IS) state of the sulfide mineral assemblage. The primary products of HS deposits are silver, gold with variable amounts of zinc, lead copper, tin and manganese."@en ;
    skos:inScheme cs: ;
    skos:notation "11.01.07"^^dt:LocalHierarchyKey ;
    skos:prefLabel "Intermediate-sulfidation (IS) epithermal silver-gold ± Zn, Pb, Cu, Sn, Mn"@en ;
    schema:additionalType :DepositType ;
.

:ion-adsorption-ree
    a skos:Concept ;
    rdfs:isDefinedBy cs: ;
    skos:broader :clay-supergene ;
    skos:definition "A REE deposit formed by the adsorption of REE to the surface of the clay minerals kaolinite or halloysite through the weathering of igneous rocks (typically granites) in temperate and tropical climates."@en ;
    skos:inScheme cs: ;
    skos:notation "02.02.03"^^dt:LocalHierarchyKey ;
    skos:prefLabel "Ion adsorption REE"@en ;
    schema:additionalType :DepositType ;
.

:irish-type-sediment-hosted-zinc-lead
    a skos:Concept ;
    rdfs:isDefinedBy cs: ;
    skos:broader :sediment-hosted ;
    skos:definition "Stratabound, massive sphalerite, galena, iron sulfide, and barite lenses with associate calcite, dolomite, and quartz gangue in dolomitized platformal limestones. Deposits are structurally controlled and adjacent to normal growth faults."@en ;
    skos:inScheme cs: ;
    skos:notation "06.03.05"^^dt:LocalHierarchyKey ;
    skos:prefLabel "Irish-type sediment-hosted zinc-lead"@en ;
    schema:additionalType :DepositType ;
.

:iron-oxide-gold
    a skos:Concept ;
    rdfs:isDefinedBy cs: ;
    skos:broader :metasomatic-iron ;
    skos:definition "Not yet available"@en ;
    skos:inScheme cs: ;
    skos:notation "09.02.06"^^dt:LocalHierarchyKey ;
    skos:prefLabel "Iron oxide gold"@en ;
    schema:additionalType :DepositType ;
.

:iron-oxide-polymetallic
    a skos:Concept ;
    rdfs:isDefinedBy cs: ;
    skos:broader :metasomatic-iron ;
    skos:definition "Not yet available"@en ;
    skos:inScheme cs: ;
    skos:notation "09.02.04"^^dt:LocalHierarchyKey ;
    skos:prefLabel "Iron oxide polymetallic"@en ;
    schema:additionalType :DepositType ;
.

:iron-oxide-uranium
    a skos:Concept ;
    rdfs:isDefinedBy cs: ;
    skos:broader :metasomatic-iron ;
    skos:definition "Not yet available"@en ;
    skos:inScheme cs: ;
    skos:notation "09.02.05"^^dt:LocalHierarchyKey ;
    skos:prefLabel "Iron oxide uranium"@en ;
    schema:additionalType :DepositType ;
.

:iron-silicate-polymetallic
    a skos:Concept ;
    rdfs:isDefinedBy cs: ;
    skos:broader :metasomatic-iron ;
    skos:definition "Not yet available"@en ;
    skos:inScheme cs: ;
    skos:notation "09.02.03"^^dt:LocalHierarchyKey ;
    skos:prefLabel "Iron silicate polymetallic"@en ;
    schema:additionalType :DepositType ;
.

:iron-sulfide-polymetallic
    a skos:Concept ;
    rdfs:isDefinedBy cs: ;
    skos:broader :metasomatic-iron ;
    skos:definition "Not yet available"@en ;
    skos:inScheme cs: ;
    skos:notation "09.02.02"^^dt:LocalHierarchyKey ;
    skos:prefLabel "Iron sulfide polymetallic"@en ;
    schema:additionalType :DepositType ;
.

:karst-bauxite
    a skos:Concept ;
    rdfs:isDefinedBy cs: ;
    skos:broader :laterite ;
    skos:definition "A bauxite deposit formed by the surface weathering of clay rocks in karst landscapes."@en ;
    skos:inScheme cs: ;
    skos:notation "02.01.02"^^dt:LocalHierarchyKey ;
    skos:prefLabel "Karst bauxite"@en ;
    schema:additionalType :DepositType ;
.

:kimberlite-diamond
    a skos:Concept ;
    rdfs:isDefinedBy cs: ;
    skos:broader :kimberlite ;
    skos:definition "A kimberlite hosted diamond deposit. Kimberlites are the primary source of diamonds."@en ;
    skos:inScheme cs: ;
    skos:notation "12.06.01"^^dt:LocalHierarchyKey ;
    skos:prefLabel "Kimberlite diamond"@en ;
    schema:additionalType :DepositType ;
.

:kipushi-type-sediment-hosted-copper-zinc-lead
    a skos:Concept ;
    rdfs:isDefinedBy cs: ;
    skos:broader :sediment-hosted ;
    skos:definition "Massive base-metal sulfides and As-sulfosalts in dolomite breccias. Breccia zones are tabular or pipe-like and form in continental platform or shelf terranes with rifting. Breccias act as prosoud conduits for fluid flow, and ores are deposited in reducing environments."@en ;
    skos:inScheme cs: ;
    skos:notation "06.03.06"^^dt:LocalHierarchyKey ;
    skos:prefLabel "Kipushi-type sediment-hosted copper-zinc-lead"@en ;
    schema:additionalType :DepositType ;
.

:komatiite-nickel-copper-pge
    a skos:Concept ;
    rdfs:isDefinedBy cs: ;
    skos:broader :komatiite ;
    skos:definition "Nickel-copper-platinum group element mineralisation associated with komatiitic volcanic extrusive rocks. Sulfide bodies can be lenticular, irregular enlongate to tabular, or pipelike."@en ;
    skos:inScheme cs: ;
    skos:notation "12.07.01"^^dt:LocalHierarchyKey ;
    skos:prefLabel "Komatiite nickel-copper-PGE"@en ;
    schema:additionalType :DepositType ;
.

:lacustrine-brine-lithium
    a skos:Concept ;
    rdfs:isDefinedBy cs: ;
    skos:broader :brine ;
    skos:definition "Lithium-enriched brine pore-waters in suprasealevel saline lacustrine settings, typically in arid continental high altitude volcanogenic terrains."@en ;
    skos:inScheme cs: ;
    skos:notation "04.02.03"^^dt:LocalHierarchyKey ;
    skos:prefLabel "Lacustrine brine lithium"@en ;
    schema:additionalType :DepositType ;
.

:lacustrine-brine-potash
    a skos:Concept ;
    rdfs:isDefinedBy cs: ;
    skos:broader :brine ;
    skos:definition "Potash-enriched brine pore-waters in suprasealevel saline lacustrine settings. Derived from resurging deep basinal brines/formation waters."@en ;
    skos:inScheme cs: ;
    skos:notation "04.02.02"^^dt:LocalHierarchyKey ;
    skos:prefLabel "Lacustrine brine potash"@en ;
    schema:additionalType :DepositType ;
.

:lacustrine-clay-lithium
    a skos:Concept ;
    rdfs:isDefinedBy cs: ;
    skos:broader :clay-basin-evaporative ;
    skos:definition "Clay-hosted lithium deposit. Mineralized clays are derived from tuffaceous sediments during closed hydrologic system diagenesis, with a likely secondary magmatic source of lithium."@en ;
    skos:inScheme cs: ;
    skos:notation "04.04.01"^^dt:LocalHierarchyKey ;
    skos:prefLabel "Lacustrine clay lithium"@en ;
    schema:additionalType :DepositType ;
.

:lacustrine-evaporite-borate
    a skos:Concept ;
    rdfs:isDefinedBy cs: ;
    skos:broader :evaporite ;
    skos:definition "Borate deposit formed by the evaporation of saline water in lakes. Most deposits form in lakes in high-relief, active or formerly active volcanic terrains above sealevel in cooler arid conditions."@en ;
    skos:inScheme cs: ;
    skos:notation "04.01.09"^^dt:LocalHierarchyKey ;
    skos:prefLabel "Lacustrine evaporite borate"@en ;
    schema:additionalType :DepositType ;
.

:lacustrine-evaporite-carnallite-bischofite
    a skos:Concept ;
    rdfs:isDefinedBy cs: ;
    skos:broader :evaporite ;
    skos:definition "Carnallite-bischofite deposit formed by the evaporation of saline water in lakes."@en ;
    skos:inScheme cs: ;
    skos:notation "04.01.08"^^dt:LocalHierarchyKey ;
    skos:prefLabel "Lacustrine evaporite carnallite-bischofite"@en ;
    schema:additionalType :DepositType ;
.

:lacustrine-evaporite-magnesite
    a skos:Concept ;
    rdfs:isDefinedBy cs: ;
    skos:broader :evaporite ;
    skos:definition "Magnesite deposit formed by the evaporation of saline water in lakes."@en ;
    skos:inScheme cs: ;
    skos:notation "04.01.10"^^dt:LocalHierarchyKey ;
    skos:prefLabel "Lacustrine evaporite magnesite"@en ;
    schema:additionalType :DepositType ;
.

:lacustrine-evaporite-nitrate
    a skos:Concept ;
    rdfs:isDefinedBy cs: ;
    skos:broader :evaporite ;
    skos:definition "Nitrate salt deposit formed by the evaporation of saline water in lakes."@en ;
    skos:inScheme cs: ;
    skos:notation "04.01.11"^^dt:LocalHierarchyKey ;
    skos:prefLabel "Lacustrine evaporite nitrate"@en ;
    schema:additionalType :DepositType ;
.

:lacustrine-evaporite-potash
    a skos:Concept ;
    rdfs:isDefinedBy cs: ;
    skos:broader :evaporite ;
    skos:definition "Potash deposit formed by the evaporation of saline water in lakes."@en ;
    skos:inScheme cs: ;
    skos:notation "04.01.07"^^dt:LocalHierarchyKey ;
    skos:prefLabel "Lacustrine evaporite potash"@en ;
    schema:additionalType :DepositType ;
.

:lacustrine-evaporite-salt
    a skos:Concept ;
    rdfs:isDefinedBy cs: ;
    skos:broader :evaporite ;
    skos:definition "Salt deposit formed by the evaporation of saline water in lakes. Basin floor elevations are well above sea level when salts are accumulating."@en ;
    skos:inScheme cs: ;
    skos:notation "04.01.06"^^dt:LocalHierarchyKey ;
    skos:prefLabel "Lacustrine evaporite salt"@en ;
    schema:additionalType :DepositType ;
.

:lacustrine-evaporite-trona
    a skos:Concept ;
    rdfs:isDefinedBy cs: ;
    skos:broader :evaporite ;
    skos:definition "Trona (soda-ash) deposit formed by the evaporation of saline water in lakes. Trona is a sodium carbonate that forms from lake waters enriched in HCO3 compared to Mg and Ca."@en ;
    skos:inScheme cs: ;
    skos:notation "04.01.05"^^dt:LocalHierarchyKey ;
    skos:prefLabel "Lacustrine evaporite trona"@en ;
    schema:additionalType :DepositType ;
.

:lacustrine-iron-formation
    a skos:Concept ;
    rdfs:isDefinedBy cs: ;
    skos:broader :iron-formation ;
    skos:definition "Thin beds and laminations of fine-grained hematite formed by exhalation of hydrothermal fluids into caldera lakes. Subsequent volcanic processes may disturb the bedded hematite, forming breccias."@en ;
    skos:inScheme cs: ;
    skos:notation "05.03.03"^^dt:LocalHierarchyKey ;
    skos:prefLabel "Lacustrine iron formation"@en ;
    schema:additionalType :DepositType ;
.

:lacustrine-manganese
    a skos:Concept ;
    rdfs:isDefinedBy cs: ;
    skos:broader :manganese ;
    skos:definition "Bedded and vein manganese oxide in sedimentary and volcanic rocks filling half-graben basins associated with detachment faulting in extensional terranes."@en ;
    skos:inScheme cs: ;
    skos:notation "05.04.05"^^dt:LocalHierarchyKey ;
    skos:prefLabel "Lacustrine manganese"@en ;
    schema:additionalType :DepositType ;
.

:lacustrine-zeolite-li-b
    a skos:Concept ;
    rdfs:isDefinedBy cs: ;
    skos:broader :zeolite ;
    skos:definition "Microcrystalline zeolites crystallised in relatively thick, generally nonmarine tephra sequences. Zeolites crystallised in the post-depositional environment and show a more or less vertical zonation reflecting chemical modification by vertical movement of meteoric water."@en ;
    skos:inScheme cs: ;
    skos:notation "04.03.01"^^dt:LocalHierarchyKey ;
    skos:prefLabel "Lacustrine zeolite (± Li, B)"@en ;
    schema:additionalType :DepositType ;
.

:laterite-magnesite
    a skos:Concept ;
    rdfs:isDefinedBy cs: ;
    skos:broader :laterite ;
    skos:definition "A lateritic soil hosted magnesite deposit, formed by the weathering of ultramafic rocks in humid tropical to sub-tropical conditions."@en ;
    skos:inScheme cs: ;
    skos:notation "02.01.04"^^dt:LocalHierarchyKey ;
    skos:prefLabel "Laterite magnesite"@en ;
    schema:additionalType :DepositType ;
.

:laterite-nickel
    a skos:Concept ;
    rdfs:isDefinedBy cs: ;
    skos:broader :laterite ;
    skos:definition "A lateritic soil hosted nickel deposit, formed by the weathering of ultramafic rocks in humid tropical to sub-tropical conditions."@en ;
    skos:inScheme cs: ;
    skos:notation "02.01.03"^^dt:LocalHierarchyKey ;
    skos:prefLabel "Laterite nickel"@en ;
    schema:additionalType :DepositType ;
.

:lct-pegmatite
    a skos:Concept ;
    rdfs:isDefinedBy cs: ;
    skos:broader :pegmatite ;
    skos:definition "Pegmatites enriched in lithium, cesium and tantalum."@en ;
    skos:inScheme cs: ;
    skos:notation "12.01.03"^^dt:LocalHierarchyKey ;
    skos:prefLabel "LCT pegmatite"@en ;
    schema:additionalType :DepositType ;
.

:low-fluorine-porphyry-molybdenum
    a skos:Concept ;
    rdfs:isDefinedBy cs: ;
    skos:broader :porphyry ;
    skos:definition "Not yet available"@en ;
    skos:inScheme cs: ;
    skos:notation "11.08.05"^^dt:LocalHierarchyKey ;
    skos:prefLabel "Low-fluorine porphyry molybdenum"@en ;
    schema:additionalType :DepositType ;
.

:low-iron-alkali-calcic
    a skos:Concept ;
    rdfs:isDefinedBy cs: ;
    skos:broader :alkali-calcic ;
    skos:definition "Not yet available"@en ;
    skos:inScheme cs: ;
    skos:notation "09.01.01"^^dt:LocalHierarchyKey ;
    skos:prefLabel "Low iron alkali-calcic"@en ;
    schema:additionalType :DepositType ;
.

:low-sulfidation-epithermal-gold-silver
    a skos:Concept ;
    rdfs:isDefinedBy cs: ;
    skos:broader :epithermal ;
    skos:definition "Epithermal deposits characterised by the low sulphidation (LS) state of the sulfide mineral assemblage. The primary products of HS deposits are gold and silver."@en ;
    skos:inScheme cs: ;
    skos:notation "11.01.02"^^dt:LocalHierarchyKey ;
    skos:prefLabel "Low-sulfidation (LS) epithermal gold-silver"@en ;
    schema:additionalType :DepositType ;
.

:mafic-siliciclastic-vms
    a skos:Concept ;
    rdfs:isDefinedBy cs: ;
    skos:broader :volcanogenic-massive-sulfide-vms ;
    skos:definition "Copper-zinc-lead-Au-Ag deposits formed at or near the seafloor at sediment-covered ridges and related rifts where circulating hydrothermal fluids driven by magmatic heat are quenched through mixing with bottom waters or porewaters. Massive sulfide lenses form in a variety of shapes and sizes; they may be podlike or sheetlike and are generally stratiform. These deposits have an association with mafic and siliciclastic lithologies."@en ;
    skos:inScheme cs: ;
    skos:notation "10.01.02"^^dt:LocalHierarchyKey ;
    skos:prefLabel "Mafic-siliciclastic VMS"@en ;
    schema:additionalType :DepositType ;
.

:mafic-ultramafic-vms
    a skos:Concept ;
    rdfs:isDefinedBy cs: ;
    skos:broader :volcanogenic-massive-sulfide-vms ;
    skos:definition "Copper-zinc-lead-Au-Ag deposits formed at or near the seafloor at mid-ocean ridges or in mature back-arc basins where circulating hydrothermal fluids driven by magmatic heat are quenched through mixing with bottom waters or porewaters. Massive sulfide lenses form in a variety of shapes and sizes; they may be podlike or sheetlike and are generally stratiform. These deposits have an association with mafic and ultramafic lithologies."@en ;
    skos:inScheme cs: ;
    skos:notation "10.01.01"^^dt:LocalHierarchyKey ;
    skos:prefLabel "Mafic-ultramafic VMS"@en ;
    schema:additionalType :DepositType ;
.

:magnetite-dominant-ioa
    a skos:Concept ;
    rdfs:isDefinedBy cs: ;
    skos:broader :ioa ;
    skos:definition "Iron oxide-apatite (IOA) deposits in which the dominant iron oxide mineralisation is magnetite."@en ;
    skos:inScheme cs: ;
    skos:notation "09.04.02"^^dt:LocalHierarchyKey ;
    skos:prefLabel "Magnetite-dominant IOA"@en ;
    schema:additionalType :DepositType ;
.

:magnetite-dominant-iocg
    a skos:Concept ;
    rdfs:isDefinedBy cs: ;
    skos:broader :iocg ;
    skos:definition "Iron oxide copper-gold (IOCG) deposits in which the dominant iron oxide mineralisation is magnetite."@en ;
    skos:inScheme cs: ;
    skos:notation "09.03.01"^^dt:LocalHierarchyKey ;
    skos:prefLabel "Magnetite-dominant IOCG"@en ;
    schema:additionalType :DepositType ;
.

:marine-brine-potash-mg-li-and-so-on
    a skos:Concept ;
    rdfs:isDefinedBy cs: ;
    skos:broader :brine ;
    skos:definition "A marine brine, concentrated in potash and or magnesium and lithium salts. Derived from hydrothermally-modified marine water; today this occurs in and near active fracture zones where seawater interacts with oceanic crust at mid-ocean ridges."@en ;
    skos:inScheme cs: ;
    skos:notation "04.02.01"^^dt:LocalHierarchyKey ;
    skos:prefLabel "Marine brine potash (± Mg, Li, and so on)"@en ;
    schema:additionalType :DepositType ;
.

:marine-evaporite-gypsum
    a skos:Concept ;
    rdfs:isDefinedBy cs: ;
    skos:broader :evaporite ;
    skos:definition "Gypsum deposit formed by the evaporation of seawater. Gypsum has been one of the most volumetrically significant marine evaporite salts since the Phanerozoic; prior to the Mesoproterozoic, free sulfate levels in the ocean were insufficent to allow gypsum precipitation."@en ;
    skos:inScheme cs: ;
    skos:notation "04.01.01"^^dt:LocalHierarchyKey ;
    skos:prefLabel "Marine evaporite gypsum"@en ;
    schema:additionalType :DepositType ;
.

:marine-evaporite-magnesite
    a skos:Concept ;
    rdfs:isDefinedBy cs: ;
    skos:broader :evaporite ;
    skos:definition "Magnesite deposit formed by the evaporation of seawater."@en ;
    skos:inScheme cs: ;
    skos:notation "04.01.04"^^dt:LocalHierarchyKey ;
    skos:prefLabel "Marine evaporite magnesite"@en ;
    schema:additionalType :DepositType ;
.

:marine-evaporite-potash
    a skos:Concept ;
    rdfs:isDefinedBy cs: ;
    skos:broader :evaporite ;
    skos:definition "Potash deposit formed at the surface or in the shallow subsurface by the evaporation of seawater. As a bittern, potash typically only begins to form once seawater reaches 60-70 times its original concentration."@en ;
    skos:inScheme cs: ;
    skos:notation "04.01.03"^^dt:LocalHierarchyKey ;
    skos:prefLabel "Marine evaporite potash"@en ;
    schema:additionalType :DepositType ;
.

:marine-evaporite-salt
    a skos:Concept ;
    rdfs:isDefinedBy cs: ;
    skos:broader :evaporite ;
    skos:definition "Salt deposit formed by the evaporation of seawater. Halite is one of the most volumetrically significant marine evaporite salts."@en ;
    skos:inScheme cs: ;
    skos:notation "04.01.02"^^dt:LocalHierarchyKey ;
    skos:prefLabel "Marine evaporite salt"@en ;
    schema:additionalType :DepositType ;
.

:mesozonal-orogenic-gold
    a skos:Concept ;
    rdfs:isDefinedBy cs: ;
    skos:broader :orogenic ;
    skos:definition "Gold-bearing quartz veins hosted in deformed metamorphic terranes, formed in collisional orogenic belts at depths of 6-12 km and temperatures 300-475C."@en ;
    skos:inScheme cs: ;
    skos:notation "07.01.02"^^dt:LocalHierarchyKey ;
    skos:prefLabel "Mesozonal orogenic gold"@en ;
    schema:additionalType :DepositType ;
.

:metamorphic-graphite
    a skos:Concept ;
    rdfs:isDefinedBy cs: ;
    skos:broader :metamorphic-group ;
    skos:definition "Graphite formed a result of maturation of organic material during sub-greenschist to granulite facies regional or contact metamorphism."@en ;
    skos:inScheme cs: ;
    skos:notation "08.01.01"^^dt:LocalHierarchyKey ;
    skos:prefLabel "Metamorphic graphite"@en ;
    schema:additionalType :DepositType ;
.

:metamorphic-kyanite
    a skos:Concept ;
    rdfs:isDefinedBy cs: ;
    skos:broader :metamorphic-group ;
    skos:definition "Kyanite deposit formed by upper amphibolite facies metamorphism of aluminous sediments, followed by hydrothermal leaching and volcanic alteration."@en ;
    skos:inScheme cs: ;
    skos:notation "08.01.02"^^dt:LocalHierarchyKey ;
    skos:prefLabel "Metamorphic kyanite"@en ;
    schema:additionalType :DepositType ;
.

:mvt-barite
    a skos:Concept ;
    rdfs:isDefinedBy cs: ;
    skos:broader :mississippi-valley-type-mvt ;
    skos:definition "An epigenetic barite deposit formed by replacement of dolostone and limestone by barite with lesser sphalerite, galena, pyrite, and marcasite. MVT deposits form in platform carbonate sequences commonly at the flanks of basins or in foreland thrust belts, where basinal brines source metals and sulfur from the crust and are focused by faults, fractures, collapse breccias, and lithological transitions into the overlying carbonate sequences."@en ;
    skos:inScheme cs: ;
    skos:notation "06.04.02"^^dt:LocalHierarchyKey ;
    skos:prefLabel "MVT barite"@en ;
    schema:additionalType :DepositType ;
.

:mvt-fluorspar
    a skos:Concept ;
    rdfs:isDefinedBy cs: ;
    skos:broader :mississippi-valley-type-mvt ;
    skos:definition "An epigenetic lead-zinc(-fluorspar-barite) deposit formed in carbonate aquifer rocks where a metalliferous and fluorine-rich brine mixed with a second, likely more sulfide-rich brine. Both brines likely have deep basinal groundwater sources, likely including igneous rocks as the fluorine source, mixing at fracture zones or pinched-out confining beds and precipitating sulfides and fluorite. "@en ;
    skos:inScheme cs: ;
    skos:notation "06.04.03"^^dt:LocalHierarchyKey ;
    skos:prefLabel "MVT fluorspar"@en ;
    schema:additionalType :DepositType ;
.

:mvt-strontium
    a skos:Concept ;
    rdfs:isDefinedBy cs: ;
    skos:broader :mississippi-valley-type-mvt ;
    skos:definition "An epigenetic strontium deposit formed in carbonate aquifer rocks where a deep basinal brine mixed with a second, stromtium-rich brine. Both brines likely have deep basinal groundwater sources, likely including volcaniclastic sediments as the strontium source, mixing and precipitating stronium-bearing minerals including celestine. "@en ;
    skos:inScheme cs: ;
    skos:notation "06.04.04"^^dt:LocalHierarchyKey ;
    skos:prefLabel "MVT strontium"@en ;
    schema:additionalType :DepositType ;
.

:mvt-zinc-lead
    a skos:Concept ;
    rdfs:isDefinedBy cs: ;
    skos:broader :mississippi-valley-type-mvt ;
    skos:definition "An epigenetic lead and zinc deposit formed by replacement of dolostone and limestone by sphalerite, galena, pyrite, and marcasite, with lesser barite. MVT deposits form in platform carbonate sequences commonly at the flanks of basins or in foreland thrust belts, where basinal brines source metals and sulfur from the crust and are focused by faults, fractures, collapse breccias, and lithological transitions into the overlying carbonate sequences."@en ;
    skos:inScheme cs: ;
    skos:notation "06.04.01"^^dt:LocalHierarchyKey ;
    skos:prefLabel "MVT zinc-lead"@en ;
    schema:additionalType :DepositType ;
.

:nodular-magnesite
    a skos:Concept ;
    rdfs:isDefinedBy cs: ;
    skos:broader :magnesite ;
    skos:definition "Coarse-grained magnesite deposits occurring in carbonates as well as sandstones and other clastic sediments. Ore zones are lens-shapes, stratabound and typically stratiform."@en ;
    skos:inScheme cs: ;
    skos:notation "03.04.01"^^dt:LocalHierarchyKey ;
    skos:prefLabel "Nodular magnesite"@en ;
    schema:additionalType :DepositType ;
.

:nodule-manganese
    a skos:Concept ;
    rdfs:isDefinedBy cs: ;
    skos:broader :manganese ;
    skos:definition "Nodular manganese deposits are composed of ferromanganese oxidesand form by hydrogenetic or diagentic precipitation around a hard nuceleus on the surface or in the subsurface of soft seafloor sediment."@en ;
    skos:inScheme cs: ;
    skos:notation "05.04.01"^^dt:LocalHierarchyKey ;
    skos:prefLabel "Nodule manganese"@en ;
    schema:additionalType :DepositType ;
.

:non-sulfide-zinc-lead-mn
    a skos:Concept ;
    rdfs:isDefinedBy cs: ;
    skos:broader :non-sulfide ;
    skos:definition "A non-sulfide hypogene zinc-lead deposit comprising zinc silicates and oxides, with minor sphalerite. Deposits occur primarily within carbonate rocks and may be stratiform lenses or structurally controlled veins and irregular pipes. "@en ;
    skos:inScheme cs: ;
    skos:notation "06.05.01"^^dt:LocalHierarchyKey ;
    skos:prefLabel "Non-sulfide zinc-lead ± Mn"@en ;
    schema:additionalType :DepositType ;
.

:nyf-pegmatite
    a skos:Concept ;
    rdfs:isDefinedBy cs: ;
    skos:broader :pegmatite ;
    skos:definition "Pegmatites enriched in niobium, yttrium and flourine."@en ;
    skos:inScheme cs: ;
    skos:notation "12.01.01"^^dt:LocalHierarchyKey ;
    skos:prefLabel "NYF pegmatite"@en ;
    schema:additionalType :DepositType ;
.

:oolitic-iron-formation
    a skos:Concept ;
    rdfs:isDefinedBy cs: ;
    skos:broader :iron-formation ;
    skos:definition "Beds rich in iron silicate and oxide minerals with oolitic texture, deposited in shallow-shelf to intertidal, clastic dominated environments. Lacks layered chert and primary siderite."@en ;
    skos:inScheme cs: ;
    skos:notation "05.03.02"^^dt:LocalHierarchyKey ;
    skos:prefLabel "Oolitic iron formation"@en ;
    schema:additionalType :DepositType ;
.

:ophiolite-chromium
    a skos:Concept ;
    rdfs:isDefinedBy cs: ;
    skos:broader :ophiolite ;
    skos:definition "An ophiolite hosted chromium (Cr) deposit."@en ;
    skos:inScheme cs: ;
    skos:notation "12.11.01"^^dt:LocalHierarchyKey ;
    skos:prefLabel "Ophiolite chromium"@en ;
    schema:additionalType :DepositType ;
.

:ophiolite-nickel-copper-pge
    a skos:Concept ;
    rdfs:isDefinedBy cs: ;
    skos:broader :ophiolite ;
    skos:definition "An ophiolite hosted nickel-copper-platinum-group elements (PGE) deposit."@en ;
    skos:inScheme cs: ;
    skos:notation "12.11.02"^^dt:LocalHierarchyKey ;
    skos:prefLabel "Ophiolite nickel-copper-PGE"@en ;
    schema:additionalType :DepositType ;
.

:orogenic-copper-gold
    a skos:Concept ;
    rdfs:isDefinedBy cs: ;
    skos:broader :orogenic ;
    skos:definition "Copper-gold-bearing pipes, lenses and veins in basin sedimentary sequences. Mineralization occurs during basin inversion and is focused into sites of dilation. Orebodies are mostly sulfidic, with some magnetite or pyrrhotite. "@en ;
    skos:inScheme cs: ;
    skos:notation "07.01.07"^^dt:LocalHierarchyKey ;
    skos:prefLabel "Orogenic copper ± gold"@en ;
    schema:additionalType :DepositType ;
.

:orogenic-graphite
    a skos:Concept ;
    rdfs:isDefinedBy cs: ;
    skos:broader :orogenic ;
    skos:definition "Graphite-bearing veins and graphite-rich zones formed by precipitation from metamorphic or metasomatic C-O-H fluid. Mineralization is triggered by changes in temperature and pressure, fluid buffering, or by mixing with another fluid."@en ;
    skos:inScheme cs: ;
    skos:notation "07.01.08"^^dt:LocalHierarchyKey ;
    skos:prefLabel "Orogenic graphite"@en ;
    schema:additionalType :DepositType ;
.

:orogenic-silver-lead-zinc-copper-antimony
    a skos:Concept ;
    rdfs:isDefinedBy cs: ;
    skos:broader :orogenic ;
    skos:definition "Silver-lead-zinc-copper-antimony-bearing veins in deformed metamorphic terranes, formed in collisional orogenic belts at average depths of 6 km and temperates 250-300C. Veins are often spatially associated with a crustal-scale fault."@en ;
    skos:inScheme cs: ;
    skos:notation "07.01.06"^^dt:LocalHierarchyKey ;
    skos:prefLabel "Orogenic silver-lead-zinc-copper-antimony"@en ;
    schema:additionalType :DepositType ;
.

:oxidized-intrusion-related-gold
    a skos:Concept ;
    rdfs:isDefinedBy cs: ;
    skos:broader :intrusion-related ;
    skos:definition "Not yet available"@en ;
    skos:inScheme cs: ;
    skos:notation "11.10.02"^^dt:LocalHierarchyKey ;
    skos:prefLabel "Oxidized intrusion-related gold"@en ;
    schema:additionalType :DepositType ;
.

:paleochannel-iron
    a skos:Concept ;
    rdfs:isDefinedBy cs: ;
    skos:broader :paleochannel ;
    skos:definition "Concentrations of iron bearing minerals within paleochannels."@en ;
    skos:inScheme cs: ;
    skos:notation "03.02.01"^^dt:LocalHierarchyKey ;
    skos:prefLabel "Paleochannel iron"@en ;
    schema:additionalType :DepositType ;
.

:paleoplacer-gold-uranium
    a skos:Concept ;
    rdfs:isDefinedBy cs: ;
    skos:broader :placer ;
    skos:definition "Placer concentrations of gold ± uranium formed in the geological past and now hosted in a consolidated rock."@en ;
    skos:inScheme cs: ;
    skos:notation "01.01.15"^^dt:LocalHierarchyKey ;
    skos:prefLabel "Paleoplacer gold ± uranium"@en ;
    schema:additionalType :DepositType ;
.

:paleoplacer-heavy-mineral-sands
    a skos:Concept ;
    rdfs:isDefinedBy cs: ;
    skos:broader :placer ;
    skos:definition "Placer concentrations of heavy mineral sands formed in the geological past and now hosted in a consolidated rock."@en ;
    skos:inScheme cs: ;
    skos:notation "01.01.14"^^dt:LocalHierarchyKey ;
    skos:prefLabel "Paleoplacer heavy mineral sands"@en ;
    schema:additionalType :DepositType ;
.

:paleoplacer-tin
    a skos:Concept ;
    rdfs:isDefinedBy cs: ;
    skos:broader :placer ;
    skos:definition "Placer concentrations of tin bearing minerals formed in the geological past and now hosted in a consolidated rock."@en ;
    skos:inScheme cs: ;
    skos:notation "01.01.13"^^dt:LocalHierarchyKey ;
    skos:prefLabel "Paleoplacer tin"@en ;
    schema:additionalType :DepositType ;
.

:peralkaline-igneous-hfse-ree
    a skos:Concept ;
    rdfs:isDefinedBy cs: ;
    skos:broader :peralkaline-igneous ;
    skos:definition "High field strength and rare earth element mineralisation associated with peralkaline igneous rocks. Mineralisation is related to crystallisation of the igneous rock and late magmatic to hydrothermal fluids."@en ;
    skos:inScheme cs: ;
    skos:notation "12.03.01"^^dt:LocalHierarchyKey ;
    skos:prefLabel "Peralkaline igneous HFSE-REE"@en ;
    schema:additionalType :DepositType ;
.

:phosphorite-group
    a skos:Concept ;
    rdfs:isDefinedBy cs: ;
    skos:broader :phosphorite ;
    skos:definition "A stratiform or lens-shaped sedimentary rock with a high content of phosphate minerals. Most commonly it is a bedded primary or reworked secondary marine rock composed of microcrystalline carbonate fluorapatite in the form of laminae, pellets, oolites, nodules and skeletal, shell and bone fragments. Commodities may include fluorine, REE, vanadium, uranium, and gypsum."@en ;
    skos:inScheme cs: ;
    skos:notation "05.02.01"^^dt:LocalHierarchyKey ;
    skos:prefLabel "Phosphorite"@en ;
    schema:additionalType :DepositType ;
.

:porphyry-gold-copper
    a skos:Concept ;
    rdfs:isDefinedBy cs: ;
    skos:broader :porphyry ;
    skos:definition "Not yet available"@en ;
    skos:inScheme cs: ;
    skos:notation "11.08.03"^^dt:LocalHierarchyKey ;
    skos:prefLabel "Porphyry gold ± copper"@en ;
    schema:additionalType :DepositType ;
.

:porphyry-copper-gold
    a skos:Concept ;
    rdfs:isDefinedBy cs: ;
    skos:broader :porphyry ;
    skos:definition "Not yet available"@en ;
    skos:inScheme cs: ;
    skos:notation "11.08.01"^^dt:LocalHierarchyKey ;
    skos:prefLabel "Porphyry copper ± gold"@en ;
    schema:additionalType :DepositType ;
.

:porphyry-copper-molybdenum
    a skos:Concept ;
    rdfs:isDefinedBy cs: ;
    skos:broader :porphyry ;
    skos:definition "Not yet available"@en ;
    skos:inScheme cs: ;
    skos:notation "11.08.02"^^dt:LocalHierarchyKey ;
    skos:prefLabel "Porphyry copper-molybdenum"@en ;
    schema:additionalType :DepositType ;
.

:porphyry-tin
    a skos:Concept ;
    rdfs:isDefinedBy cs: ;
    skos:broader :porphyry ;
    skos:definition "Not yet available"@en ;
    skos:inScheme cs: ;
    skos:notation "11.08.07"^^dt:LocalHierarchyKey ;
    skos:prefLabel "Porphyry tin"@en ;
    schema:additionalType :DepositType ;
.

:porphyry-tungsten
    a skos:Concept ;
    rdfs:isDefinedBy cs: ;
    skos:broader :porphyry ;
    skos:definition "Not yet available"@en ;
    skos:inScheme cs: ;
    skos:notation "11.08.06"^^dt:LocalHierarchyKey ;
    skos:prefLabel "Porphyry tungsten"@en ;
    schema:additionalType :DepositType ;
.

:reduced-intrusion-related-gold
    a skos:Concept ;
    rdfs:isDefinedBy cs: ;
    skos:broader :intrusion-related ;
    skos:definition "Not yet available"@en ;
    skos:inScheme cs: ;
    skos:notation "11.10.01"^^dt:LocalHierarchyKey ;
    skos:prefLabel "Reduced intrusion-related gold"@en ;
    schema:additionalType :DepositType ;
.

:replacement-gold-silver
    a skos:Concept ;
    rdfs:isDefinedBy cs: ;
    skos:broader :replacement ;
    skos:definition "A gold-silver deposit formed by replacement processes."@en ;
    skos:inScheme cs: ;
    skos:notation "11.06.02"^^dt:LocalHierarchyKey ;
    skos:prefLabel "Replacement gold-silver"@en ;
    schema:additionalType :DepositType ;
.

:replacement-copper
    a skos:Concept ;
    rdfs:isDefinedBy cs: ;
    skos:broader :replacement ;
    skos:definition "A copper deposit formed by replacement processes."@en ;
    skos:inScheme cs: ;
    skos:notation "11.06.04"^^dt:LocalHierarchyKey ;
    skos:prefLabel "Replacement copper"@en ;
    schema:additionalType :DepositType ;
.

:replacement-fluorite
    a skos:Concept ;
    rdfs:isDefinedBy cs: ;
    skos:broader :replacement ;
    skos:definition "A flourite deposit formed by replacement processes."@en ;
    skos:inScheme cs: ;
    skos:notation "11.06.08"^^dt:LocalHierarchyKey ;
    skos:prefLabel "Replacement fluorite"@en ;
    schema:additionalType :DepositType ;
.

:replacement-magnesium
    a skos:Concept ;
    rdfs:isDefinedBy cs: ;
    skos:broader :replacement ;
    skos:definition "A magnesium deposit formed by replacement processes."@en ;
    skos:inScheme cs: ;
    skos:notation "11.06.07"^^dt:LocalHierarchyKey ;
    skos:prefLabel "Replacement magnesium"@en ;
    schema:additionalType :DepositType ;
.

:replacement-manganese
    a skos:Concept ;
    rdfs:isDefinedBy cs: ;
    skos:broader :replacement ;
    skos:definition "A manganese deposit formed by replacement processes."@en ;
    skos:inScheme cs: ;
    skos:notation "11.06.06"^^dt:LocalHierarchyKey ;
    skos:prefLabel "Replacement manganese"@en ;
    schema:additionalType :DepositType ;
.

:replacement-polymetallic
    a skos:Concept ;
    rdfs:isDefinedBy cs: ;
    skos:broader :replacement ;
    skos:definition "A mineral deposit formed by the replacement of sedimentary rocks by metal bearing fluids associated with igneous intrusions."@en ;
    skos:inScheme cs: ;
    skos:notation "11.06.01"^^dt:LocalHierarchyKey ;
    skos:prefLabel "Replacement polymetallic"@en ;
    schema:additionalType :DepositType ;
.

:replacement-tin
    a skos:Concept ;
    rdfs:isDefinedBy cs: ;
    skos:broader :replacement ;
    skos:definition "A tin deposit formed by replacement processes."@en ;
    skos:inScheme cs: ;
    skos:notation "11.06.03"^^dt:LocalHierarchyKey ;
    skos:prefLabel "Replacement tin"@en ;
    schema:additionalType :DepositType ;
.

:replacement-zinc-lead
    a skos:Concept ;
    rdfs:isDefinedBy cs: ;
    skos:broader :replacement ;
    skos:definition "A zinc-lead deposit formed by replacement processes."@en ;
    skos:inScheme cs: ;
    skos:notation "11.06.05"^^dt:LocalHierarchyKey ;
    skos:prefLabel "Replacement zinc-lead"@en ;
    schema:additionalType :DepositType ;
.

:residual-clay
    a skos:Concept ;
    rdfs:isDefinedBy cs: ;
    skos:broader :clay-supergene ;
    skos:definition "Clay material formed in place by the weathering of rock, derived either from the chemical decay minerals or from the removal of non-clay-mineral constituents by solution from a clay-bearing rock (such as an argillaceous limestone)."@en ;
    skos:inScheme cs: ;
    skos:notation "02.02.01"^^dt:LocalHierarchyKey ;
    skos:prefLabel "Residual clay"@en ;
    schema:additionalType :DepositType ;
.

:residual-placer-lead
    a skos:Concept ;
    rdfs:isDefinedBy cs: ;
    skos:broader :placer ;
    skos:definition "A lead deposit formed by the conentration of tin bearing minerals  near the parent rock via the weathering of surrounding lighter and less stable material."@en ;
    skos:inScheme cs: ;
    skos:notation "01.01.02"^^dt:LocalHierarchyKey ;
    skos:prefLabel "Residual placer lead"@en ;
    schema:additionalType :DepositType ;
.

:residual-placer-tin
    a skos:Concept ;
    rdfs:isDefinedBy cs: ;
    skos:broader :placer ;
    skos:definition "A tin deposit formed by the conentration of tin bearing minerals  near the parent rock via the weathering of surrounding lighter and less stable material."@en ;
    skos:inScheme cs: ;
    skos:notation "01.01.01"^^dt:LocalHierarchyKey ;
    skos:prefLabel "Residual placer tin"@en ;
    schema:additionalType :DepositType ;
.

:sandstone-hosted-zinc-lead
    a skos:Concept ;
    rdfs:isDefinedBy cs: ;
    skos:broader :mississippi-valley-type-mvt ;
    skos:definition "Stratabound to stratiform galena and sphalerite in multiple, thin, sheetlike ore bodies in sandstones. Sandstones may include local conglomerate, grit, siltstone, and evaporite components deposited in combined continental and marine environments during deep weathering in stable tectonic conditions."@en ;
    skos:inScheme cs: ;
    skos:notation "06.04.05"^^dt:LocalHierarchyKey ;
    skos:prefLabel "Sandstone-hosted zinc-lead"@en ;
    schema:additionalType :DepositType ;
.

:sandstone-uranium
    a skos:Concept ;
    rdfs:isDefinedBy cs: ;
    skos:broader :uranium ;
    skos:definition "Uranium accumulations in medium- to coarse-grained siliciclastic sedimentary rocks deposited in fluvial, lacustrine, or shallow-marine environments. Uranium is precipitated by reduction processes caused by the presence of agents including detrital plant debris, sulfides, ferro-magnesian minerals, sulfate-reducing bacteria, or migrating fluids."@en ;
    skos:inScheme cs: ;
    skos:notation "03.03.01"^^dt:LocalHierarchyKey ;
    skos:prefLabel "Sandstone uranium"@en ;
    schema:additionalType :DepositType ;
.

:sediment-hosted-copper-co
    a skos:Concept ;
    rdfs:isDefinedBy cs: ;
    skos:broader :sediment-hosted ;
    skos:definition "Disseminated, cementing, and veinlet-hosted copper minerals peneconformable with their sedimentary or metasedimentary host rocks. Ore minerals have strong lateral zoning. Host rocks are typically a reduced facies (fine grained sediments or carbonaceous dolosiltstone), fine to coarse grained sandstones, or red-bed fluvial sandstones."@en ;
    skos:inScheme cs: ;
    skos:notation "06.03.01"^^dt:LocalHierarchyKey ;
    skos:prefLabel "Sediment-hosted copper ± Co"@en ;
    schema:additionalType :DepositType ;
.

:sedimentary-manganese
    a skos:Concept ;
    rdfs:isDefinedBy cs: ;
    skos:broader :manganese ;
    skos:definition "Laterally extensive beds of manganite, psilomelane, rhodochrosite and other manganese within marine sediments. Textures include oolites, pisolites, rhythmic laminations, slumped bedding, hard-ground fragments and fossils. These form in shallow marine settings in interior or marginal basins on stable cratons."@en ;
    skos:inScheme cs: ;
    skos:notation "05.04.03"^^dt:LocalHierarchyKey ;
    skos:prefLabel "Sedimentary manganese"@en ;
    schema:additionalType :DepositType ;
.

:shoreline-placer-gold
    a skos:Concept ;
    rdfs:isDefinedBy cs: ;
    skos:broader :placer ;
    skos:definition "A gold deposit formed by the concentration of gold bearing minerals on the upper parts of beaches through wave action."@en ;
    skos:inScheme cs: ;
    skos:notation "01.01.12"^^dt:LocalHierarchyKey ;
    skos:prefLabel "Shoreline placer gold"@en ;
    schema:additionalType :DepositType ;
.

:siliciclastic-carbonate-zinc-lead
    a skos:Concept ;
    rdfs:isDefinedBy cs: ;
    skos:broader :sediment-hosted ;
    skos:definition "Tabular or stratiform zinc-lead orebodies hosted by marine siliciclastic or carbonate rocks of basin-sag phase sequences. Principal ore minerals sphalerite and galena precipitated from warm, saline basin brines of or just below the seafloor."@en ;
    skos:inScheme cs: ;
    skos:notation "06.03.04"^^dt:LocalHierarchyKey ;
    skos:prefLabel "Siliciclastic-carbonate zinc-lead"@en ;
    schema:additionalType :DepositType ;
.

:siliciclastic-mafic-barite
    a skos:Concept ;
    rdfs:isDefinedBy cs: ;
    skos:broader :sediment-hosted ;
    skos:definition "Fine grained and finely laminated barite in siliciclastic basin sequences, and/or barite clasts incorporated into turbidites and debris flows. Barite precipitates on or just below the seafloor from hydrothermal brines, which can migrate some distance from the discharge zone."@en ;
    skos:inScheme cs: ;
    skos:notation "06.03.03"^^dt:LocalHierarchyKey ;
    skos:prefLabel "Siliciclastic-mafic barite"@en ;
    schema:additionalType :DepositType ;
.

:siliciclastic-mafic-zinc-lead
    a skos:Concept ;
    rdfs:isDefinedBy cs: ;
    skos:broader :sediment-hosted ;
    skos:definition "Massive to semimassive galena, sphalerite, pyrrhotite, pyrite, and/or magnetite layers or stacked lenses hosted by thinly bedded paragneiss successions. Associated with bimodal volcanics reflecting active extensional tectonics. Host successions are generally interpreted as shallow marine environments. Host and mineralisation are strongly deformed and metamorphosed."@en ;
    skos:inScheme cs: ;
    skos:notation "06.03.02"^^dt:LocalHierarchyKey ;
    skos:prefLabel "Siliciclastic-mafic zinc-lead"@en ;
    schema:additionalType :DepositType ;
.

:simple-pegmatite
    a skos:Concept ;
    rdfs:isDefinedBy cs: ;
    skos:broader :pegmatite ;
    skos:definition "Not yet available"@en ;
    skos:inScheme cs: ;
    skos:notation "12.01.02"^^dt:LocalHierarchyKey ;
    skos:prefLabel "Simple pegmatite"@en ;
    schema:additionalType :DepositType ;
.

:skarn-gold-copper-tungsten
    a skos:Concept ;
    rdfs:isDefinedBy cs: ;
    skos:broader :skarn ;
    skos:definition "A skarn deposit containing a significant concentration of gold, copper and tungsten formed formed by the replacement of carbonate rocks by contact metamorphism and metasomatism."@en ;
    skos:inScheme cs: ;
    skos:notation "11.07.04"^^dt:LocalHierarchyKey ;
    skos:prefLabel "Skarn gold ± copper ± tungsten"@en ;
    schema:additionalType :DepositType ;
.

:skarn-beryllium-fluorite
    a skos:Concept ;
    rdfs:isDefinedBy cs: ;
    skos:broader :skarn ;
    skos:definition "A skarn deposit containing a significant concentration of beryllium and fluorite formed formed by the replacement of carbonate rocks by contact metamorphism and metasomatism."@en ;
    skos:inScheme cs: ;
    skos:notation "11.07.07"^^dt:LocalHierarchyKey ;
    skos:prefLabel "Skarn beryllium-fluorite"@en ;
    schema:additionalType :DepositType ;
.

:skarn-copper
    a skos:Concept ;
    rdfs:isDefinedBy cs: ;
    skos:broader :skarn ;
    skos:definition "A skarn deposit containing a significant concentration of copper, formed formed by the replacement of carbonate rocks by contact metamorphism and metasomatism."@en ;
    skos:inScheme cs: ;
    skos:notation "11.07.01"^^dt:LocalHierarchyKey ;
    skos:prefLabel "Skarn copper"@en ;
    schema:additionalType :DepositType ;
.

:skarn-molybdenum
    a skos:Concept ;
    rdfs:isDefinedBy cs: ;
    skos:broader :skarn ;
    skos:definition "A skarn deposit containing a significant concentration of molybdenum formed formed by the replacement of carbonate rocks by contact metamorphism and metasomatism."@en ;
    skos:inScheme cs: ;
    skos:notation "11.07.06"^^dt:LocalHierarchyKey ;
    skos:prefLabel "Skarn molybdenum"@en ;
    schema:additionalType :DepositType ;
.

:skarn-tin-copper-mo
    a skos:Concept ;
    rdfs:isDefinedBy cs: ;
    skos:broader :skarn ;
    skos:definition "A skarn deposit containing a significant concentration of tin, copper and molybdenum, formed formed by the replacement of carbonate rocks by contact metamorphism and metasomatism."@en ;
    skos:inScheme cs: ;
    skos:notation "11.07.03"^^dt:LocalHierarchyKey ;
    skos:prefLabel "Skarn tin ± copper ± Mo"@en ;
    schema:additionalType :DepositType ;
.

:skarn-uranium-ree
    a skos:Concept ;
    rdfs:isDefinedBy cs: ;
    skos:broader :skarn ;
    skos:definition "A skarn deposit containing a significant concentration of uranium and REEs formed formed by the replacement of carbonate rocks by contact metamorphism and metasomatism."@en ;
    skos:inScheme cs: ;
    skos:notation "11.07.08"^^dt:LocalHierarchyKey ;
    skos:prefLabel "Skarn uranium-REE"@en ;
    schema:additionalType :DepositType ;
.

:skarn-tungsten-mo
    a skos:Concept ;
    rdfs:isDefinedBy cs: ;
    skos:broader :skarn ;
    skos:definition "A skarn deposit containing a significant concentration of tungsten and molybdenum, formed formed by the replacement of carbonate rocks by contact metamorphism and metasomatism."@en ;
    skos:inScheme cs: ;
    skos:notation "11.07.02"^^dt:LocalHierarchyKey ;
    skos:prefLabel "Skarn tungsten ± Mo"@en ;
    schema:additionalType :DepositType ;
.

:skarn-zinc-lead-silver
    a skos:Concept ;
    rdfs:isDefinedBy cs: ;
    skos:broader :skarn ;
    skos:definition "A skarn deposit containing a significant concentration of zinc, lead and silver formed formed by the replacement of carbonate rocks by contact metamorphism and metasomatism."@en ;
    skos:inScheme cs: ;
    skos:notation "11.07.05"^^dt:LocalHierarchyKey ;
    skos:prefLabel "Skarn zinc-lead-silver"@en ;
    schema:additionalType :DepositType ;
.

:supergene-copper
    a skos:Concept ;
    rdfs:isDefinedBy cs: ;
    skos:broader :supergene-group ;
    skos:definition "A copper deposit resulting from release by chemical weathering of soluble minerals and concentration by chemical gradients associated with the downward percolation of meteoric water in the unsaturated zone."@en ;
    skos:inScheme cs: ;
    skos:notation "02.03.07"^^dt:LocalHierarchyKey ;
    skos:prefLabel "Supergene copper"@en ;
    schema:additionalType :DepositType ;
.

:supergene-gold
    a skos:Concept ;
    rdfs:isDefinedBy cs: ;
    skos:broader :supergene-group ;
    skos:definition "A gold deposit resulting from release by chemical weathering of soluble minerals and concentration by chemical gradients associated with the downward percolation of meteoric water in the unsaturated zone."@en ;
    skos:inScheme cs: ;
    skos:notation "02.03.05"^^dt:LocalHierarchyKey ;
    skos:prefLabel "Supergene gold"@en ;
    schema:additionalType :DepositType ;
.

:supergene-iron
    a skos:Concept ;
    rdfs:isDefinedBy cs: ;
    skos:broader :supergene-group ;
    skos:definition "A iron deposit resulting from release by chemical weathering of soluble minerals and concentration by chemical gradients associated with the downward percolation of meteoric water in the unsaturated zone."@en ;
    skos:inScheme cs: ;
    skos:notation "02.03.09"^^dt:LocalHierarchyKey ;
    skos:prefLabel "Supergene iron"@en ;
    schema:additionalType :DepositType ;
.

:supergene-lead
    a skos:Concept ;
    rdfs:isDefinedBy cs: ;
    skos:broader :supergene-group ;
    skos:definition "A lead deposit resulting from release by chemical weathering of soluble minerals and concentration by chemical gradients associated with the downward percolation of meteoric water in the unsaturated zone."@en ;
    skos:inScheme cs: ;
    skos:notation "02.03.02"^^dt:LocalHierarchyKey ;
    skos:prefLabel "Supergene lead"@en ;
    schema:additionalType :DepositType ;
.

:supergene-manganese
    a skos:Concept ;
    rdfs:isDefinedBy cs: ;
    skos:broader :supergene-group ;
    skos:definition "A manganese deposit resulting from release by chemical weathering of soluble minerals and concentration by chemical gradients associated with the downward percolation of meteoric water in the unsaturated zone."@en ;
    skos:inScheme cs: ;
    skos:notation "02.03.08"^^dt:LocalHierarchyKey ;
    skos:prefLabel "Supergene manganese"@en ;
    schema:additionalType :DepositType ;
.

:supergene-silver
    a skos:Concept ;
    rdfs:isDefinedBy cs: ;
    skos:broader :supergene-group ;
    skos:definition "A silver deposit resulting from release by chemical weathering of soluble minerals and concentration by chemical gradients associated with the downward percolation of meteoric water in the unsaturated zone."@en ;
    skos:inScheme cs: ;
    skos:notation "02.03.01"^^dt:LocalHierarchyKey ;
    skos:prefLabel "Supergene silver"@en ;
    schema:additionalType :DepositType ;
.

:supergene-uranium
    a skos:Concept ;
    rdfs:isDefinedBy cs: ;
    skos:broader :supergene-group ;
    skos:definition "A uranium deposit resulting from release by chemical weathering of soluble minerals and concentration by chemical gradients associated with the downward percolation of meteoric water in the unsaturated zone."@en ;
    skos:inScheme cs: ;
    skos:notation "02.03.03"^^dt:LocalHierarchyKey ;
    skos:prefLabel "Supergene uranium"@en ;
    schema:additionalType :DepositType ;
.

:supergene-vanadium
    a skos:Concept ;
    rdfs:isDefinedBy cs: ;
    skos:broader :supergene-group ;
    skos:definition "A vanadium deposit resulting from release by chemical weathering of soluble minerals and concentration by chemical gradients associated with the downward percolation of meteoric water in the unsaturated zone."@en ;
    skos:inScheme cs: ;
    skos:notation "02.03.04"^^dt:LocalHierarchyKey ;
    skos:prefLabel "Supergene vanadium"@en ;
    schema:additionalType :DepositType ;
.

:supergene-zinc
    a skos:Concept ;
    rdfs:isDefinedBy cs: ;
    skos:broader :supergene-group ;
    skos:definition "A zinc deposit resulting from release by chemical weathering of soluble minerals and concentration by chemical gradients associated with the downward percolation of meteoric water in the unsaturated zone."@en ;
    skos:inScheme cs: ;
    skos:notation "02.03.06"^^dt:LocalHierarchyKey ;
    skos:prefLabel "Supergene zinc"@en ;
    schema:additionalType :DepositType ;
.

:superior-type-banded-iron-formation
    a skos:Concept ;
    rdfs:isDefinedBy cs: ;
    skos:broader :iron-formation ;
    skos:definition "Banded iron-rich sedimentary rock, generally laterally extensive, typically layered on a centimeter scale with siliceous beds."@en ;
    skos:inScheme cs: ;
    skos:notation "05.03.01"^^dt:LocalHierarchyKey ;
    skos:prefLabel "Superior-type banded iron formation"@en ;
    schema:additionalType :DepositType ;
.

:superior-type-banded-manganese
    a skos:Concept ;
    rdfs:isDefinedBy cs: ;
    skos:broader :manganese ;
    skos:definition "Laminated manganese-rich sedimentary rock comprising microcrystalline Mn-bearing carbonates, braunite and hematite."@en ;
    skos:inScheme cs: ;
    skos:notation "05.04.02"^^dt:LocalHierarchyKey ;
    skos:prefLabel "Superior-type banded manganese"@en ;
    schema:additionalType :DepositType ;
.

:u-m-conduit-nickel-copper-pge
    a skos:Concept ;
    rdfs:isDefinedBy cs: ;
    skos:broader :ultramafic-and-or-mafic-conduit ;
    skos:definition "Nickel-copper-platinum group element mineralisation associated with conduits underlying ultramafic to mafic large igneous provinces. Conduits are represented by sill complexes that crystallised and cooled at shallow depths. Ore-bearing intrusions have an elongate, finger-like shapes."@en ;
    skos:inScheme cs: ;
    skos:notation "12.10.01"^^dt:LocalHierarchyKey ;
    skos:prefLabel "U-M conduit nickel-copper-PGE"@en ;
    schema:additionalType :DepositType ;
.

:u-m-intrusion-nickel-copper-pge
    a skos:Concept ;
    rdfs:isDefinedBy cs: ;
    skos:broader :ultramafic-and-or-mafic-intrusion ;
    skos:definition "Mafic to ultramafic intrusion containing a significant concentration of nickel (Ni), copper (Cu) and platinum-group elements (PGE).  Mafic to ultramafic Ni-Cu-PGE intrusions host some of the world's largest nickel deposits."@en ;
    skos:inScheme cs: ;
    skos:notation "12.09.02"^^dt:LocalHierarchyKey ;
    skos:prefLabel "U-M intrusion nickel-copper-PGE"@en ;
    schema:additionalType :DepositType ;
.

:u-m-layered-intrusion-chromium
    a skos:Concept ;
    rdfs:isDefinedBy cs: ;
    skos:broader :ultramafic-and-or-mafic-layered-intrusion ;
    skos:definition "A mafic-ultramafic layered intrusion containing significant concentrations of chromium (Cr)."@en ;
    skos:inScheme cs: ;
    skos:notation "12.08.01"^^dt:LocalHierarchyKey ;
    skos:prefLabel "U-M layered intrusion chromium"@en ;
    schema:additionalType :DepositType ;
.

:u-m-layered-intrusion-iron-titanium-vanadium
    a skos:Concept ;
    rdfs:isDefinedBy cs: ;
    skos:broader :ultramafic-and-or-mafic-layered-intrusion ;
    skos:definition "A mafic-ultramafic layered intrusion containing significant concentrations of iron (Fe), titatnium (Ti) and vanadium (V)."@en ;
    skos:inScheme cs: ;
    skos:notation "12.08.02"^^dt:LocalHierarchyKey ;
    skos:prefLabel "U-M layered intrusion iron-titanium-vanadium"@en ;
    schema:additionalType :DepositType ;
.

:u-m-layered-intrusion-nickel-copper-pge
    a skos:Concept ;
    rdfs:isDefinedBy cs: ;
    skos:broader :ultramafic-and-or-mafic-layered-intrusion ;
    skos:definition "A mafic-ultramafic layered intrusion containing significant concentrations of nickel (Ni), copper (Cu) and platinum-group elements (PGE)."@en ;
    skos:inScheme cs: ;
    skos:notation "12.08.04"^^dt:LocalHierarchyKey ;
    skos:prefLabel "U-M layered intrusion nickel-copper-PGE"@en ;
    schema:additionalType :DepositType ;
.

:u-m-layered-intrusion-pge
    a skos:Concept ;
    rdfs:isDefinedBy cs: ;
    skos:broader :ultramafic-and-or-mafic-layered-intrusion ;
    skos:definition "A mafic-ultramafic layered intrusion containing significant concentrations of platinum-group elements (PGE)."@en ;
    skos:inScheme cs: ;
    skos:notation "12.08.03"^^dt:LocalHierarchyKey ;
    skos:prefLabel "U-M layered intrusion PGE"@en ;
    schema:additionalType :DepositType ;
.

:unconformity-related-ree
    a skos:Concept ;
    rdfs:isDefinedBy cs: ;
    skos:broader :unconformity-related ;
    skos:definition "A REE deposit occurring in fault zones at and immediately above or below a prominent regional unconformity. REEs are sourced from the underlying metamorphic basement rocks and mobilised into fault zones by fluids. Mixing of fluids at the unconformity results in precipitation of REE-bearing minerals, principally xenotime."@en ;
    skos:inScheme cs: ;
    skos:notation "06.01.02"^^dt:LocalHierarchyKey ;
    skos:prefLabel "Unconformity-related REE"@en ;
    schema:additionalType :DepositType ;
.

:unconformity-related-uranium
    a skos:Concept ;
    rdfs:isDefinedBy cs: ;
    skos:broader :unconformity-related ;
    skos:definition "A uranium deposit ocurring at and immediately above or below an unconformity separating relatively undeformed, intracratonic sandstone basins from underlying metamorphic basement rocks. Ore bodies are structurally controlled pods, veins, breccias and replacements with extensive domains of alteration."@en ;
    skos:inScheme cs: ;
    skos:notation "06.01.01"^^dt:LocalHierarchyKey ;
    skos:prefLabel "Unconformity-related uranium"@en ;
    schema:additionalType :DepositType ;
.

:underclay-overclay
    a skos:Concept ;
    rdfs:isDefinedBy cs: ;
    skos:broader :clay-supergene ;
    skos:definition "** doesn't describe overclays yet** Massive, non-bedded clay layers underlying horizons of coal, usually containing cracks with slickensides. Underclays are thought to represent paleosols pre-dating deposition of coal, or have formed as a result of alteration or diagenesis."@en ;
    skos:inScheme cs: ;
    skos:notation "02.02.02"^^dt:LocalHierarchyKey ;
    skos:prefLabel
        "Underclay, overclay"@en ;
    schema:additionalType :DepositType ;
.

:vein-cobalt-ni
    a skos:Concept ;
    rdfs:isDefinedBy cs: ;
    skos:broader :vein ;
    skos:definition "Veins containing mineralised copper and or nickel."@en ;
    skos:inScheme cs: ;
    skos:notation "11.02.02"^^dt:LocalHierarchyKey ;
    skos:prefLabel "Vein cobalt ± Ni"@en ;
    schema:additionalType :DepositType ;
.

:vein-copper
    a skos:Concept ;
    rdfs:isDefinedBy cs: ;
    skos:broader :vein ;
    skos:definition "Veins containing mineralised copper."@en ;
    skos:inScheme cs: ;
    skos:notation "11.02.03"^^dt:LocalHierarchyKey ;
    skos:prefLabel "Vein copper"@en ;
    schema:additionalType :DepositType ;
.

:vein-five-element
    a skos:Concept ;
    rdfs:isDefinedBy cs: ;
    skos:broader :five-element ;
    skos:definition "Hydrothermal vein deposits dominated by nickel-copper-arsenides ± native elements. Mineralisation is not restricted to five elements but can include a wide variety of arsenides, sulfarsenides, and/or native elements. "@en ;
    skos:inScheme cs: ;
    skos:notation "06.06.01"^^dt:LocalHierarchyKey ;
    skos:prefLabel "Vein five-element"@en ;
    schema:additionalType :DepositType ;
.

:vein-fluorite
    a skos:Concept ;
    rdfs:isDefinedBy cs: ;
    skos:broader :vein ;
    skos:definition "Not yet available"@en ;
    skos:inScheme cs: ;
    skos:notation "11.02.07"^^dt:LocalHierarchyKey ;
    skos:prefLabel "Vein fluorite"@en ;
    schema:additionalType :DepositType ;
.

:vein-polymetallic
    a skos:Concept ;
    rdfs:isDefinedBy cs: ;
    skos:broader :vein ;
    skos:definition "Not yet available"@en ;
    skos:inScheme cs: ;
    skos:notation "11.02.08"^^dt:LocalHierarchyKey ;
    skos:prefLabel "Vein polymetallic"@en ;
    schema:additionalType :DepositType ;
.

:vein-replacement-nickel
    a skos:Concept ;
    rdfs:isDefinedBy cs: ;
    skos:broader :vein ;
    skos:definition "Not yet available"@en ;
    skos:inScheme cs: ;
    skos:notation "11.02.01"^^dt:LocalHierarchyKey ;
    skos:prefLabel "Vein ± replacement nickel"@en ;
    schema:additionalType :DepositType ;
.

:vein-tin-polymetallic
    a skos:Concept ;
    rdfs:isDefinedBy cs: ;
    skos:broader :vein ;
    skos:definition "Not yet available"@en ;
    skos:inScheme cs: ;
    skos:notation "11.02.06"^^dt:LocalHierarchyKey ;
    skos:prefLabel "Vein tin polymetallic"@en ;
    schema:additionalType :DepositType ;
.

:vein-tin
    a skos:Concept ;
    rdfs:isDefinedBy cs: ;
    skos:broader :vein ;
    skos:definition "Veins containing mineralised tin."@en ;
    skos:inScheme cs: ;
    skos:notation "11.02.04"^^dt:LocalHierarchyKey ;
    skos:prefLabel "Vein tin"@en ;
    schema:additionalType :DepositType ;
.

:vein-tungsten
    a skos:Concept ;
    rdfs:isDefinedBy cs: ;
    skos:broader :vein ;
    skos:definition "Veins containing mineralised tungsten."@en ;
    skos:inScheme cs: ;
    skos:notation "11.02.05"^^dt:LocalHierarchyKey ;
    skos:prefLabel "Vein tungsten"@en ;
    schema:additionalType :DepositType ;
.

:volcanic-hosted-copper
    a skos:Concept ;
    rdfs:isDefinedBy cs: ;
    skos:broader :volcanic-hosted ;
    skos:definition "Not yet available"@en ;
    skos:inScheme cs: ;
    skos:notation "10.03.01"^^dt:LocalHierarchyKey ;
    skos:prefLabel "Volcanic-hosted copper"@en ;
    schema:additionalType :DepositType ;
.

:volcanogenic-manganese
    a skos:Concept ;
    rdfs:isDefinedBy cs: ;
    skos:broader :volcanogenic ;
    skos:definition "Not yet available"@en ;
    skos:inScheme cs: ;
    skos:notation "10.02.02"^^dt:LocalHierarchyKey ;
    skos:prefLabel "Volcanogenic manganese"@en ;
    schema:additionalType :DepositType ;
.

<https://linked.data.gov.au/org/cgi>
    a schema:Organization ;
    schema:name "Commission for Geoscience Information" ;
    schema:url "https://cgi-iugs.org"^^xsd:anyURI ;
.

<https://linked.dat.gov.au/org/ga>
    a schema:Organization ;
    schema:name "Geoscience Australia" ;
    schema:url "https://www.ga.gov.au"^^xsd:anyURI ;
.

:anorthosite-conduit
    a skos:Concept ;
    rdfs:isDefinedBy cs: ;
    skos:broader :magmatic ;
    skos:definition "Anorthosite rocks formed by the transportation and crystallisation of anorthositic magma to the surface via conduits such as dykes."@en ;
    skos:inScheme cs: ;
    skos:narrower :anorthosite-conduit-nickel-copper-pge ;
    skos:notation "12.13."^^dt:LocalHierarchyKey ;
    skos:prefLabel "Anorthosite conduit"@en ;
    schema:additionalType :DepositGroup ;
.

:anorthosite-massif
    a skos:Concept ;
    rdfs:isDefinedBy cs: ;
    skos:broader :magmatic ;
    skos:definition "Large anorthosite rocks formed by the crystalisation of plagioclase in magma chambers. Massif-type anorthosites are constrained to the Proterozoic and the exact processes by which they form are disputed."@en ;
    skos:inScheme cs: ;
    skos:narrower :anorthosite-massif-titanium ;
    skos:notation "12.12."^^dt:LocalHierarchyKey ;
    skos:prefLabel "Anorthosite massif"@en ;
    schema:additionalType :DepositGroup ;
.

:apatite-intrusion
    a skos:Concept ;
    rdfs:isDefinedBy cs: ;
    skos:broader :magmatic ;
    skos:definition "Massive apatite hydrothermal veins formed from high-temperature hydrothermal fluids sourced from crystallising alkali melts or possibly an enriched mantle or juvenile lower crust."@en ;
    skos:inScheme cs: ;
    skos:narrower :apatite-intrusion-ree ;
    skos:notation "12.05."^^dt:LocalHierarchyKey ;
    skos:prefLabel "Apatite intrusion"@en ;
    schema:additionalType :DepositGroup ;
.

:carlin-type
    a skos:Concept ;
    rdfs:isDefinedBy cs: ;
    skos:broader :magmatic-hydrothermal ;
    skos:definition "Carlin-type deposits are epigeneitc,, disseminated, auriferous pyrite deposits enriched in As, Sb, Hg, Tl that are typically hosted in calcareous sedimentary rocks. They are named after a deposit near Carlin, Nevada."@en ;
    skos:inScheme cs: ;
    skos:narrower :carlin-type-gold ;
    skos:notation "11.04."^^dt:LocalHierarchyKey ;
    skos:prefLabel "Carlin-type"@en ;
    schema:additionalType :DepositGroup ;
.

:clay-basin-evaporative
    a skos:Concept ;
    rdfs:isDefinedBy cs: ;
    skos:broader :basin-evaporative ;
    skos:definition "Not yet available"@en ;
    skos:inScheme cs: ;
    skos:narrower :lacustrine-clay-lithium ;
    skos:notation "04.04."^^dt:LocalHierarchyKey ;
    skos:prefLabel "Clay (basin evaporative)"@en ;
    schema:additionalType :DepositGroup ;
.

:collapse-breccia-pipe
    a skos:Concept ;
    rdfs:isDefinedBy cs: ;
    skos:broader :basin-hydrothermal ;
    skos:definition "Vertical collapse breccia pipes developed in marine platform carbonates deposited in a tectonically stable cratonic environment. Known exclusively in northwestern Arizona, USA."@en ;
    skos:inScheme cs: ;
    skos:narrower :collapse-breccia-pipe-uranium ;
    skos:notation "06.02."^^dt:LocalHierarchyKey ;
    skos:prefLabel "Collapse breccia pipe"@en ;
    schema:additionalType :DepositGroup ;
.

:distal-disseminated
    a skos:Concept ;
    rdfs:isDefinedBy cs: ;
    skos:broader :magmatic-hydrothermal ;
    skos:definition "Carlin-type style deposits which occur on the on the distal edges of magmatic-hydrothermal systems related to upper crustal intrusive complexes."@en ;
    skos:inScheme cs: ;
    skos:narrower :distal-disseminated-ag-au ;
    skos:notation "11.05."^^dt:LocalHierarchyKey ;
    skos:prefLabel "Distal-disseminated"@en ;
    schema:additionalType :DepositGroup ;
.

:erosional
    a skos:Concept ;
    rdfs:isDefinedBy cs: ;
    skos:definition "In erosional environments, gravity-driven turbulent flow of surface water or tidal- and wind-driven wave action concentrate heavy, insoluble, or hard minerals by winnowing away light, soluble, or soft minerals."@en ;
    skos:inScheme cs: ;
    skos:narrower :placer ;
    skos:notation "01.."^^dt:LocalHierarchyKey ;
    skos:prefLabel "Erosional"@en ;
    skos:topConceptOf cs: ;
    schema:additionalType :DepositEnvironment ;
.

:exotic
    a skos:Concept ;
    rdfs:isDefinedBy cs: ;
    skos:broader :infiltrational ;
    skos:definition "Exotic deposits form in conjunction with supergene enrichment, but involve lateral solution movement. Solutions may be transported through paleodrainage systems up to 8 km from the source, producing new mineralisation."@en ;
    skos:inScheme cs: ;
    skos:narrower :exotic-copper ;
    skos:notation "03.01."^^dt:LocalHierarchyKey ;
    skos:prefLabel "Exotic"@en ;
    schema:additionalType :DepositGroup ;
.

:five-element
    a skos:Concept ;
    rdfs:isDefinedBy cs: ;
    skos:broader :basin-hydrothermal ;
    skos:definition "Hydrothermal ore deposits dominated by nickel-copper-arsenides ± native elements. Mineralisation can be veins, stratabound, or replacement of the host rock, and is not restricted to five elements but can include a wide variety of arsenides, sulfarsenides, and/or native elements. "@en ;
    skos:inScheme cs: ;
    skos:narrower :vein-five-element ;
    skos:notation "06.06."^^dt:LocalHierarchyKey ;
    skos:prefLabel "Five-element"@en ;
    schema:additionalType :DepositGroup ;
.

:kimberlite
    a skos:Concept ;
    rdfs:isDefinedBy cs: ;
    skos:broader :magmatic ;
    skos:definition "An ultramafic igneous rock containing at least 35% olivine with one or more of the following in the groundmass; monticellite, phlogiopite, carbonate, serpentine, diopside. It is the primary source of diamonds."@en ;
    skos:inScheme cs: ;
    skos:narrower :kimberlite-diamond ;
    skos:notation "12.06."^^dt:LocalHierarchyKey ;
    skos:prefLabel "Kimberlite"@en ;
    schema:additionalType :DepositGroup ;
.

:komatiite
    a skos:Concept ;
    rdfs:isDefinedBy cs: ;
    skos:broader :magmatic ;
    skos:definition "An ultramafic volcanic rock defined as having crystallised from lava of at least 18% wt% MgO."@en ;
    skos:inScheme cs: ;
    skos:narrower :komatiite-ni-cu-pge ;
    skos:notation "12.07."^^dt:LocalHierarchyKey ;
    skos:prefLabel "Komatiite"@en ;
    schema:additionalType :DepositGroup ;
.

:magnesite
    a skos:Concept ;
    rdfs:isDefinedBy cs: ;
    skos:broader :infiltrational ;
    skos:definition "A magnesium carbonate mineral (MgCO3)."@en ;
    skos:inScheme cs: ;
    skos:narrower :nodular-magnesite ;
    skos:notation "03.04."^^dt:LocalHierarchyKey ;
    skos:prefLabel "Magnesite"@en ;
    schema:additionalType :DepositGroup ;
.

:metamorphic
    a skos:Concept ;
    rdfs:isDefinedBy cs: ;
    skos:definition "In metamorphic environments, ore minerals are produced by metamorphic transformation of precursor minerals that contain valuable commodities."@en ;
    skos:inScheme cs: ;
    skos:narrower :metamorphic-group ;
    skos:notation "08.."^^dt:LocalHierarchyKey ;
    skos:prefLabel "Metamorphic"@en ;
    skos:topConceptOf cs: ;
    schema:additionalType :DepositEnvironment ;
.

:metamorphic-hydrothermal
    a skos:Concept ;
    rdfs:isDefinedBy cs: ;
    skos:definition "In metamorphic hydrothermal environments, elements dissolved in metamorphic (± magmatic) fluids are concentrated by physical and chemical gradients encountered along flow paths."@en ;
    skos:inScheme cs: ;
    skos:narrower :orogenic ;
    skos:notation "07.."^^dt:LocalHierarchyKey ;
    skos:prefLabel "Metamorphic hydrothermal"@en ;
    skos:topConceptOf cs: ;
    schema:additionalType :DepositEnvironment ;
.

:non-sulfide
    a skos:Concept ;
    rdfs:isDefinedBy cs: ;
    skos:broader :basin-hydrothermal ;
    skos:definition "A zinc deposit where ore minerals are largely non-sulfides. They occur mostly in carbonate rocks in a range of geologic environments and form by either supergene or hypogene processes."@en ;
    skos:inScheme cs: ;
    skos:narrower :non-sulfide-zinc-lead-mn ;
    skos:notation "06.05."^^dt:LocalHierarchyKey ;
    skos:prefLabel "Non-sulfide"@en ;
    schema:additionalType :DepositGroup ;
.

:paleochannel
    a skos:Concept ;
    rdfs:isDefinedBy cs: ;
    skos:broader :infiltrational ;
    skos:definition "Remnants of a fluvial channel cut in older rock or sediment and filled by the younger overlying rock or sediment."@en ;
    skos:inScheme cs: ;
    skos:narrower :paleochannel-iron ;
    skos:notation "03.02."^^dt:LocalHierarchyKey ;
    skos:prefLabel "Paleochannel"@en ;
    schema:additionalType :DepositGroup ;
.

:peralkaline-igneous
    a skos:Concept ;
    rdfs:isDefinedBy cs: ;
    skos:broader :magmatic ;
    skos:definition "An igneous rock with a high (Na + K)/Al ratio. Typically enriched in alkali elements, halogens, and rare earth elements."@en ;
    skos:inScheme cs: ;
    skos:narrower :peralkaline-igneous-hfse-ree ;
    skos:notation "12.03."^^dt:LocalHierarchyKey ;
    skos:prefLabel "Peralkaline igneous"@en ;
    schema:additionalType :DepositGroup ;
.

:phosphorite
    a skos:Concept ;
    rdfs:isDefinedBy cs: ;
    skos:broader :basin-chemical ;
    skos:definition "A stratiform or lens-shaped sedimentary rock with a high content of phosphate minerals. Most commonly it is a bedded primary or reworked secondary marine rock composed of microcrystalline carbonate fluorapatite in the form of laminae, pellets, oolites, nodules and skeletal, shell and bone fragments."@en ;
    skos:inScheme cs: ;
    skos:narrower :phosphorite-group ;
    skos:notation "05.02."^^dt:LocalHierarchyKey ;
    skos:prefLabel "Phosphorite"@en ;
    schema:additionalType :DepositGroup ;
.

:skarn-iron
    a skos:Concept ;
    rdfs:isDefinedBy cs: ;
    skos:broader
        :metasomatic-iron ,
        :skarn ;
    skos:definition
        "A skarn deposit containing a significant concentration of iron, formed by the replacement of carbonate rocks through contact metamorphism and metasomatism."@en ;
    skos:inScheme cs: ;
    skos:notation
        "09.02.07"^^dt:LocalHierarchyKey ,
        "11.07.09"^^dt:LocalHierarchyKey ;
    skos:prefLabel "Skarn iron"@en ;
    schema:additionalType :DepositType ;
.

:ultramafic-and-or-mafic-conduit
    a skos:Concept ;
    rdfs:isDefinedBy cs: ;
    skos:broader :magmatic ;
    skos:definition "Conduits underlying ultramafic to mafic large igneous provinces. Conduits are represented by sill complexes that crystallised and cooled at shallow depths."@en ;
    skos:inScheme cs: ;
    skos:narrower :u-m-conduit-ni-cu-pge ;
    skos:notation "12.10."^^dt:LocalHierarchyKey ;
    skos:prefLabel "Ultramafic and (or) mafic conduit"@en ;
    schema:additionalType :DepositGroup ;
.

:volcanic-hosted
    a skos:Concept ;
    rdfs:isDefinedBy cs: ;
    skos:broader :volcanic-basin-hydrothermal ;
    skos:definition "Not yet available"@en ;
    skos:inScheme cs: ;
    skos:narrower :volcanic-hosted-copper ;
    skos:notation "10.03."^^dt:LocalHierarchyKey ;
    skos:prefLabel "Volcanic-hosted"@en ;
    schema:additionalType :DepositType ;
.

:zeolite
    a skos:Concept ;
    rdfs:isDefinedBy cs: ;
    skos:broader :basin-evaporative ;
    skos:definition "A group of white or colourless hydrous aluminosilicate minerals. Zeolites form by reaction between volcanic rock and ash layers and alkali groundwater, and in post-depositional environments in shallow sedimentary basins."@en ;
    skos:inScheme cs: ;
    skos:narrower :lacustrine-zeolite-li-b ;
    skos:notation "04.03."^^dt:LocalHierarchyKey ;
    skos:prefLabel "Zeolite"@en ;
    schema:additionalType :DepositGroup ;
.

:alkali-calcic
    a skos:Concept ;
    rdfs:isDefinedBy cs: ;
    skos:broader :regional-metasomatic ;
    skos:definition "Not yet available"@en ;
    skos:inScheme cs: ;
    skos:narrower
        :albitite-hosted-uranium ,
        :low-fe-alkali-calcic ;
    skos:notation "09.01."^^dt:LocalHierarchyKey ;
    skos:prefLabel "Alkali-calcic"@en ;
    schema:additionalType :DepositGroup ;
.

:carbonatite
    a skos:Concept ;
    rdfs:isDefinedBy cs: ;
    skos:broader :magmatic ;
    skos:definition "An igneous rock composed of at least 50% carbonate minerals."@en ;
    skos:inScheme cs: ;
    skos:narrower
        :carbonatite-nb ,
        :carbonatite-ree ;
    skos:notation "12.02."^^dt:LocalHierarchyKey ;
    skos:prefLabel "Carbonatite"@en ;
    schema:additionalType :DepositGroup ;
.

:intrusion-related
    a skos:Concept ;
    rdfs:isDefinedBy cs: ;
    skos:broader :magmatic-hydrothermal ;
    skos:definition "Not yet available"@en ;
    skos:inScheme cs: ;
    skos:narrower
        :oxidized-intrusion-related-au ,
        :reduced-intrusion-related-au ;
    skos:notation "11.10."^^dt:LocalHierarchyKey ;
    skos:prefLabel "Intrusion-related"@en ;
    schema:additionalType :DepositGroup ;
.

:ioa
    a skos:Concept ;
    rdfs:isDefinedBy cs: ;
    skos:broader :regional-metasomatic ;
    skos:definition "Iron oxide-apatite (IOA) deposits, also known as Kiruna-type deposits. Significant source of iron as well as phosphorus, rare earth elements, vanadium and cobalt. IOA deposits represent the copper poor endmember of iron oxide-copper-gold (IOCG) deposit types. Structurally controlled and are dominantly associated with volcanic and intrusivce rocks of intermediate composition and calc-alkaline affinity. Magnetite is the main consistituent of IOA deposits."@en ;
    skos:inScheme cs: ;
    skos:narrower
        :hematite-dominant-ioa ,
        :magnetite-dominant-ioa ;
    skos:notation "09.04."^^dt:LocalHierarchyKey ;
    skos:prefLabel "IOA"@en ;
    schema:additionalType :DepositGroup ;
.

:iocg
    a skos:Concept ;
    rdfs:isDefinedBy cs: ;
    skos:broader :regional-metasomatic ;
    skos:definition "Iron oxide copper-gold (IOCG) are a group of mineral deposits characterised by magnetite and or hematite breccia zones and veins forming pipe-like and tabular orebodies hosted by subaerial volcanic, sedimentary and intrusive rocks. These deposits vary from apatite-iron (Kiruna type) to polymetallic iron, copper, uranium, gold and rare earth element-bearing (Olympic Dam-type) subtypes."@en ;
    skos:inScheme cs: ;
    skos:narrower
        :hematite-dominant-iocg ,
        :magnetite-dominant-iocg ;
    skos:notation "09.03."^^dt:LocalHierarchyKey ;
    skos:prefLabel "IOCG"@en ;
    schema:additionalType :DepositGroup ;
.

:metamorphic-group
    a skos:Concept ;
    rdfs:isDefinedBy cs: ;
    skos:broader :metamorphic ;
    skos:definition "Not yet available"@en ;
    skos:inScheme cs: ;
    skos:narrower
        :metamorphic-graphite ,
        :metamorphic-kyanite ;
    skos:notation "08.01."^^dt:LocalHierarchyKey ;
    skos:prefLabel "Metamorphic"@en ;
    schema:additionalType :DepositGroup ;
.

:ophiolite
    a skos:Concept ;
    rdfs:isDefinedBy cs: ;
    skos:broader :magmatic ;
    skos:definition "An intact section of oceanic crust and upper mantle thrust on top of the continental lithosphere. A typical section through an ophiolite includes ultramafic rock and serpentinite, gabbro and basalt, and bedded chert or turbidite at the top."@en ;
    skos:inScheme cs: ;
    skos:narrower
        :ophiolite-cr ,
        :ophiolite-ni-cu-pge ;
    skos:notation "12.11."^^dt:LocalHierarchyKey ;
    skos:prefLabel "Ophiolite"@en ;
    schema:additionalType :DepositGroup ;
.

:unconformity-related
    a skos:Concept ;
    rdfs:isDefinedBy cs: ;
    skos:broader :basin-hydrothermal ;
    skos:definition "A deposit associated with a prominent regional unconformity."@en ;
    skos:inScheme cs: ;
    skos:narrower
        :unconformity-related-ree ,
        :unconformity-related-uranium ;
    skos:notation "06.01."^^dt:LocalHierarchyKey ;
    skos:prefLabel "Unconformity-related"@en ;
    schema:additionalType :DepositGroup ;
.

:volcanogenic
    a skos:Concept ;
    rdfs:isDefinedBy cs: ;
    skos:broader :volcanic-basin-hydrothermal ;
    skos:definition "Formed by processes directly connected with volcanism."@en ;
    skos:inScheme cs: ;
    skos:narrower
        :algoma-type-banded-iron-formation ,
        :volcanogenic-manganese ;
    skos:notation "10.02."^^dt:LocalHierarchyKey ;
    skos:prefLabel "Volcanogenic"@en ;
    schema:additionalType :DepositGroup ;
.

:brine
    a skos:Concept ;
    rdfs:isDefinedBy cs: ;
    skos:broader :basin-evaporative ;
    skos:definition "Naturally occurring, unmodified, highly saline pore fluids in subsurface lithologies. Brines are a salt solution and lithium and calcium chloride brines are two common targets."@en ;
    skos:inScheme cs: ;
    skos:narrower
        :lacustrine-brine-lithium ,
        :lacustrine-brine-potash ,
        :marine-brine-potash-mg-li-and-so-on ;
    skos:notation "04.02."^^dt:LocalHierarchyKey ;
    skos:prefLabel "Brine"@en ;
    schema:additionalType :DepositGroup ;
.

:clay-supergene
    a skos:Concept ;
    rdfs:isDefinedBy cs: ;
    skos:broader :supergene ;
    skos:definition "Clays are a group of hydrated alumino-phyllosilicates or material with a particle size of less than 2 μm. Clay deposits can form through various processes including erosion, diagenesis and weathering."@en ;
    skos:inScheme cs: ;
    skos:narrower
        :ion-adsorption-ree ,
        :residual-clay ,
        :underclay-overclay ;
    skos:notation "02.02."^^dt:LocalHierarchyKey ;
    skos:prefLabel "Clay (supergene)"@en ;
    schema:additionalType :DepositGroup ;
.

:greisen
    a skos:Concept ;
    rdfs:isDefinedBy cs: ;
    skos:broader :magmatic-hydrothermal ;
    skos:definition "A pneumatolytically altered grantitic rock composed largely of quartz, mica, and topaz. The mica is usually muscovite or lepidolite. Tourmaline, fluorite, rutile, cassiterite and wolframite are common acessory minerals."@en ;
    skos:inScheme cs: ;
    skos:narrower
        :greisen-be-li ,
        :greisen-sn-w-mo ,
        :greisen-w-mo-bi ;
    skos:notation "11.09."^^dt:LocalHierarchyKey ;
    skos:prefLabel "Greisen"@en ;
    schema:additionalType :DepositGroup ;
.

:iron-formation
    a skos:Concept ;
    rdfs:isDefinedBy cs: ;
    skos:broader :basin-chemical ;
    skos:definition "A chemical sedimatary rock, typically thin-bedded and or/finely laminated, containing at least 15% iron of sedimentary origin, and commonly but not necessarily containing layers of chert."@en ;
    skos:inScheme cs: ;
    skos:narrower
        :lacustrine-iron-formation ,
        :oolitic-iron-formation ,
        :superior-type-banded-iron-formation ;
    skos:notation "05.03."^^dt:LocalHierarchyKey ;
    skos:prefLabel "Iron formation"@en ;
    schema:additionalType :DepositGroup ;
.

:supergene
    a skos:Concept ;
    rdfs:isDefinedBy cs: ;
    skos:definition "In supergene environments, elements released by chemical weathering of soluble minerals are concentrated by chemical gradients associated with the downward percolation of meteoric water in the unsaturated zone."@en ;
    skos:inScheme cs: ;
    skos:narrower
        :clay-supergene ,
        :laterite ,
        :supergene-group ;
    skos:notation "02.."^^dt:LocalHierarchyKey ;
    skos:prefLabel "Supergene"@en ;
    skos:topConceptOf cs: ;
    schema:additionalType :DepositEnvironment ;
.

:volcanic-basin-hydrothermal
    a skos:Concept ;
    rdfs:isDefinedBy cs: ;
    skos:definition "In volcanic basin hydrothermal environments, elements dissolved from volcanic-floored basins by heat-driven convection of seawater (± magmatic fluid) are concentrated by steep chemical and thermal gradients near seafloor vents."@en ;
    skos:inScheme cs: ;
    skos:narrower
        :volcanic-hosted ,
        :volcanogenic ,
        :volcanogenic-massive-sulfide-vms ;
    skos:notation "10.."^^dt:LocalHierarchyKey ;
    skos:prefLabel "Volcanic basin hydrothermal"@en ;
    skos:topConceptOf cs: ;
    schema:additionalType :DepositEnvironment ;
.

:basin-chemical
    a skos:Concept ;
    rdfs:isDefinedBy cs: ;
    skos:definition "In basin chemical environments, elements dissolved in freshwater or seawater precipitate at redox fronts in sedimentary basins."@en ;
    skos:inScheme cs: ;
    skos:narrower
        :black-shale ,
        :iron-formation ,
        :manganese ,
        :phosphorite ;
    skos:notation "05.."^^dt:LocalHierarchyKey ;
    skos:prefLabel "Basin chemical"@en ;
    skos:topConceptOf cs: ;
    schema:additionalType :DepositEnvironment ;
.

:basin-evaporative
    a skos:Concept ;
    rdfs:isDefinedBy cs: ;
    skos:definition "In basin evaporative environments, elements present in closed lacustrine or silled marine basins are concentrated by evaporation in arid to hyperarid climatic zones until they precipitate from brines."@en ;
    skos:inScheme cs: ;
    skos:narrower
        :brine ,
        :clay-basin-evaporative ,
        :evaporite ,
        :zeolite ;
    skos:notation "04.."^^dt:LocalHierarchyKey ;
    skos:prefLabel "Basin evaporative"@en ;
    skos:topConceptOf cs: ;
    schema:additionalType :DepositEnvironment ;
.

:black-shale
    a skos:Concept ;
    rdfs:isDefinedBy cs: ;
    skos:broader :basin-chemical ;
    skos:definition "A dark, thinly laminated carbonaceous shale, exceptionally rich in organic matter (5% or more carbon content) and sulphide and commonly containing unusual concentrations of uranium, vanadium, copper, or nickel; also composed of manganese oxides."@en ;
    skos:inScheme cs: ;
    skos:narrower
        :black-shale-gold ,
        :black-shale-nickel-mo-pge ,
        :black-shale-uranium ,
        :black-shale-vanadium-mo-ni ;
    skos:notation "05.01."^^dt:LocalHierarchyKey ;
    skos:prefLabel "Black shale"@en ;
    schema:additionalType :DepositGroup ;
.

:breccia-pipe
    a skos:Concept ;
    rdfs:isDefinedBy cs: ;
    skos:broader :magmatic-hydrothermal ;
    skos:definition "A cylindrical chimney filled with breccia fragments of the country rock. Often found in mineralied epithermal systems and associated with prophyry-type mineral deposits."@en ;
    skos:inScheme cs: ;
    skos:narrower
        :breccia-pipe-copper ,
        :breccia-pipe-gold ,
        :breccia-pipe-molybdenum ,
        :breccia-pipe-ree ;
    skos:notation "11.03."^^dt:LocalHierarchyKey ;
    skos:prefLabel "Breccia pipe"@en ;
    schema:additionalType :DepositGroup ;
.

:infiltrational
    a skos:Concept ;
    rdfs:isDefinedBy cs: ;
    skos:definition "In infiltrational environments, elements dissolved from soluble minerals by gravity-driven flow of oxidized meteoric groundwater are concentrated by chemical gradients encountered in aquifers."@en ;
    skos:inScheme cs: ;
    skos:narrower
        :exotic ,
        :magnesite ,
        :paleochannel ,
        :uranium ;
    skos:notation "03.."^^dt:LocalHierarchyKey ;
    skos:prefLabel "Infiltrational"@en ;
    skos:topConceptOf cs: ;
    schema:additionalType :DepositEnvironment ;
.

:pegmatite
    a skos:Concept ;
    rdfs:isDefinedBy cs: ;
    skos:broader :magmatic ;
    skos:definition "A very coarse grained intrusive igneous rock, usually found as irregular dykes, lenses or veins. Most grains are one cm or more in diameter. Pegmatites can be any igneous composition, though generally are granitic. Pegmatites represent the last and most hydrous portion of a magma to crystallise and hence contain high concentrations of minerals or elements present only in trace amounts in granitic rocks."@en ;
    skos:inScheme cs: ;
    skos:narrower
        :abyssal-pegmatite-ree ,
        :lct-pegmatite ,
        :nyf-pegmatite ,
        :simple-pegmatite ;
    skos:notation "12.01."^^dt:LocalHierarchyKey ;
    skos:prefLabel "Pegmatite"@en ;
    schema:additionalType :DepositGroup ;
.

:regional-metasomatic
    a skos:Concept ;
    rdfs:isDefinedBy cs: ;
    skos:definition "In regional metasomatic environments, elements dissolved in magmatic, metamorphic, or basinal brines are concentrated by chemical and thermal gradients encountered along heat-, tectonic-, and gravity-driven flow paths."@en ;
    skos:inScheme cs: ;
    skos:narrower
        :alkali-calcic ,
        :ioa ,
        :iocg ,
        :metasomatic-iron ;
    skos:notation "09.."^^dt:LocalHierarchyKey ;
    skos:prefLabel "Regional metasomatic"@en ;
    skos:topConceptOf cs: ;
    schema:additionalType :DepositEnvironment ;
.

:ultramafic-and-or-mafic-intrusion
    a skos:Concept ;
    rdfs:isDefinedBy cs: ;
    skos:broader :magmatic ;
    skos:definition "An intrusion with a mafic to ultramafic composition."@en ;
    skos:inScheme cs: ;
    skos:narrower
        :arc-u-m-intrusion-nickel-copper-pge ,
        :arc-u-m-intrusion-titanium-vanadium ,
        :impact-u-m-intrusion-nickel-copper-pge ,
        :u-m-intrusion-nickel-copper-pge ;
    skos:notation "12.09."^^dt:LocalHierarchyKey ;
    skos:prefLabel "Ultramafic and (or) mafic intrusion"@en ;
    schema:additionalType :DepositGroup ;
.

:ultramafic-and-or-mafic-layered-intrusion
    a skos:Concept ;
    rdfs:isDefinedBy cs: ;
    skos:broader :magmatic ;
    skos:definition "Layered mafic to ultramafic intrusions formed by crystallisation of magma deep in the crust. Intrusions are primarily cumulates with sheet- to dyke-like shapes."@en ;
    skos:inScheme cs: ;
    skos:narrower
        :u-m-layered-intrusion-chromium ,
        :u-m-layered-intrusion-iron-titanium-vanadium ,
        :u-m-layered-intrusion-nickel-copper-pge ,
        :u-m-layered-intrusion-pge ;
    skos:notation "12.08."^^dt:LocalHierarchyKey ;
    skos:prefLabel "Ultramafic and (or) mafic-layered intrusion"@en ;
    schema:additionalType :DepositGroup ;
.

:uranium
    a skos:Concept ;
    rdfs:isDefinedBy cs: ;
    skos:broader :infiltrational ;
    skos:definition "A uranium deposit."@en ;
    skos:inScheme cs: ;
    skos:narrower
        :calcrete-uranium ,
        :carbonate-uranium ,
        :coal-peat-bog-uranium ,
        :sandstone-uranium ;
    skos:notation "03.03."^^dt:LocalHierarchyKey ;
    skos:prefLabel "Uranium"@en ;
    schema:additionalType :DepositGroup ;
.

:laterite
    a skos:Concept ;
    rdfs:isDefinedBy cs: ;
    skos:broader :supergene ;
    skos:definition "A soil type rich in iron and or aluminum oxides formed by extensive weathering of the parent rock. Laterites form in humid tropical to sub-tropical regions."@en ;
    skos:inScheme cs: ;
    skos:narrower
        :bauxite ,
        :carbonatite-laterite-ree ,
        :karst-bauxite ,
        :laterite-magnesite ,
        :laterite-nickel ;
    skos:notation "02.01."^^dt:LocalHierarchyKey ;
    skos:prefLabel "Laterite"@en ;
    schema:additionalType :DepositGroup ;
.

:manganese
    a skos:Concept ;
    rdfs:isDefinedBy cs: ;
    skos:broader :basin-chemical ;
    skos:definition "The element manganese (Mn) is a silvery white, hard and brittle naturally occuring metal."@en ;
    skos:inScheme cs: ;
    skos:narrower
        :crust-manganese ,
        :lacustrine-manganese ,
        :nodule-manganese ,
        :sedimentary-manganese ,
        :superior-type-banded-manganese ;
    skos:notation "05.04."^^dt:LocalHierarchyKey ;
    skos:prefLabel "Manganese"@en ;
    schema:additionalType :DepositGroup ;
.

:mississippi-valley-type-mvt
    a skos:Concept ;
    rdfs:isDefinedBy cs: ;
    skos:broader :basin-hydrothermal ;
    skos:definition "An epigenetic lead and zinc deposit formed by replacement of dolostone and limestone by sphalerite, galena, pyrite, and marcasite; barite may be present in minor to trace amounts and fluorite is rare. MVT deposits form in platform carbonate sequences commonly at the flanks of basins or in foreland thrust belts, where basinal brines source metals and sulfur from the crust and are focused by faults, fractures, collapse breccias, and lithological transitions into the overlying carbonate sequences."@en ;
    skos:inScheme cs: ;
    skos:narrower
        :mvt-barite ,
        :mvt-fluorspar ,
        :mvt-strontium ,
        :mvt-zinc-lead ,
        :sandstone-hosted-zinc-lead ;
    skos:notation "06.04."^^dt:LocalHierarchyKey ;
    skos:prefLabel "Mississippi Valley-type (MVT)"@en ;
    schema:additionalType :DepositGroup ;
.

:volcanogenic-massive-sulfide-vms
    a skos:Concept ;
    rdfs:isDefinedBy cs: ;
    skos:broader :volcanic-basin-hydrothermal ;
    skos:definition "Copper-zinc-lead-Au-Ag deposits formed at or near the seafloor where circulating hydrothermal fluids driven by magmatic heat are quenched through mixing with bottom waters or porewaters. Massive sulfide lenses form in a variety of shapes and sizes; they may be podlike or sheetlike and are generally stratiform."@en ;
    skos:inScheme cs: ;
    skos:narrower
        :bimodal-felsic-vms ,
        :bimodal-mafic-vms ,
        :felsic-siliciclastic-vms ,
        :mafic-siliciclastic-vms ,
        :mafic-ultramafic-vms ;
    skos:notation "10.01."^^dt:LocalHierarchyKey ;
    skos:prefLabel "Volcanogenic massive sulfide (VMS)"@en ;
    schema:additionalType :DepositGroup ;
.

:basin-hydrothermal
    a skos:Concept ;
    rdfs:isDefinedBy cs: ;
    skos:definition "In basin hydrothermal environments, elements are dissolved from minerals by gravity-driven and (or) heat-driven flow of brines produced by the evaporation of seawater or dissolution of minerals; elements are concentrated by chemical gradients encountered in basin aquifers or at the seawater-sediment interface."@en ;
    skos:inScheme cs: ;
    skos:narrower
        :collapse-breccia-pipe ,
        :five-element ,
        :mississippi-valley-type-mvt ,
        :non-sulfide ,
        :sediment-hosted ,
        :unconformity-related ;
    skos:notation "06.."^^dt:LocalHierarchyKey ;
    skos:prefLabel "Basin hydrothermal"@en ;
    skos:topConceptOf cs: ;
    schema:additionalType :DepositEnvironment ;
.

:sediment-hosted
    a skos:Concept ;
    rdfs:isDefinedBy cs: ;
    skos:broader :basin-hydrothermal ;
    skos:definition "Sediment-hosted deposits can be divided into two major subtypes. The first subtype is clastic-dominated lead-zinc ores, which are hosted in shale, sandstone, siltstone, or mixed clastic rocks, or occur as carbonate replacement, within a clastic-dominated sedimentary rock sequence. This subtype includes deposits that have been traditionally referred to as sedimentary exhalative (SEDEX) deposits. The second subtype of sediment-hosted Pb-Zn deposits is the Mississippi Valley-type that occurs in platform carbonate sequences, typically in passive-margin tectonic settings."@en ;
    skos:inScheme cs: ;
    skos:narrower
        :irish-type-sediment-hosted-zinc-lead ,
        :kipushi-type-sediment-hosted-copper-zinc-lead ,
        :sediment-hosted-copper-co ,
        :siliciclastic-carbonate-zinc-lead ,
        :siliciclastic-mafic-barite ,
        :siliciclastic-mafic-zinc-lead ;
    skos:notation "06.03."^^dt:LocalHierarchyKey ;
    skos:prefLabel "Sediment-hosted"@en ;
    schema:additionalType :DepositGroup ;
.

:epithermal
    a skos:Concept ;
    rdfs:isDefinedBy cs: ;
    skos:broader :magmatic-hydrothermal ;
    skos:definition "Deposits formed in relatively near-surface magmatic hydrothermal environment associated with volcanic rocks that overlie cogenetic intrusive rocks. Generally accepted to form at temperatures <300 degrees celcius and depths of less than 1500m. Epithermal mineralisation occurs in three types, low-sulfidation, intermediate-sulfidation and high-sulfidation."@en ;
    skos:inScheme cs: ;
    skos:narrower
        :alkalic-epithermal-gold-ag ,
        :epithermal-beryllium ,
        :epithermal-mercury ,
        :epithermal-uranium ,
        :high-sulfidation-epithermal-silver-gold-cu ,
        :intermediate-sulfidation-epithermal-silver-gold-zn-pb-cu-sn-mn ,
        :low-sulfidation-epithermal-gold-silver ;
    skos:notation "11.01."^^dt:LocalHierarchyKey ;
    skos:prefLabel "Epithermal"@en ;
    schema:additionalType :DepositGroup ;
.

:metasomatic-iron
    a skos:Concept ;
    rdfs:isDefinedBy cs: ;
    skos:broader :regional-metasomatic ;
    skos:definition "Not yet available"@en ;
    skos:inScheme cs: ;
    skos:narrower
        :ferroan-carbonate-polymetallic ,
        :iron-oxide-gold ,
        :iron-oxide-polymetallic ,
        :iron-oxide-uranium ,
        :iron-silicate-polymetallic ,
        :iron-sulfide-polymetallic ,
        :skarn-iron ;
    skos:notation "09.02."^^dt:LocalHierarchyKey ;
    skos:prefLabel "Metasomatic iron"@en ;
    schema:additionalType :DepositGroup ;
.

:porphyry
    a skos:Concept ;
    rdfs:isDefinedBy cs: ;
    skos:broader :magmatic-hydrothermal ;
    skos:definition "An igneous rock of any composition that contains conspicuous phenocrysts in a fine-grained groundmass; a porphyritic igneous rock."@en ;
    skos:inScheme cs: ;
    skos:narrower
        :climax-type-porphyry-molybdenum ,
        :low-fluorine-porphyry-molybdenum ,
        :porphyry-gold-copper ,
        :porphyry-copper-gold ,
        :porphyry-copper-molybdenum ,
        :porphyry-tin ,
        :porphyry-tungsten ;
    skos:notation "11.08."^^dt:LocalHierarchyKey ;
    skos:prefLabel "Porphyry"@en ;
    schema:additionalType :DepositGroup ;
.

:orogenic
    a skos:Concept ;
    rdfs:isDefinedBy cs: ;
    skos:broader :metamorphic-hydrothermal ;
    skos:definition "Deposits of mineralized quartz veins hosted in deformed metamorphic terranes in collisional orogenic belts, divided into epizonal, mesozonal, and hypozonal deposits based on depth and temperature of formation."@en ;
    skos:inScheme cs: ;
    skos:narrower
        :epizonal-orogenic-antimony-gold ,
        :epizonal-orogenic-gold ,
        :epizonal-orogenic-mercury ,
        :hypozonal-orogenic-gold ,
        :mesozonal-orogenic-gold ,
        :orogenic-copper-gold ,
        :orogenic-graphite ,
        :orogenic-silver-lead-zinc-copper-antimony ;
    skos:notation "07.01."^^dt:LocalHierarchyKey ;
    skos:prefLabel "Orogenic"@en ;
    schema:additionalType :DepositGroup ;
.

:replacement
    a skos:Concept ;
    rdfs:isDefinedBy cs: ;
    skos:broader :magmatic-hydrothermal ;
    skos:definition "A change in mineral or composition of a mineral or mineral aggregate presumably by diffusion of new material in and old material out."@en ;
    skos:inScheme cs: ;
    skos:narrower
        :replacement-gold-silver ,
        :replacement-copper ,
        :replacement-fluorite ,
        :replacement-magnesium ,
        :replacement-manganese ,
        :replacement-polymetallic ,
        :replacement-tin ,
        :replacement-zinc-lead ;
    skos:notation "11.06."^^dt:LocalHierarchyKey ;
    skos:prefLabel "Replacement"@en ;
    schema:additionalType :DepositGroup ;
.

:vein
    a skos:Concept ;
    rdfs:isDefinedBy cs: ;
    skos:broader :magmatic-hydrothermal ;
    skos:definition "Any fracture that contains mineralised material. Veins can display either crack-normal extension or shear displacement couple with crack normal extension."@en ;
    skos:inScheme cs: ;
    skos:narrower
        :vein-cobalt-ni ,
        :vein-copper ,
        :vein-fluorite ,
        :vein-polymetallic ,
        :vein-replacement-nickel ,
        :vein-tin-polymetallic ,
        :vein-tin ,
        :vein-tungsten ;
    skos:notation "11.02."^^dt:LocalHierarchyKey ;
    skos:prefLabel "Vein"@en ;
    schema:additionalType :DepositGroup ;
.

:skarn
    a skos:Concept ;
    rdfs:isDefinedBy cs: ;
    skos:broader :magmatic-hydrothermal ;
    skos:definition "A mining term for silicate gangue (amphibole, pyroxene, garnet etc.) of certain iron-ore and sulphide deposits of Archaean age, particularly those that have replaced limestone and dolomite. Its meaning has been generally expanded to include calcium-bearing silicates of any geologic age, derived from nearly pure limestone and dolomite with the introduction of large amounts of Si, Al, Fe, Mg."@en ;
    skos:inScheme cs: ;
    skos:narrower
        :skarn-gold-copper-tungsten ,
        :skarn-beryllium-fluorite ,
        :skarn-copper ,
        :skarn-iron ,
        :skarn-molybdenum ,
        :skarn-tin-copper-mo ,
        :skarn-uranium-ree ,
        :skarn-tungsten-mo ,
        :skarn-zinc-lead-silver ;
    skos:notation "11.07."^^dt:LocalHierarchyKey ;
    skos:prefLabel "Skarn"@en ;
    schema:additionalType :DepositGroup ;
.

:supergene-group
    a skos:Concept ;
    rdfs:isDefinedBy cs: ;
    skos:broader :supergene ;
    skos:definition "The supergene group"@en ;
    skos:inScheme cs: ;
    skos:narrower
        :supergene-copper ,
        :supergene-gold ,
        :supergene-iron ,
        :supergene-lead ,
        :supergene-manganese ,
        :supergene-silver ,
        :supergene-uranium ,
        :supergene-vanadium ,
        :supergene-zinc ;
    skos:notation "02.03."^^dt:LocalHierarchyKey ;
    skos:prefLabel "Supergene"@en ;
    schema:additionalType :DepositGroup ;
.

:magmatic-hydrothermal
    a skos:Concept ;
    rdfs:isDefinedBy cs: ;
    skos:definition "In magmatic hydrothermal environments, elements dissolved in magmatic fluids, brines, and vapors, or in heated external fluids, are concentrated by the steep chemical and thermal gradients around volcano-plutonic centers."@en ;
    skos:inScheme cs: ;
    skos:narrower
        :breccia-pipe ,
        :carlin-type ,
        :distal-disseminated ,
        :epithermal ,
        :greisen ,
        :intrusion-related ,
        :porphyry ,
        :replacement ,
        :skarn ,
        :vein ;
    skos:notation "11.."^^dt:LocalHierarchyKey ;
    skos:prefLabel "Magmatic hydrothermal"@en ;
    skos:topConceptOf cs: ;
    schema:additionalType :DepositEnvironment ;
.

:DepositEnvironment
    a owl:Class ;
    schema:name "Mineral Deposit Environment" ;
.

:evaporite
    a skos:Concept ;
    rdfs:isDefinedBy cs: ;
    skos:broader :basin-evaporative ;
    skos:definition "Sediments formed by solar-driven concentration of a surface or near-surface brine. These can form in marine and lacustrine settings."@en ;
    skos:inScheme cs: ;
    skos:narrower
        :lacustrine-evaporite-borate ,
        :lacustrine-evaporite-carnallite-bischofite ,
        :lacustrine-evaporite-magnesite ,
        :lacustrine-evaporite-nitrate ,
        :lacustrine-evaporite-potash ,
        :lacustrine-evaporite-salt ,
        :lacustrine-evaporite-trona ,
        :marine-evaporite-gypsum ,
        :marine-evaporite-magnesite ,
        :marine-evaporite-potash ,
        :marine-evaporite-salt ;
    skos:notation "04.01."^^dt:LocalHierarchyKey ;
    skos:prefLabel "Evaporite"@en ;
    schema:additionalType :DepositGroup ;
.

:magmatic
    a skos:Concept ;
    rdfs:isDefinedBy cs: ;
    skos:definition "In magmatic environments, ore minerals crystallize directly from igneous melts, including immiscible silicate, carbonate, sulfide, or other melts."@en ;
    skos:inScheme cs: ;
    skos:narrower
        :anorthosite-conduit ,
        :anorthosite-massif ,
        :apatite-intrusion ,
        :apatite-nepheline-titanite-intrusion ,
        :carbonatite ,
        :kimberlite ,
        :komatiite ,
        :ophiolite ,
        :pegmatite ,
        :peralkaline-igneous ,
        :ultramafic-and-or-mafic-conduit ,
        :ultramafic-and-or-mafic-intrusion ,
        :ultramafic-and-or-mafic-layered-intrusion ;
    skos:notation "12.."^^dt:LocalHierarchyKey ;
    skos:prefLabel "Magmatic"@en ;
    skos:topConceptOf cs: ;
    schema:additionalType :DepositEnvironment ;
.

:placer
    a skos:Concept ;
    rdfs:isDefinedBy cs: ;
    skos:broader :erosional ;
    skos:definition "A surficial mineral deposit formed by mechanical concentration of mineral particles from weathered material. The mineral is usually a heavy metal or mineral such as gold."@en ;
    skos:inScheme cs: ;
    skos:narrower
        :fluvial-placer-diamond ,
        :fluvial-placer-garnet ,
        :fluvial-placer-gemstones ,
        :fluvial-placer-gold ,
        :fluvial-placer-niobium-tantalum ,
        :fluvial-placer-pge ,
        :fluvial-placer-ree ,
        :fluvial-placer-tin ,
        :fluvial-placer-tungsten ,
        :heavy-mineral-sands ,
        :paleoplacer-gold-uranium ,
        :paleoplacer-heavy-mineral-sands ,
        :paleoplacer-tin ,
        :residual-placer-lead ,
        :residual-placer-tin ,
        :shoreline-placer-gold ;
    skos:notation "01.01."^^dt:LocalHierarchyKey ;
    skos:prefLabel "Placer"@en ;
    schema:additionalType :DepositGroup ;
.

:DepositGroup
    a owl:Class ;
    schema:name "Mineral Deposit Group" ;
.

:DepositType
    a owl:Class ;
    schema:name "Mineral Deposit Type" ;
.

cs:
    a skos:ConceptScheme ;
    skos:definition "Minerals and groups of them from the Critical Mineral Mapping Initiative project"@en ;
    skos:hasTopConcept
        :basin-chemical ,
        :basin-evaporative ,
        :basin-hydrothermal ,
        :erosional ,
        :infiltrational ,
        :magmatic ,
        :magmatic-hydrothermal ,
        :metamorphic ,
        :metamorphic-hydrothermal ,
        :regional-metasomatic ,
        :supergene ,
        :volcanic-basin-hydrothermal ;
    skos:historyNote "Taken from Geoscience Australia's internal database, November 2023" ;
    skos:prefLabel "Mineral Deposit Model"@en ;
    schema:copyrightNotice "(c) Commission for Geoscience Information, 2023" ;
    schema:creator <https://linked.dat.gov.au/org/ga> ;
    schema:dateCreated "2022-06-30"^^xsd:date ;
    schema:dateModified "2023-11-11"^^xsd:date ;
    schema:license <https://purl.org/NET/rdflicense/cc-by4.0> ;
    schema:publisher <https://linked.data.gov.au/org/cgi> ;
    schema:citation "https://earthresourceml.org"^^xsd:anyURI ;
    schema:status astatus:experimental ;
.

:carbonatite-nb
    a skos:Concept ;
    rdfs:isDefinedBy cs: ;
    skos:definition "Not yet given"@en ;
    skos:historyNote "Added by NJC in 2025-09 to fix vocab validity. Needs scientific review" ;
    skos:inScheme cs: ;
    skos:notation "0"^^dt:LocalHierarchyKey ;
    skos:prefLabel "carbonatite-nb"@en ;
.

:u-m-conduit-ni-cu-pge
    a skos:Concept ;
    rdfs:isDefinedBy cs: ;
    skos:definition "Not yet given"@en ;
    skos:historyNote "Added by NJC in 2025-09 to fix vocab validity. Needs scientific review" ;
    skos:inScheme cs: ;
    skos:notation "0"^^dt:LocalHierarchyKey ;
    skos:prefLabel "u-m-conduit-ni-cu-pge"@en ;
.

:komatiite-ni-cu-pge
    a skos:Concept ;
    rdfs:isDefinedBy cs: ;
    skos:definition "Not yet given"@en ;
    skos:historyNote "Added by NJC in 2025-09 to fix vocab validity. Needs scientific review" ;
    skos:inScheme cs: ;
    skos:notation "0"^^dt:LocalHierarchyKey ;
    skos:prefLabel "komatiite-ni-cu-pge"@en ;
.

:ophiolite-cr
    a skos:Concept ;
    rdfs:isDefinedBy cs: ;
    skos:definition "Not yet given"@en ;
    skos:historyNote "Added by NJC in 2025-09 to fix vocab validity. Needs scientific review" ;
    skos:inScheme cs: ;
    skos:notation "0"^^dt:LocalHierarchyKey ;
    skos:prefLabel "ophiolite-cr"@en ;
.

:ophiolite-ni-cu-pge
    a skos:Concept ;
    rdfs:isDefinedBy cs: ;
    skos:definition "Not yet given"@en ;
    skos:historyNote "Added by NJC in 2025-09 to fix vocab validity. Needs scientific review" ;
    skos:inScheme cs: ;
    skos:notation "0"^^dt:LocalHierarchyKey ;
    skos:prefLabel "ophiolite-ni-cu-pge"@en ;
.

:distal-disseminated-ag-au
    a skos:Concept ;
    rdfs:isDefinedBy cs: ;
    skos:definition "Not yet given"@en ;
    skos:historyNote "Added by NJC in 2025-09 to fix vocab validity. Needs scientific review" ;
    skos:inScheme cs: ;
    skos:notation "0"^^dt:LocalHierarchyKey ;
    skos:prefLabel "distal-disseminated-ag-au"@en ;
.

:greisen-w-mo-bi
    a skos:Concept ;
    rdfs:isDefinedBy cs: ;
    skos:definition "Not yet given"@en ;
    skos:historyNote "Added by NJC in 2025-09 to fix vocab validity. Needs scientific review" ;
    skos:inScheme cs: ;
    skos:notation "0"^^dt:LocalHierarchyKey ;
    skos:prefLabel "greisen-w-mo-bi"@en ;
.

:greisen-be-li
    a skos:Concept ;
    rdfs:isDefinedBy cs: ;
    skos:definition "Not yet given"@en ;
    skos:historyNote "Added by NJC in 2025-09 to fix vocab validity. Needs scientific review" ;
    skos:inScheme cs: ;
    skos:notation "0"^^dt:LocalHierarchyKey ;
    skos:prefLabel "greisen-be-li"@en ;
.

:greisen-sn-w-mo
    a skos:Concept ;
    rdfs:isDefinedBy cs: ;
    skos:definition "Not yet given"@en ;
    skos:historyNote "Added by NJC in 2025-09 to fix vocab validity. Needs scientific review" ;
    skos:inScheme cs: ;
    skos:notation "0"^^dt:LocalHierarchyKey ;
    skos:prefLabel "greisen-sn-w-mo"@en ;
.

:oxidized-intrusion-related-au
    a skos:Concept ;
    rdfs:isDefinedBy cs: ;
    skos:definition "Not yet given"@en ;
    skos:historyNote "Added by NJC in 2025-09 to fix vocab validity. Needs scientific review" ;
    skos:inScheme cs: ;
    skos:notation "0"^^dt:LocalHierarchyKey ;
    skos:prefLabel "oxidized-intrusion-related-au"@en ;
.

:reduced-intrusion-related-au
    a skos:Concept ;
    rdfs:isDefinedBy cs: ;
    skos:definition "Not yet given"@en ;
    skos:historyNote "Added by NJC in 2025-09 to fix vocab validity. Needs scientific review" ;
    skos:inScheme cs: ;
    skos:notation "0"^^dt:LocalHierarchyKey ;
    skos:prefLabel "reduced-intrusion-related-au"@en ;
.

:low-fe-alkali-calcic
    a skos:Concept ;
    rdfs:isDefinedBy cs: ;
    skos:definition "Not yet given"@en ;
    skos:historyNote "Added by NJC in 2025-09 to fix vocab validity. Needs scientific review" ;
    skos:inScheme cs: ;
    skos:notation "0"^^dt:LocalHierarchyKey ;
    skos:prefLabel "low-fe-alkali-calcic"@en ;
.

<http://resource.geosciml.org/classifier/cgi/mineral-deposit-model>
    a skos:Collection ;
    schema:citation "The original vocabulary - all its concepts"@en ;
    skos:changeNote "2025-09-15 NJC created to list all vocab Concepts"@en ;
    skos:definition "All the Concepts in this vocabulary"@en ;
    skos:member
        :abyssal-pegmatite-ree ,
        :albitite-hosted-uranium ,
        :algoma-type-banded-iron-formation ,
        :alkali-calcic ,
        :alkalic-epithermal-gold-ag ,
        :anorthosite-conduit ,
        :anorthosite-conduit-nickel-copper-pge ,
        :anorthosite-massif ,
        :anorthosite-massif-titanium ,
        :apatite-intrusion ,
        :apatite-intrusion-ree ,
        :apatite-nepheline-titanite-intrusion ,
        :arc-u-m-intrusion-nickel-copper-pge ,
        :arc-u-m-intrusion-titanium-vanadium ,
        :basin-chemical ,
        :basin-evaporative ,
        :basin-hydrothermal ,
        :bauxite ,
        :bimodal-felsic-vms ,
        :bimodal-mafic-vms ,
        :black-shale ,
        :black-shale-gold ,
        :black-shale-nickel-mo-pge ,
        :black-shale-uranium ,
        :black-shale-vanadium-mo-ni ,
        :breccia-pipe ,
        :breccia-pipe-copper ,
        :breccia-pipe-gold ,
        :breccia-pipe-molybdenum ,
        :breccia-pipe-ree ,
        :brine ,
        :calcrete-uranium ,
        :carbonate-uranium ,
        :carbonatite ,
        :carbonatite-laterite-ree ,
        :carbonatite-nb ,
        :carbonatite-niobium ,
        :carbonatite-ree ,
        :carlin-type ,
        :carlin-type-gold ,
        :clay-basin-evaporative ,
        :clay-supergene ,
        :climax-type-porphyry-molybdenum ,
        :coal-peat-bog-uranium ,
        :collapse-breccia-pipe ,
        :collapse-breccia-pipe-uranium ,
        :crust-manganese ,
        :distal-disseminated ,
        :distal-disseminated-ag-au ,
        :distal-disseminated-silver-gold ,
        :epithermal ,
        :epithermal-beryllium ,
        :epithermal-mercury ,
        :epithermal-uranium ,
        :epizonal-orogenic-antimony-gold ,
        :epizonal-orogenic-gold ,
        :epizonal-orogenic-mercury ,
        :erosional ,
        :evaporite ,
        :exotic ,
        :exotic-copper ,
        :felsic-siliciclastic-vms ,
        :ferroan-carbonate-polymetallic ,
        :five-element ,
        :fluvial-placer-diamond ,
        :fluvial-placer-garnet ,
        :fluvial-placer-gemstones ,
        :fluvial-placer-gold ,
        :fluvial-placer-niobium-tantalum ,
        :fluvial-placer-pge ,
        :fluvial-placer-ree ,
        :fluvial-placer-tin ,
        :fluvial-placer-tungsten ,
        :greisen ,
        :greisen-be-li ,
        :greisen-beryllium-li ,
        :greisen-sn-w-mo ,
        :greisen-tin-w-mo ,
        :greisen-tungsten-molybdenum-bi ,
        :greisen-w-mo-bi ,
        :heavy-mineral-sands ,
        :hematite-dominant-ioa ,
        :hematite-dominant-iocg ,
        :high-sulfidation-epithermal-silver-gold-cu ,
        :hypozonal-orogenic-gold ,
        :impact-u-m-intrusion-nickel-copper-pge ,
        :infiltrational ,
        :intermediate-sulfidation-epithermal-silver-gold-zn-pb-cu-sn-mn ,
        :intrusion-related ,
        :ioa ,
        :iocg ,
        :ion-adsorption-ree ,
        :irish-type-sediment-hosted-zinc-lead ,
        :iron-formation ,
        :iron-oxide-gold ,
        :iron-oxide-polymetallic ,
        :iron-oxide-uranium ,
        :iron-silicate-polymetallic ,
        :iron-sulfide-polymetallic ,
        :karst-bauxite ,
        :kimberlite ,
        :kimberlite-diamond ,
        :kipushi-type-sediment-hosted-copper-zinc-lead ,
        :komatiite ,
        :komatiite-ni-cu-pge ,
        :komatiite-nickel-copper-pge ,
        :lacustrine-brine-lithium ,
        :lacustrine-brine-potash ,
        :lacustrine-clay-lithium ,
        :lacustrine-evaporite-borate ,
        :lacustrine-evaporite-carnallite-bischofite ,
        :lacustrine-evaporite-magnesite ,
        :lacustrine-evaporite-nitrate ,
        :lacustrine-evaporite-potash ,
        :lacustrine-evaporite-salt ,
        :lacustrine-evaporite-trona ,
        :lacustrine-iron-formation ,
        :lacustrine-manganese ,
        :lacustrine-zeolite-li-b ,
        :laterite ,
        :laterite-magnesite ,
        :laterite-nickel ,
        :lct-pegmatite ,
        :low-fe-alkali-calcic ,
        :low-fluorine-porphyry-molybdenum ,
        :low-iron-alkali-calcic ,
        :low-sulfidation-epithermal-gold-silver ,
        :mafic-siliciclastic-vms ,
        :mafic-ultramafic-vms ,
        :magmatic ,
        :magmatic-hydrothermal ,
        :magnesite ,
        :magnetite-dominant-ioa ,
        :magnetite-dominant-iocg ,
        :manganese ,
        :marine-brine-potash-mg-li-and-so-on ,
        :marine-evaporite-gypsum ,
        :marine-evaporite-magnesite ,
        :marine-evaporite-potash ,
        :marine-evaporite-salt ,
        :mesozonal-orogenic-gold ,
        :metamorphic ,
        :metamorphic-graphite ,
        :metamorphic-group ,
        :metamorphic-hydrothermal ,
        :metamorphic-kyanite ,
        :metasomatic-iron ,
        :mississippi-valley-type-mvt ,
        :mvt-barite ,
        :mvt-fluorspar ,
        :mvt-strontium ,
        :mvt-zinc-lead ,
        :nodular-magnesite ,
        :nodule-manganese ,
        :non-sulfide ,
        :non-sulfide-zinc-lead-mn ,
        :nyf-pegmatite ,
        :oolitic-iron-formation ,
        :ophiolite ,
        :ophiolite-chromium ,
        :ophiolite-cr ,
        :ophiolite-ni-cu-pge ,
        :ophiolite-nickel-copper-pge ,
        :orogenic ,
        :orogenic-copper-gold ,
        :orogenic-graphite ,
        :orogenic-silver-lead-zinc-copper-antimony ,
        :oxidized-intrusion-related-au ,
        :oxidized-intrusion-related-gold ,
        :paleochannel ,
        :paleochannel-iron ,
        :paleoplacer-gold-uranium ,
        :paleoplacer-heavy-mineral-sands ,
        :paleoplacer-tin ,
        :pegmatite ,
        :peralkaline-igneous ,
        :peralkaline-igneous-hfse-ree ,
        :phosphorite ,
        :phosphorite-group ,
        :placer ,
        :porphyry ,
        :porphyry-copper-gold ,
        :porphyry-copper-molybdenum ,
        :porphyry-gold-copper ,
        :porphyry-tin ,
        :porphyry-tungsten ,
        :reduced-intrusion-related-au ,
        :reduced-intrusion-related-gold ,
        :regional-metasomatic ,
        :replacement ,
        :replacement-copper ,
        :replacement-fluorite ,
        :replacement-gold-silver ,
        :replacement-magnesium ,
        :replacement-manganese ,
        :replacement-polymetallic ,
        :replacement-tin ,
        :replacement-zinc-lead ,
        :residual-clay ,
        :residual-placer-lead ,
        :residual-placer-tin ,
        :sandstone-hosted-zinc-lead ,
        :sandstone-uranium ,
        :sediment-hosted ,
        :sediment-hosted-copper-co ,
        :sedimentary-manganese ,
        :shoreline-placer-gold ,
        :siliciclastic-carbonate-zinc-lead ,
        :siliciclastic-mafic-barite ,
        :siliciclastic-mafic-zinc-lead ,
        :simple-pegmatite ,
        :skarn ,
        :skarn-beryllium-fluorite ,
        :skarn-copper ,
        :skarn-gold-copper-tungsten ,
        :skarn-iron ,
        :skarn-molybdenum ,
        :skarn-tin-copper-mo ,
        :skarn-tungsten-mo ,
        :skarn-uranium-ree ,
        :skarn-zinc-lead-silver ,
        :supergene ,
        :supergene-copper ,
        :supergene-gold ,
        :supergene-group ,
        :supergene-iron ,
        :supergene-lead ,
        :supergene-manganese ,
        :supergene-silver ,
        :supergene-uranium ,
        :supergene-vanadium ,
        :supergene-zinc ,
        :superior-type-banded-iron-formation ,
        :superior-type-banded-manganese ,
        :u-m-conduit-ni-cu-pge ,
        :u-m-conduit-nickel-copper-pge ,
        :u-m-intrusion-nickel-copper-pge ,
        :u-m-layered-intrusion-chromium ,
        :u-m-layered-intrusion-iron-titanium-vanadium ,
        :u-m-layered-intrusion-nickel-copper-pge ,
        :u-m-layered-intrusion-pge ,
        :ultramafic-and-or-mafic-conduit ,
        :ultramafic-and-or-mafic-intrusion ,
        :ultramafic-and-or-mafic-layered-intrusion ,
        :unconformity-related ,
        :unconformity-related-ree ,
        :unconformity-related-uranium ,
        :underclay-overclay ,
        :uranium ,
        :vein ,
        :vein-cobalt-ni ,
        :vein-copper ,
        :vein-five-element ,
        :vein-fluorite ,
        :vein-polymetallic ,
        :vein-replacement-nickel ,
        :vein-tin ,
        :vein-tin-polymetallic ,
        :vein-tungsten ,
        :volcanic-basin-hydrothermal ,
        :volcanic-hosted ,
        :volcanic-hosted-copper ,
        :volcanogenic ,
        :volcanogenic-manganese ,
        :volcanogenic-massive-sulfide-vms ,
        :zeolite ;
    skos:prefLabel "Mineral Deposit Model - All Concepts"@en
.