PREFIX dt: <http://resource.geosciml.org/datatype/>
PREFIX rdf: <http://www.w3.org/1999/02/22-rdf-syntax-ns#>
PREFIX rdfs: <http://www.w3.org/2000/01/rdf-schema#>
PREFIX schema: <https://schema.org/>
PREFIX skos: <http://www.w3.org/2004/02/skos/core#>
PREFIX xml: <http://www.w3.org/XML/1998/namespace>
PREFIX xsd: <http://www.w3.org/2001/XMLSchema#>

<http://resource.geosciml.org/classifierscheme/cgi/2016.01/mining-activity> a skos:ConceptScheme ;
    schema:keywords <https://gcmd.earthdata.nasa.gov/kms/concept/e9f67a66-e9fc-435c-b720-ae32a2c3d8f5> ;
    schema:dateCreated "2016-11-29"^^xsd:date ;
    schema:creator <https://linked.data.gov.au/org/cgi-gtwg> ;
    schema:dateModified "2025-06-04"^^xsd:date ;
    schema:citation "The EarthResourceML standard"@en ;
    schema:publisher <https://linked.data.gov.au/org/cgi> ;
    schema:citation "https://earthresourceml.org"^^xsd:anyURI ;
    skos:changeNote "2014-02-23 SMR Original conversion to SKOS."@en,
        "2015-01-08 OLR Edits to fix typos and remove '201401' from rdf file name."@en,
        "2016-11-29 OLR Regenerate SKOS-RDF file as part of migration to new vocabulary server. No change to previous concepts definitions."@en,
        "2020-06-23 NJC Added properties to ensure vocab matched Geoscience Australia's vocab profile (http://linked.data.gov.au/def/ga-skos-profile). Just annotation properties, no new content. Agents (creator/publisher) now not text but RDF resource. Dates (create/modified) derived from editorial notes & existing date properties."@en,
        "2021-12-17 R.Heaven BGS Added prefLabel and altLabel in non English languages, obtained from previously determined alignments between @en labels in CGI and Multi-lingual Thesaurus of Geosciences (MulTG) and Asian Multi-lingual Thesaurus of Geosciences (AMTG). Note that specific language packs are required to render the fonts.  Known issues: @lo and @fi labels were incorrectly encoded in the digitised source datasets; they have been included regardless of this in case the encoding can be corrected."@en ,
        "2025-06-04 NJC Updates metadata to meet the VocPub 5.1 profile"@en ;
    skos:definition "This file contains the CGI Mining Activity vocabulary, as defined by the IUGS Commission for Geoscience Information (CGI) Geoscience Terminology Working Group. The vocabulary defines concepts to categorize the type of mining activity (eg Open Cut, Underground Mine, multiple, unspecified) or processing activity (eg Ore Processing) or production. Using activity to distinguish between the extraction, processing and production activities allows distinguishing between ore mined/grade/recovery, ore treated/grade/recovery and produced payable/plant recovery. By extension, this vocabulary includes all concepts in this conceptScheme, as well as concepts in any previous versions of the scheme."@en ;
    skos:editorialNote "This file contains the 2016 SKOS-RDF version of the CGI Mining Activity vocabulary. Vocabulary Shepherd: Rachel Heaven/Tim McCormick. Compilation and review in Google doc spreadsheet; adopted 9/01/2014; converted to MS Excel XML for SKOS generation using SKOS_for_GA_from_XLS_2016.03.xslt"@en ;
    skos:hasTopConcept <http://resource.geosciml.org/classifier/cgi/mining-activity/subsurface-mining>,
        <http://resource.geosciml.org/classifier/cgi/mining-activity/surface-mining>,
        <http://resource.geosciml.org/classifier/cgi/mining-activity/underwater-mining> ;
    skos:prefLabel "Mining Activity"@en .


<http://resource.geosciml.org/classifier/cgi/mining-activity> a skos:Collection ;
    schema:citation "The original vocabulary - all its concepts"@en ;
    skos:changeNote "2021-12-17 R.Heaven BGS Added alignments to INSPIRE registry codelists using new alignments created automatically using Levenshtein similarity threshold of 0.75."@en ;
    skos:definition "All the Concepts in this vocabulary"@en ;
    skos:member <http://resource.geosciml.org/classifier/cgi/mining-activity/borehole-mining>,
        <http://resource.geosciml.org/classifier/cgi/mining-activity/dredge-mining>,
        <http://resource.geosciml.org/classifier/cgi/mining-activity/hydraulic-mining>,
        <http://resource.geosciml.org/classifier/cgi/mining-activity/in-situ-recovery>,
        <http://resource.geosciml.org/classifier/cgi/mining-activity/open-pit-mining>,
        <http://resource.geosciml.org/classifier/cgi/mining-activity/placer-dredging>,
        <http://resource.geosciml.org/classifier/cgi/mining-activity/quarrying>,
        <http://resource.geosciml.org/classifier/cgi/mining-activity/subaqueous-remote-operated-vehicle>,
        <http://resource.geosciml.org/classifier/cgi/mining-activity/subaqueous-vacuum-pumping>,
        <http://resource.geosciml.org/classifier/cgi/mining-activity/subsurface-mining>,
        <http://resource.geosciml.org/classifier/cgi/mining-activity/surface-mining>,
        <http://resource.geosciml.org/classifier/cgi/mining-activity/surface-placer-mining>,
        <http://resource.geosciml.org/classifier/cgi/mining-activity/underground-mining>,
        <http://resource.geosciml.org/classifier/cgi/mining-activity/underwater-mining> ;
    skos:prefLabel "Mining Activity - All Concepts"@en .


<http://resource.geosciml.org/classifier/cgi/mining-activity/subsurface-mining> a skos:Concept ;
    schema:citation "Dictionary of Mining, Mineral and Related Terms, 2nd ed, AGI 1997"@en ;
    rdfs:isDefinedBy <http://resource.geosciml.org/classifierscheme/cgi/2016.01/mining-activity> ;
    skos:definition "Mining beneath the surface of the earth."@en ;
    skos:exactMatch <http://inspire.ec.europa.eu/codelist/MiningActivityTypeValue/subsurfaceMining> ;
    skos:inScheme <http://resource.geosciml.org/classifierscheme/cgi/2016.01/mining-activity> ;
    skos:narrower <http://resource.geosciml.org/classifier/cgi/mining-activity/borehole-mining>,
        <http://resource.geosciml.org/classifier/cgi/mining-activity/underground-mining> ;
    skos:notation "02.."^^dt:LocalHierarchyKey ;
    skos:prefLabel "subsurface mining"@en ;
    skos:topConceptOf <http://resource.geosciml.org/classifierscheme/cgi/2016.01/mining-activity> .


<http://resource.geosciml.org/classifier/cgi/mining-activity/surface-mining> a skos:Concept ;
    schema:citation "Dictionary of Mining, Mineral and Related Terms, 2nd ed, AGI 1997"@en ;
    rdfs:isDefinedBy <http://resource.geosciml.org/classifierscheme/cgi/2016.01/mining-activity> ;
    skos:definition "Mining via surface excavations."@en ;
    skos:exactMatch <http://inspire.ec.europa.eu/codelist/MiningActivityTypeValue/surfaceMining> ;
    skos:inScheme <http://resource.geosciml.org/classifierscheme/cgi/2016.01/mining-activity> ;
    skos:narrower <http://resource.geosciml.org/classifier/cgi/mining-activity/hydraulic-mining>,
        <http://resource.geosciml.org/classifier/cgi/mining-activity/open-pit-mining>,
        <http://resource.geosciml.org/classifier/cgi/mining-activity/surface-placer-mining> ;
    skos:notation "01.."^^dt:LocalHierarchyKey ;
    skos:prefLabel "surface mining"@en ;
    skos:topConceptOf <http://resource.geosciml.org/classifierscheme/cgi/2016.01/mining-activity> .


<http://resource.geosciml.org/classifier/cgi/mining-activity/underwater-mining> a skos:Concept ;
    rdfs:isDefinedBy <http://resource.geosciml.org/classifierscheme/cgi/2016.01/mining-activity> ;
    skos:definition "Mining of underwater mineral deposits at or close to the sea, lake or river bed. May be from floating or land-based platforms involving dredging or vaccuum pumping or may use remote operated vehicle (submersible)."@en ;
    skos:exactMatch <http://inspire.ec.europa.eu/codelist/MiningActivityTypeValue/underwaterMining> ;
    skos:inScheme <http://resource.geosciml.org/classifierscheme/cgi/2016.01/mining-activity> ;
    skos:narrower <http://resource.geosciml.org/classifier/cgi/mining-activity/dredge-mining>,
        <http://resource.geosciml.org/classifier/cgi/mining-activity/subaqueous-remote-operated-vehicle>,
        <http://resource.geosciml.org/classifier/cgi/mining-activity/subaqueous-vacuum-pumping> ;
    skos:notation "03.."^^dt:LocalHierarchyKey ;
    skos:prefLabel "underwater mining"@en ;
    skos:topConceptOf <http://resource.geosciml.org/classifierscheme/cgi/2016.01/mining-activity> .


<http://resource.geosciml.org/classifier/cgi/mining-activity/borehole-mining> a skos:Concept ;
    schema:citation "Dictionary of Mining, Mineral and Related Terms, 2nd ed, AGI 1997"@en ;
    rdfs:isDefinedBy <http://resource.geosciml.org/classifierscheme/cgi/2016.01/mining-activity> ;
    skos:broader <http://resource.geosciml.org/classifier/cgi/mining-activity/subsurface-mining> ;
    skos:definition "Extraction of a mineral product in the liquid or gaseous state from the Earth's crust by means of boreholes. Boreholes are used for mining petroleum, and for the extraction of liquid solutions of salt, sulfur, etc."@en ;
    skos:exactMatch <http://inspire.ec.europa.eu/codelist/MiningActivityTypeValue/boreholeMining> ;
    skos:inScheme <http://resource.geosciml.org/classifierscheme/cgi/2016.01/mining-activity> ;
    skos:narrower <http://resource.geosciml.org/classifier/cgi/mining-activity/in-situ-recovery> ;
    skos:notation "02.02."^^dt:LocalHierarchyKey ;
    skos:prefLabel "borehole mining"@en .


<http://resource.geosciml.org/classifier/cgi/mining-activity/dredge-mining> a skos:Concept ;
    schema:citation "http://www.britannica.com/EBchecked/topic/171297/dredgin; adapted to include all types of mineral resources, not just placer deposits (e.g. could include sulfide deposits, manganese nodules on sea floor)"@en ;
    rdfs:isDefinedBy <http://resource.geosciml.org/classifierscheme/cgi/2016.01/mining-activity> ;
    skos:broader <http://resource.geosciml.org/classifier/cgi/mining-activity/underwater-mining> ;
    skos:definition "Excavation of underwater mineral resources by floating equipment. Dredging systems are classified as mechanical or hydraulic, depending on the method of material transport."@en ;
    skos:exactMatch <http://inspire.ec.europa.eu/codelist/MiningActivityTypeValue/dredgeMining> ;
    skos:inScheme <http://resource.geosciml.org/classifierscheme/cgi/2016.01/mining-activity> ;
    skos:narrower <http://resource.geosciml.org/classifier/cgi/mining-activity/placer-dredging> ;
    skos:notation "03.03.."^^dt:LocalHierarchyKey ;
    skos:prefLabel "dredge mining"@en .


<http://resource.geosciml.org/classifier/cgi/mining-activity/hydraulic-mining> a skos:Concept ;
    schema:citation "Glossary of Geology. 5th Edition, AGI - online"@en ;
    rdfs:isDefinedBy <http://resource.geosciml.org/classifierscheme/cgi/2016.01/mining-activity> ;
    skos:broader <http://resource.geosciml.org/classifier/cgi/mining-activity/surface-mining> ;
    skos:definition "The recovery of desired material, generally in open pits, by means of strong jets of water"@en ;
    skos:exactMatch <http://inspire.ec.europa.eu/codelist/MiningActivityTypeValue/hydraulicMining> ;
    skos:inScheme <http://resource.geosciml.org/classifierscheme/cgi/2016.01/mining-activity> ;
    skos:notation "01.20."^^dt:LocalHierarchyKey ;
    skos:prefLabel "hydraulic mining"@en .


<http://resource.geosciml.org/classifier/cgi/mining-activity/in-situ-recovery> a skos:Concept ;
    schema:citation "Glossary of Geology. 5th Edition, AGI - online, adapted from chemical mining and enhanced oil recovery"@en ;
    rdfs:isDefinedBy <http://resource.geosciml.org/classifierscheme/cgi/2016.01/mining-activity> ;
    skos:altLabel "chemical mining"@en,
        "solution mining"@en,
        "underground gasification"@en ;
    skos:broader <http://resource.geosciml.org/classifier/cgi/mining-activity/borehole-mining> ;
    skos:definition "The extraction of valuable constituents of an orebody in place from boreholes using thermal, miscible, and chemical methods e.g. by dissolution, leaching, underground gasification"@en ;
    skos:inScheme <http://resource.geosciml.org/classifierscheme/cgi/2016.01/mining-activity> ;
    skos:notation "02.02.01."^^dt:LocalHierarchyKey ;
    skos:prefLabel "Laugungsbergbau"@de,
        "in-situ recovery"@en,
        "explotación por disolución"@es,
        "liuotuslouhinta"@fi,
        "exploitation par dissolution"@fr,
        "penambangan larutan"@id,
        "sfruttamento per dissoluzione"@it,
        "溶解採掘法"@ja,
        "karcMraj;Er:edayviFIsUluysüúg"@km,
        "용액체굴"@ko,
        "¡¾­¢÷©£í­Á»ÈÂ©¨¡¾­Ã§É¦¾­ì½ì¾¨"@lo,
        "perlombongan larutan"@ms,
        "dobycha vyshchelachivaniem"@ru,
        "lakningsbrytning"@sv,
        "การทำเหมืองโดยใช้สารละลาย"@th,
        "khai mỏ bằng phương pháp hoà tan"@vi,
        "溶解法开采"@zh .


<http://resource.geosciml.org/classifier/cgi/mining-activity/open-pit-mining> a skos:Concept ;
    schema:citation "CGI/ERML 2.0"@en ;
    rdfs:isDefinedBy <http://resource.geosciml.org/classifierscheme/cgi/2016.01/mining-activity> ;
    skos:altLabel "open cut mining"@en,
        "open sky mining"@en,
        "open-cast mining"@en,
        "strip mining"@en ;
    skos:broader <http://resource.geosciml.org/classifier/cgi/mining-activity/surface-mining> ;
    skos:definition "An open-sky excavation for the extraction of mineral resources (eg, open cut, open cast, strip mining)"@en ;
    skos:inScheme <http://resource.geosciml.org/classifierscheme/cgi/2016.01/mining-activity> ;
    skos:narrower <http://resource.geosciml.org/classifier/cgi/mining-activity/quarrying> ;
    skos:notation "01.03."^^dt:LocalHierarchyKey ;
    skos:prefLabel "Tagebau"@de,
        "open-pit mining"@en,
        "cielo abierto"@es,
        "avolouhinta"@fi,
        "ciel ouvert"@fr,
        "penambangan terbuka"@id,
        "miniera a cielo aperto"@it,
        "露天採掘"@ja,
        "GNþÚgEr:ebIk"@km,
        "노천채굴"@ko,
        "¡¾­¢÷©£í­Á®®®ÒÀ¯ò©"@lo,
        "lombong lelubang terbuka"@ms,
        "razrabotka otkrytaya"@ru,
        "dagbrott"@sv,
        "เหมืองเปิด"@th,
        "khai mỏ lộ thiên"@vi,
        "露天采矿"@zh .


<http://resource.geosciml.org/classifier/cgi/mining-activity/placer-dredging> a skos:Concept ;
    schema:citation "this vocabulary"@en ;
    rdfs:isDefinedBy <http://resource.geosciml.org/classifierscheme/cgi/2016.01/mining-activity> ;
    skos:broader <http://resource.geosciml.org/classifier/cgi/mining-activity/dredge-mining>,
        <http://resource.geosciml.org/classifier/cgi/mining-activity/surface-placer-mining> ;
    skos:definition "The extraction of minerals from an underwater placer deposit by the use of floating equipment for scooping or suction"@en ;
    skos:inScheme <http://resource.geosciml.org/classifierscheme/cgi/2016.01/mining-activity> ;
    skos:notation "01.01.01."^^dt:LocalHierarchyKey ;
    skos:prefLabel "placer dredging"@en .


<http://resource.geosciml.org/classifier/cgi/mining-activity/quarrying> a skos:Concept ;
    schema:citation "Glossary of Geology. 5th Edition, AGI - online"@en ;
    rdfs:isDefinedBy <http://resource.geosciml.org/classifierscheme/cgi/2016.01/mining-activity> ;
    skos:broader <http://resource.geosciml.org/classifier/cgi/mining-activity/open-pit-mining> ;
    skos:definition "The extraction of building stone or other valuable nonmetallic constituent from an open or surface mineral working. It is distinguished from a mine because a quarry usually is open at the top and front, and, in ordinary use of the term, by the character of the material extracted."@en ;
    skos:exactMatch <http://inspire.ec.europa.eu/codelist/MiningActivityTypeValue/quarry> ;
    skos:inScheme <http://resource.geosciml.org/classifierscheme/cgi/2016.01/mining-activity> ;
    skos:notation "01.03.01."^^dt:LocalHierarchyKey ;
    skos:prefLabel "quarrying"@en .


<http://resource.geosciml.org/classifier/cgi/mining-activity/subaqueous-remote-operated-vehicle> a skos:Concept ;
    schema:citation "this vocabulary"@en ;
    rdfs:isDefinedBy <http://resource.geosciml.org/classifierscheme/cgi/2016.01/mining-activity> ;
    skos:broader <http://resource.geosciml.org/classifier/cgi/mining-activity/underwater-mining> ;
    skos:definition "not given"@en ;
    skos:exactMatch <http://inspire.ec.europa.eu/codelist/MiningActivityTypeValue/subaqueousRemoteOperatedVehicle> ;
    skos:inScheme <http://resource.geosciml.org/classifierscheme/cgi/2016.01/mining-activity> ;
    skos:notation "03.02.."^^dt:LocalHierarchyKey ;
    skos:prefLabel "subaqueous remote operated vehicle"@en .


<http://resource.geosciml.org/classifier/cgi/mining-activity/subaqueous-vacuum-pumping> a skos:Concept ;
    schema:citation "this vocabulary"@en ;
    rdfs:isDefinedBy <http://resource.geosciml.org/classifierscheme/cgi/2016.01/mining-activity> ;
    skos:broader <http://resource.geosciml.org/classifier/cgi/mining-activity/underwater-mining> ;
    skos:definition "not given"@en ;
    skos:exactMatch <http://inspire.ec.europa.eu/codelist/MiningActivityTypeValue/subaqueousVacuumPumping> ;
    skos:inScheme <http://resource.geosciml.org/classifierscheme/cgi/2016.01/mining-activity> ;
    skos:notation "03.01.."^^dt:LocalHierarchyKey ;
    skos:prefLabel "subaqueous vacuum pumping"@en .


<http://resource.geosciml.org/classifier/cgi/mining-activity/surface-placer-mining> a skos:Concept ;
    schema:citation "Dictionary of Mining, Mineral and Related Terms, 2nd ed, AGI 1997"@en ;
    rdfs:isDefinedBy <http://resource.geosciml.org/classifierscheme/cgi/2016.01/mining-activity> ;
    skos:altLabel "alluvial mining"@en ;
    skos:broader <http://resource.geosciml.org/classifier/cgi/mining-activity/surface-mining> ;
    skos:definition "The extraction of heavy mineral from beach or sand-bank deposits by concentration in running water. It includes ground sluicing, panning, shoveling gravel into a sluice, scraping by power scraper and excavation by dragline, dredge or other mechanized equipment."@en ;
    skos:inScheme <http://resource.geosciml.org/classifierscheme/cgi/2016.01/mining-activity> ;
    skos:narrower <http://resource.geosciml.org/classifier/cgi/mining-activity/placer-dredging> ;
    skos:notation "01.01."^^dt:LocalHierarchyKey ;
    skos:prefLabel "surface placer mining"@en .


<http://resource.geosciml.org/classifier/cgi/mining-activity/underground-mining> a skos:Concept ;
    schema:citation "Dictionary of Mining, Mineral and Related Terms, 1st edition"@en ;
    rdfs:isDefinedBy <http://resource.geosciml.org/classifierscheme/cgi/2016.01/mining-activity> ;
    skos:altLabel "lombong bawah tanah"@ms,
        "地下采矿"@zh ;
    skos:broader <http://resource.geosciml.org/classifier/cgi/mining-activity/subsurface-mining> ;
    skos:definition "A mineral extraction activity in which ore is extracted from the subsurface via underground mine workings (adits, shafts, drifts, stopes, etc.)."@en ;
    skos:exactMatch <http://inspire.ec.europa.eu/codelist/MiningActivityTypeValue/underground> ;
    skos:inScheme <http://resource.geosciml.org/classifierscheme/cgi/2016.01/mining-activity> ;
    skos:notation "02.01."^^dt:LocalHierarchyKey ;
    skos:prefLabel "unterirdische Gewinnung"@de,
        "underground mining"@en,
        "minería subterránea"@es,
        "maanalainen louhinta"@fi,
        "mine souterraine"@fr,
        "penambangan bawah tanah"@id,
        "coltivazione in sottosuolo"@it,
        "抗内採掘"@ja,
        "GaCIvkmµEr:eRkamdI"@km,
        "갱내채광"@ko,
        "¡¾­¢÷©£í­Á»úÃªÉ©ò­"@lo,
        "perlombongan bawah tanah"@ms,
        "vyrabotka podzemnaya"@ru,
        "underjordsbrytning"@sv,
        "เหมืองใต้ดิน"@th,
        "khai thác ngầm"@vi,
        "地下开采"@zh .

