PREFIX cs: <http://resource.geosciml.org/classifierscheme/cgi/2016.01/geologicunitmorphology>
PREFIX rdfs: <http://www.w3.org/2000/01/rdf-schema#>
PREFIX schema: <https://schema.org/>
PREFIX skos: <http://www.w3.org/2004/02/skos/core#>
PREFIX xsd: <http://www.w3.org/2001/XMLSchema#>

<http://resource.geosciml.org/classifier/cgi/geologicunitmorphology>
    a skos:Collection ;
    rdfs:isDefinedBy cs: ;
    skos:definition "All Concepts in this vocabulary" ;
    skos:historyNote "this vocabulary" ;
    skos:inScheme cs: ;
    skos:member
        <http://resource.geosciml.org/classifier/cgi/geologicunitmorphology/arch_morphology> ,
        <http://resource.geosciml.org/classifier/cgi/geologicunitmorphology/arcuate_sheet> ,
        <http://resource.geosciml.org/classifier/cgi/geologicunitmorphology/basin_shape> ,
        <http://resource.geosciml.org/classifier/cgi/geologicunitmorphology/blanket_shape> ,
        <http://resource.geosciml.org/classifier/cgi/geologicunitmorphology/blob> ,
        <http://resource.geosciml.org/classifier/cgi/geologicunitmorphology/block> ,
        <http://resource.geosciml.org/classifier/cgi/geologicunitmorphology/boudin_shape> ,
        <http://resource.geosciml.org/classifier/cgi/geologicunitmorphology/bread_loaf_ellipsoid> ,
        <http://resource.geosciml.org/classifier/cgi/geologicunitmorphology/channel_shape> ,
        <http://resource.geosciml.org/classifier/cgi/geologicunitmorphology/circular_cylinder> ,
        <http://resource.geosciml.org/classifier/cgi/geologicunitmorphology/circular_profile> ,
        <http://resource.geosciml.org/classifier/cgi/geologicunitmorphology/column_shape> ,
        <http://resource.geosciml.org/classifier/cgi/geologicunitmorphology/cone> ,
        <http://resource.geosciml.org/classifier/cgi/geologicunitmorphology/cone_segment> ,
        <http://resource.geosciml.org/classifier/cgi/geologicunitmorphology/conical_sheet> ,
        <http://resource.geosciml.org/classifier/cgi/geologicunitmorphology/cupola> ,
        <http://resource.geosciml.org/classifier/cgi/geologicunitmorphology/cylinder> ,
        <http://resource.geosciml.org/classifier/cgi/geologicunitmorphology/dart_ellipsoid> ,
        <http://resource.geosciml.org/classifier/cgi/geologicunitmorphology/diapir> ,
        <http://resource.geosciml.org/classifier/cgi/geologicunitmorphology/dike> ,
        <http://resource.geosciml.org/classifier/cgi/geologicunitmorphology/disc> ,
        <http://resource.geosciml.org/classifier/cgi/geologicunitmorphology/discoid_anulus> ,
        <http://resource.geosciml.org/classifier/cgi/geologicunitmorphology/discus> ,
        <http://resource.geosciml.org/classifier/cgi/geologicunitmorphology/dome> ,
        <http://resource.geosciml.org/classifier/cgi/geologicunitmorphology/dome_sheet> ,
        <http://resource.geosciml.org/classifier/cgi/geologicunitmorphology/ductolith> ,
        <http://resource.geosciml.org/classifier/cgi/geologicunitmorphology/ellipsoid> ,
        <http://resource.geosciml.org/classifier/cgi/geologicunitmorphology/elliptical_cylinder> ,
        <http://resource.geosciml.org/classifier/cgi/geologicunitmorphology/elliptical_profile> ,
        <http://resource.geosciml.org/classifier/cgi/geologicunitmorphology/elongate_discus> ,
        <http://resource.geosciml.org/classifier/cgi/geologicunitmorphology/equant_polygonal_profile> ,
        <http://resource.geosciml.org/classifier/cgi/geologicunitmorphology/equant_profile> ,
        <http://resource.geosciml.org/classifier/cgi/geologicunitmorphology/ethmolith> ,
        <http://resource.geosciml.org/classifier/cgi/geologicunitmorphology/fan> ,
        <http://resource.geosciml.org/classifier/cgi/geologicunitmorphology/football_ellipsoid> ,
        <http://resource.geosciml.org/classifier/cgi/geologicunitmorphology/geologic_body> ,
        <http://resource.geosciml.org/classifier/cgi/geologicunitmorphology/graben_shape> ,
        <http://resource.geosciml.org/classifier/cgi/geologicunitmorphology/hemispheroid> ,
        <http://resource.geosciml.org/classifier/cgi/geologicunitmorphology/irregular_profile> ,
        <http://resource.geosciml.org/classifier/cgi/geologicunitmorphology/laccolith> ,
        <http://resource.geosciml.org/classifier/cgi/geologicunitmorphology/layer_shape> ,
        <http://resource.geosciml.org/classifier/cgi/geologicunitmorphology/lens> ,
        <http://resource.geosciml.org/classifier/cgi/geologicunitmorphology/lenticular_profile> ,
        <http://resource.geosciml.org/classifier/cgi/geologicunitmorphology/longitudinal_section_of_cylinder> ,
        <http://resource.geosciml.org/classifier/cgi/geologicunitmorphology/lopolith> ,
        <http://resource.geosciml.org/classifier/cgi/geologicunitmorphology/mound> ,
        <http://resource.geosciml.org/classifier/cgi/geologicunitmorphology/pancake_ellipsoid> ,
        <http://resource.geosciml.org/classifier/cgi/geologicunitmorphology/phacolith> ,
        <http://resource.geosciml.org/classifier/cgi/geologicunitmorphology/pillow_ellipsoid> ,
        <http://resource.geosciml.org/classifier/cgi/geologicunitmorphology/pipe> ,
        <http://resource.geosciml.org/classifier/cgi/geologicunitmorphology/planar_profile> ,
        <http://resource.geosciml.org/classifier/cgi/geologicunitmorphology/planar_sheet> ,
        <http://resource.geosciml.org/classifier/cgi/geologicunitmorphology/planar_vein> ,
        <http://resource.geosciml.org/classifier/cgi/geologicunitmorphology/pod> ,
        <http://resource.geosciml.org/classifier/cgi/geologicunitmorphology/polygonal_cylinder> ,
        <http://resource.geosciml.org/classifier/cgi/geologicunitmorphology/polygonal_profile> ,
        <http://resource.geosciml.org/classifier/cgi/geologicunitmorphology/prism> ,
        <http://resource.geosciml.org/classifier/cgi/geologicunitmorphology/ribbon> ,
        <http://resource.geosciml.org/classifier/cgi/geologicunitmorphology/ring_dyke> ,
        <http://resource.geosciml.org/classifier/cgi/geologicunitmorphology/rock_body_geometry_irregular> ,
        <http://resource.geosciml.org/classifier/cgi/geologicunitmorphology/rock_body_geometry_not_specified> ,
        <http://resource.geosciml.org/classifier/cgi/geologicunitmorphology/rod> ,
        <http://resource.geosciml.org/classifier/cgi/geologicunitmorphology/sheet> ,
        <http://resource.geosciml.org/classifier/cgi/geologicunitmorphology/sheet_ellipsoid> ,
        <http://resource.geosciml.org/classifier/cgi/geologicunitmorphology/sigmoid_sheet> ,
        <http://resource.geosciml.org/classifier/cgi/geologicunitmorphology/sigmoidal_vein> ,
        <http://resource.geosciml.org/classifier/cgi/geologicunitmorphology/sill_form> ,
        <http://resource.geosciml.org/classifier/cgi/geologicunitmorphology/sphenolith> ,
        <http://resource.geosciml.org/classifier/cgi/geologicunitmorphology/spheroid> ,
        <http://resource.geosciml.org/classifier/cgi/geologicunitmorphology/square_profile> ,
        <http://resource.geosciml.org/classifier/cgi/geologicunitmorphology/tablet> ,
        <http://resource.geosciml.org/classifier/cgi/geologicunitmorphology/tabular_prism> ,
        <http://resource.geosciml.org/classifier/cgi/geologicunitmorphology/tear_drop> ,
        <http://resource.geosciml.org/classifier/cgi/geologicunitmorphology/three_dimensional_body> ,
        <http://resource.geosciml.org/classifier/cgi/geologicunitmorphology/trough> ,
        <http://resource.geosciml.org/classifier/cgi/geologicunitmorphology/vein> ,
        <http://resource.geosciml.org/classifier/cgi/geologicunitmorphology/wedge> ;
    skos:prefLabel "Geologic Unit Morphology - All Concepts"@en ;
.

<http://resource.geosciml.org/classifier/cgi/geologicunitmorphology/arch_morphology>
    a skos:Concept ;
    rdfs:isDefinedBy cs: ;
    skos:broader <http://resource.geosciml.org/classifier/cgi/geologicunitmorphology/geologic_body> ;
    skos:definition "A raised elongate body, morphologically equivalent to upside down channel"@en ;
    skos:historyNote "This vocabulary"@en ;
    skos:inScheme cs: ;
    skos:prefLabel "arch morphology"@en ;
    skos:related <http://resource.geosciml.org/classifier/cgi/geologicunitmorphology/longitudinal_section_of_cylinder> ;
.

<http://resource.geosciml.org/classifier/cgi/geologicunitmorphology/basin_shape>
    a skos:Concept ;
    rdfs:isDefinedBy cs: ;
    skos:altLabel "buffertzon"@sv ;
    skos:broader <http://resource.geosciml.org/classifier/cgi/geologicunitmorphology/geologic_body> ;
    skos:definition "Geometric analog is convex down discoid, term generally connotes a kilometer-scale feature. Map view may be circular, elliptical, or irregular, characteristic feature is thickening from the edges towards the center. Typically used to describe a body of sedimentary rock deposited in a low area in the Earth's crust, in which case there is an implication that the top is (or was) a surface of deposition."@en ;
    skos:historyNote "This vocabulary"@en ;
    skos:inScheme cs: ;
    skos:prefLabel "basin shape"@en ;
    skos:related
        <http://resource.geosciml.org/classifier/cgi/geologicunitmorphology/discus> ,
        <http://resource.geosciml.org/classifier/cgi/geologicunitmorphology/hemispheroid> ;
.

<http://resource.geosciml.org/classifier/cgi/geologicunitmorphology/block>
    a skos:Concept ;
    rdfs:isDefinedBy cs: ;
    skos:altLabel
        "Blockstruktur"@de ,
        "estructura bloques"@es ,
        "lohkorakenteet"@fi ,
        "structure bloc"@fr ,
        "bangun bongkah"@id ,
        "struktur bongkah"@id ,
        "struttura a blocchi"@it ,
        "地塊構造"@ja ,
        "rcnasm<½nCabøúk"@km ,
        "암괴구조"@ko ,
        "지괴구조"@ko ,
        "Â£¤¦É¾¤»ø®®ìñº¡"@lo ,
        "struktur bongkah"@ms ,
        "struktura blokovaya"@ru ,
        "blockstruktur"@sv ,
        "โครงสร้างบล็อก"@th ,
        "cấu trúc khối"@vi ,
        "块状构造"@zh ;
    skos:broader <http://resource.geosciml.org/classifier/cgi/geologicunitmorphology/polygonal_cylinder> ;
    skos:definition "Equant polygonal cylinder, L=W=H, definable edges separate bounding surfaces. Grades to tabular prism as one horizontal dimension becomes distinctly longer than the other, and tablet or polygonal cylinder as one vertical axis becomes distinctly shorter or longer than the horizontal axes."@en ;
    skos:historyNote "This vocabulary"@en ;
    skos:inScheme cs: ;
    skos:prefLabel "block"@en ;
.

<http://resource.geosciml.org/classifier/cgi/geologicunitmorphology/boudin_shape>
    a skos:Concept ;
    rdfs:isDefinedBy cs: ;
    skos:broader <http://resource.geosciml.org/classifier/cgi/geologicunitmorphology/geologic_body> ;
    skos:definition "Layer or bed of rock deformed into sausage-shaped segments (boudins), either separated or joined by pinched connections. Morphology generally defined in a profile view, third dimension is not denoted, use of term also implies that the body is not isolated, but is related to an original body elongate on some dimension that has been stretched and separated into separate bodies"@en ;
    skos:historyNote "This vocabulary"@en ;
    skos:inScheme cs: ;
    skos:prefLabel "boudin shape"@en ;
    skos:related <http://resource.geosciml.org/classifier/cgi/geologicunitmorphology/bread_loaf_ellipsoid> ;
.

<http://resource.geosciml.org/classifier/cgi/geologicunitmorphology/channel_shape>
    a skos:Concept ;
    rdfs:isDefinedBy cs: ;
    skos:altLabel
        "Rinne"@de ,
        "canal natural"@es ,
        "uomat"@fi ,
        "canale"@it ,
        "ruslo"@ru ,
        "gully"@sv ,
        "kanal"@sv ;
    skos:broader <http://resource.geosciml.org/classifier/cgi/geologicunitmorphology/geologic_body> ;
    skos:definition "Strongly elongate lens or ribbon with a convex downward lower surface, near planar upper surface. Morphology is equivalent to upside down arch."@en ;
    skos:historyNote "This vocabulary"@en ;
    skos:inScheme cs: ;
    skos:prefLabel "channel shape"@en ;
    skos:related
        <http://resource.geosciml.org/classifier/cgi/geologicunitmorphology/longitudinal_section_of_cylinder> ,
        <http://resource.geosciml.org/classifier/cgi/geologicunitmorphology/ribbon> ;
.

<http://resource.geosciml.org/classifier/cgi/geologicunitmorphology/circular_profile>
    a skos:Concept ;
    rdfs:isDefinedBy cs: ;
    skos:broader <http://resource.geosciml.org/classifier/cgi/geologicunitmorphology/equant_profile> ;
    skos:definition "equant profile with arcuate boundary"@en ;
    skos:historyNote "This vocabulary"@en ;
    skos:inScheme cs: ;
    skos:prefLabel "circular profile"@en ;
.

<http://resource.geosciml.org/classifier/cgi/geologicunitmorphology/column_shape>
    a skos:Concept ;
    rdfs:isDefinedBy cs: ;
    skos:broader <http://resource.geosciml.org/classifier/cgi/geologicunitmorphology/geologic_body> ;
    skos:definition "Cylindrical body, equant cross section, long in direction normal to equant cross section. Morphology equivalent to pipe, without denotation of transport function."@en ;
    skos:historyNote "This vocabulary"@en ;
    skos:inScheme cs: ;
    skos:prefLabel "column shape"@en ;
    skos:related
        <http://resource.geosciml.org/classifier/cgi/geologicunitmorphology/circular_cylinder> ,
        <http://resource.geosciml.org/classifier/cgi/geologicunitmorphology/polygonal_cylinder> ;
.

<http://resource.geosciml.org/classifier/cgi/geologicunitmorphology/conical_sheet>
    a skos:Concept ;
    rdfs:isDefinedBy cs: ;
    skos:broader <http://resource.geosciml.org/classifier/cgi/geologicunitmorphology/sheet> ;
    skos:definition "Sheet that conforms to surface of a cone."@en ;
    skos:historyNote "This vocabulary"@en ;
    skos:inScheme cs: ;
    skos:prefLabel "conical sheet"@en ;
.

<http://resource.geosciml.org/classifier/cgi/geologicunitmorphology/cupola>
    a skos:Concept ;
    rdfs:isDefinedBy cs: ;
    skos:broader <http://resource.geosciml.org/classifier/cgi/geologicunitmorphology/geologic_body> ;
    skos:definition "Large upward projection of the roof of an igneous intrusion into the country rock above. A possibly irregular dome like or columnar body rooted in a larger body."@en ;
    skos:historyNote "This vocabulary"@en ;
    skos:inScheme cs: ;
    skos:prefLabel "cupola"@en ;
    skos:related <http://resource.geosciml.org/classifier/cgi/geologicunitmorphology/hemispheroid> ;
.

<http://resource.geosciml.org/classifier/cgi/geologicunitmorphology/dart_ellipsoid>
    a skos:Concept ;
    rdfs:isDefinedBy cs: ;
    skos:broader <http://resource.geosciml.org/classifier/cgi/geologicunitmorphology/ellipsoid> ;
    skos:definition "Ellipsoid with L more than 50 times W or H"@en ;
    skos:historyNote "This vocabulary"@en ;
    skos:inScheme cs: ;
    skos:prefLabel "dart ellipsoid"@en ;
.

<http://resource.geosciml.org/classifier/cgi/geologicunitmorphology/disc>
    a skos:Concept ;
    rdfs:isDefinedBy cs: ;
    skos:broader <http://resource.geosciml.org/classifier/cgi/geologicunitmorphology/cylinder> ;
    skos:definition "Cylinder with height less than diameter. L=W>H, edges separates side from top and bottom. Grades to oblate ellipsoid as edges lose definition."@en ;
    skos:historyNote "This vocabulary"@en ;
    skos:inScheme cs: ;
    skos:prefLabel "disc"@en ;
.

<http://resource.geosciml.org/classifier/cgi/geologicunitmorphology/discoid_anulus>
    a skos:Concept ;
    rdfs:isDefinedBy cs: ;
    skos:broader <http://resource.geosciml.org/classifier/cgi/geologicunitmorphology/three_dimensional_body> ;
    skos:definition "Cone with central part removed along cylindrical volume approximately along the cone axis"@en ;
    skos:historyNote "This vocabulary"@en ;
    skos:inScheme cs: ;
    skos:prefLabel "discoid anulus"@en ;
.

<http://resource.geosciml.org/classifier/cgi/geologicunitmorphology/dome>
    a skos:Concept ;
    rdfs:isDefinedBy cs: ;
    skos:altLabel
        "Dom"@de ,
        "domo"@es ,
        "doomit"@fi ,
        "duomo"@it ,
        "kupol"@ru ,
        "dom"@sv ;
    skos:broader <http://resource.geosciml.org/classifier/cgi/geologicunitmorphology/geologic_body> ;
    skos:definition "Steep-sided disk-like body, for example and accumulation of high viscosity lava above and around a volcanic vent. A structure in which the top of the body dips gently away in all directions e.g. salt dome, extrusion dome"@en ;
    skos:historyNote "This vocabulary"@en ;
    skos:inScheme cs: ;
    skos:prefLabel "dome"@en ;
    skos:related <http://resource.geosciml.org/classifier/cgi/geologicunitmorphology/hemispheroid> ;
.

<http://resource.geosciml.org/classifier/cgi/geologicunitmorphology/dome_sheet>
    a skos:Concept ;
    rdfs:isDefinedBy cs: ;
    skos:broader <http://resource.geosciml.org/classifier/cgi/geologicunitmorphology/sheet> ;
    skos:definition "Sheet in which L and W are curved arcs."@en ;
    skos:historyNote "This vocabulary"@en ;
    skos:inScheme cs: ;
    skos:prefLabel "dome sheet"@en ;
.

<http://resource.geosciml.org/classifier/cgi/geologicunitmorphology/ductolith>
    a skos:Concept ;
    rdfs:isDefinedBy cs: ;
    skos:broader <http://resource.geosciml.org/classifier/cgi/geologicunitmorphology/geologic_body> ;
    skos:definition "Concordant intrusion, teardrop-shaped in cross section."@en ;
    skos:historyNote "This vocabulary"@en ;
    skos:inScheme cs: ;
    skos:prefLabel "ductolith"@en ;
    skos:related
        <http://resource.geosciml.org/classifier/cgi/geologicunitmorphology/diapir> ,
        <http://resource.geosciml.org/classifier/cgi/geologicunitmorphology/tear_drop> ;
.

<http://resource.geosciml.org/classifier/cgi/geologicunitmorphology/elliptical_profile>
    a skos:Concept ;
    rdfs:isDefinedBy cs: ;
    skos:broader <http://resource.geosciml.org/classifier/cgi/geologicunitmorphology/planar_profile> ;
    skos:definition "Profile approximates an ellipse, ratio of long axis to short axis is greater than 1.4"@en ;
    skos:historyNote "This vocabulary"@en ;
    skos:inScheme cs: ;
    skos:prefLabel "elliptical profile"@en ;
.

<http://resource.geosciml.org/classifier/cgi/geologicunitmorphology/elongate_discus>
    a skos:Concept ;
    rdfs:isDefinedBy cs: ;
    skos:broader <http://resource.geosciml.org/classifier/cgi/geologicunitmorphology/discus> ;
    skos:definition "Discus for which the profile defined by the bounding edge is longer in one direction than other. L>W>>H"@en ;
    skos:historyNote "This vocabulary"@en ;
    skos:inScheme cs: ;
    skos:prefLabel "elongate discus"@en ;
.

<http://resource.geosciml.org/classifier/cgi/geologicunitmorphology/equant_polygonal_profile>
    a skos:Concept ;
    rdfs:isDefinedBy cs: ;
    skos:broader <http://resource.geosciml.org/classifier/cgi/geologicunitmorphology/equant_profile> ;
    skos:definition "Aquant profile with boundary that can be divided into distinct straight sides separated by higher curvature corners."@en ;
    skos:historyNote "This vocabulary"@en ;
    skos:inScheme cs: ;
    skos:prefLabel "equant polygonal profile"@en ;
.

<http://resource.geosciml.org/classifier/cgi/geologicunitmorphology/ethmolith>
    a skos:Concept ;
    rdfs:isDefinedBy cs: ;
    skos:broader <http://resource.geosciml.org/classifier/cgi/geologicunitmorphology/geologic_body> ;
    skos:definition "Discordant, funnel-shaped intrusion, tapers downward"@en ;
    skos:historyNote "This vocabulary"@en ;
    skos:inScheme cs: ;
    skos:prefLabel "ethmolith"@en ;
    skos:related <http://resource.geosciml.org/classifier/cgi/geologicunitmorphology/cone> ;
.

<http://resource.geosciml.org/classifier/cgi/geologicunitmorphology/fan>
    a skos:Concept ;
    rdfs:isDefinedBy cs: ;
    skos:altLabel
        "Faecher"@de ,
        "cono"@es ,
        "keilat"@fi ,
        "conoide"@it ,
        "vynos veeroobraznyj"@ru ,
        "kon"@sv ;
    skos:broader <http://resource.geosciml.org/classifier/cgi/geologicunitmorphology/geologic_body> ;
    skos:definition "A cone segment, generally applied to surface morphology of sedimentary deposit with a gentle surface slope, radiating from a localized sediment source."@en ;
    skos:historyNote "This vocabulary"@en ;
    skos:inScheme cs: ;
    skos:prefLabel "fan"@en ;
    skos:related <http://resource.geosciml.org/classifier/cgi/geologicunitmorphology/cone_segment> ;
.

<http://resource.geosciml.org/classifier/cgi/geologicunitmorphology/football_ellipsoid>
    a skos:Concept ;
    rdfs:isDefinedBy cs: ;
    skos:broader <http://resource.geosciml.org/classifier/cgi/geologicunitmorphology/ellipsoid> ;
    skos:definition "Ellipsoid with L 2 to 5 times W or H"@en ;
    skos:historyNote "This vocabulary"@en ;
    skos:inScheme cs: ;
    skos:prefLabel "football ellipsoid"@en ;
.

<http://resource.geosciml.org/classifier/cgi/geologicunitmorphology/graben_shape>
    a skos:Concept ;
    rdfs:isDefinedBy cs: ;
    skos:altLabel
        "Graben"@de ,
        "graben"@es ,
        "hautavajoamat"@fi ,
        "graben"@it ,
        "graben"@ru ,
        "gravsänka"@sv ;
    skos:broader <http://resource.geosciml.org/classifier/cgi/geologicunitmorphology/geologic_body> ;
    skos:definition "an elongate body bounded on both sides by normal faults that dip toward each other"@en ;
    skos:historyNote "This vocabulary"@en ;
    skos:inScheme cs: ;
    skos:prefLabel "graben shape"@en ;
    skos:related <http://resource.geosciml.org/classifier/cgi/geologicunitmorphology/tabular_prism> ;
.

<http://resource.geosciml.org/classifier/cgi/geologicunitmorphology/irregular_profile>
    a skos:Concept ;
    rdfs:isDefinedBy cs: ;
    skos:broader <http://resource.geosciml.org/classifier/cgi/geologicunitmorphology/planar_profile> ;
    skos:definition "Profile does not conform to any of the regular geometries associated with other categories in the vocabulary."@en ;
    skos:historyNote "This vocabulary"@en ;
    skos:inScheme cs: ;
    skos:prefLabel "irregular profile"@en ;
.

<http://resource.geosciml.org/classifier/cgi/geologicunitmorphology/laccolith>
    a skos:Concept ;
    rdfs:isDefinedBy cs: ;
    skos:altLabel
        "Lakkolith"@de ,
        "lacolito"@es ,
        "lakkoliitit"@fi ,
        "laccolite"@fr ,
        "lakolit"@id ,
        "laccolite"@it ,
        "ラコリス"@ja ,
        "Lk;kUlIt"@km ,
        "병반"@ko ,
        "¹ó­-ºñ¡-£½-­ó-»ø®-À¹ñ©"@lo ,
        "¹ó­Áìñ¡-Â£-ìò©"@lo ,
        "lakolitos"@ms ,
        "lakkolit"@ru ,
        "lakkolit"@sv ,
        "หินอัคนีรูปเห็ด"@th ,
        "thể nấm"@vi ,
        "岩盖"@zh ,
        "岩盘"@zh ,
        "菌形穹隆"@zh ;
    skos:broader <http://resource.geosciml.org/classifier/cgi/geologicunitmorphology/geologic_body> ;
    skos:definition "A tabular or lenticular igneous body whose long dimensions parallel layering in the host rock, and which as a convex-up roof and a known or assumed flat floor"@en ;
    skos:historyNote "This vocabulary"@en ;
    skos:inScheme cs: ;
    skos:prefLabel "laccolith"@en ;
    skos:related
        <http://resource.geosciml.org/classifier/cgi/geologicunitmorphology/discus> ,
        <http://resource.geosciml.org/classifier/cgi/geologicunitmorphology/sheet_ellipsoid> ;
.

<http://resource.geosciml.org/classifier/cgi/geologicunitmorphology/lens>
    a skos:Concept ;
    rdfs:isDefinedBy cs: ;
    skos:altLabel
        "Linse"@de ,
        "lentejón"@es ,
        "linssit"@fi ,
        "lente"@it ,
        "linza"@ru ,
        "lins"@sv ;
    skos:broader <http://resource.geosciml.org/classifier/cgi/geologicunitmorphology/geologic_body> ;
    skos:definition "A body bounded by converging surfaces (at least one of which is curved), thick in the middle and thinning out toward the edges, resembling a convex lens."@en ;
    skos:historyNote "This vocabulary"@en ;
    skos:inScheme cs: ;
    skos:prefLabel "lens"@en ;
    skos:related <http://resource.geosciml.org/classifier/cgi/geologicunitmorphology/discus> ;
.

<http://resource.geosciml.org/classifier/cgi/geologicunitmorphology/lenticular_profile>
    a skos:Concept ;
    rdfs:isDefinedBy cs: ;
    skos:broader <http://resource.geosciml.org/classifier/cgi/geologicunitmorphology/planar_profile> ;
    skos:definition "Profile with ratio of long axis length to short axis length greater than 5 with sides that taper to a point, shaped like the profile of an optical lense."@en ;
    skos:historyNote "This vocabulary"@en ;
    skos:inScheme cs: ;
    skos:prefLabel "lenticular profile"@en ;
.

<http://resource.geosciml.org/classifier/cgi/geologicunitmorphology/lopolith>
    a skos:Concept ;
    rdfs:isDefinedBy cs: ;
    skos:altLabel
        "Lopolith"@de ,
        "lopolito"@es ,
        "lopoliitit"@fi ,
        "lopolite"@fr ,
        "lopolit"@id ,
        "lopolite"@it ,
        "ロポリス"@ja ,
        "silaEdllatsn§wgkñúgtMbn;"@km ,
        "분상암체"@ko ,
        "ÂìÂ²ìò©"@lo ,
        "lopolitos"@ms ,
        "lopolit"@ru ,
        "lopolit"@sv ,
        "หินอัคนีรูปฝักบัว"@th ,
        "thể chậu"@vi ,
        "岩盆"@zh ;
    skos:broader <http://resource.geosciml.org/classifier/cgi/geologicunitmorphology/geologic_body> ;
    skos:definition "A large, concordant, typically layered igneous intrusion whose floor is convex-down and whose roof may be convex-down or flat."@en ;
    skos:historyNote "This vocabulary"@en ;
    skos:inScheme cs: ;
    skos:prefLabel "lopolith"@en ;
    skos:related
        <http://resource.geosciml.org/classifier/cgi/geologicunitmorphology/discus> ,
        <http://resource.geosciml.org/classifier/cgi/geologicunitmorphology/sheet_ellipsoid> ;
.

<http://resource.geosciml.org/classifier/cgi/geologicunitmorphology/mound>
    a skos:Concept ;
    rdfs:isDefinedBy cs: ;
    skos:altLabel
        "Kuppe"@de ,
        "cerro"@es ,
        "kumpareet"@fi ,
        "mound"@it ,
        "kholm zemlyanoj"@ru ,
        "kulle"@sv ;
    skos:broader <http://resource.geosciml.org/classifier/cgi/geologicunitmorphology/geologic_body> ;
    skos:definition "Lense like body of rock, lateral extent less than 100m, generally flat at bottom, with stratigraphic pinch out of beds (onlap) along upper sides."@en ;
    skos:historyNote "This vocabulary"@en ;
    skos:inScheme cs: ;
    skos:prefLabel "mound"@en ;
    skos:related <http://resource.geosciml.org/classifier/cgi/geologicunitmorphology/discus> ;
.

<http://resource.geosciml.org/classifier/cgi/geologicunitmorphology/pancake_ellipsoid>
    a skos:Concept ;
    rdfs:isDefinedBy cs: ;
    skos:broader <http://resource.geosciml.org/classifier/cgi/geologicunitmorphology/ellipsoid> ;
    skos:definition "Ellipsoid with H on order of .01 of L or W"@en ;
    skos:historyNote "This vocabulary"@en ;
    skos:inScheme cs: ;
    skos:prefLabel "pancake ellipsoid"@en ;
.

<http://resource.geosciml.org/classifier/cgi/geologicunitmorphology/phacolith>
    a skos:Concept ;
    rdfs:isDefinedBy cs: ;
    skos:broader <http://resource.geosciml.org/classifier/cgi/geologicunitmorphology/geologic_body> ;
    skos:definition "Concordant, lenticular intrusion, emplaced along a fold axis"@en ;
    skos:historyNote "This vocabulary"@en ;
    skos:inScheme cs: ;
    skos:prefLabel "phacolith"@en ;
    skos:related <http://resource.geosciml.org/classifier/cgi/geologicunitmorphology/longitudinal_section_of_cylinder> ;
.

<http://resource.geosciml.org/classifier/cgi/geologicunitmorphology/pillow_ellipsoid>
    a skos:Concept ;
    rdfs:isDefinedBy cs: ;
    skos:broader <http://resource.geosciml.org/classifier/cgi/geologicunitmorphology/ellipsoid> ;
    skos:definition "Ellipsoid with H on order of 0.1 of L or W"@en ;
    skos:historyNote "This vocabulary"@en ;
    skos:inScheme cs: ;
    skos:prefLabel "pillow ellipsoid"@en ;
.

<http://resource.geosciml.org/classifier/cgi/geologicunitmorphology/pipe>
    a skos:Concept ;
    rdfs:isDefinedBy cs: ;
    skos:altLabel
        "Pipe"@de ,
        "pipa"@es ,
        "piiput"@fi ,
        "tubo"@it ,
        "trubka"@ru ,
        "pipe"@sv ;
    skos:broader <http://resource.geosciml.org/classifier/cgi/geologicunitmorphology/geologic_body> ;
    skos:definition "Rock body that has a length to width ratio greater than 10 to 1, with two sub equal width dimensions."@en ;
    skos:historyNote "This vocabulary"@en ;
    skos:inScheme cs: ;
    skos:prefLabel "pipe"@en ;
.

<http://resource.geosciml.org/classifier/cgi/geologicunitmorphology/planar_sheet>
    a skos:Concept ;
    rdfs:isDefinedBy cs: ;
    skos:broader <http://resource.geosciml.org/classifier/cgi/geologicunitmorphology/sheet> ;
    skos:definition "Sheet in which L and W axes are straight lines"@en ;
    skos:historyNote "This vocabulary"@en ;
    skos:inScheme cs: ;
    skos:prefLabel "planar sheet"@en ;
.

<http://resource.geosciml.org/classifier/cgi/geologicunitmorphology/planar_vein>
    a skos:Concept ;
    rdfs:isDefinedBy cs: ;
    skos:broader <http://resource.geosciml.org/classifier/cgi/geologicunitmorphology/vein> ;
    skos:definition "Vein with length and width significantly greater than its thickness, giving the vein a tabular form"@en ;
    skos:historyNote "This vocabulary"@en ;
    skos:inScheme cs: ;
    skos:prefLabel "planar vein"@en ;
    skos:related
        <http://resource.geosciml.org/classifier/cgi/geologicunitmorphology/dike> ,
        <http://resource.geosciml.org/classifier/cgi/geologicunitmorphology/layer_shape> ;
.

<http://resource.geosciml.org/classifier/cgi/geologicunitmorphology/pod>
    a skos:Concept ;
    rdfs:isDefinedBy cs: ;
    skos:broader <http://resource.geosciml.org/classifier/cgi/geologicunitmorphology/geologic_body> ;
    skos:definition "A small intrusion of elongate or lenticular form"@en ;
    skos:historyNote "This vocabulary"@en ;
    skos:inScheme cs: ;
    skos:prefLabel "pod"@en ;
    skos:related <http://resource.geosciml.org/classifier/cgi/geologicunitmorphology/blob> ;
.

<http://resource.geosciml.org/classifier/cgi/geologicunitmorphology/ring_dyke>
    a skos:Concept ;
    rdfs:isDefinedBy cs: ;
    skos:altLabel
        "Ringdyke"@de ,
        "dique anular"@es ,
        "rengasjuonet"@fi ,
        "ring dyke"@fr ,
        "retas cincin"@id ,
        "retas melingkar"@id ,
        "filone ad anello"@it ,
        "リングダイク"@ja ,
        "環状岩脈"@ja ,
        "TMnb;TwkB½T§CuMvij"@km ,
        "환상암맥"@ko ,
        "²½Îñ¤¸ö¤Á¹¸­"@lo ,
        "korok gelang"@ms ,
        "dajka kol'tsevaya"@ru ,
        "ringgång"@sv ,
        "พนังวงแหวน"@th ,
        "thể tường dạng vòng"@vi ,
        "环状岩墙"@zh ;
    skos:broader <http://resource.geosciml.org/classifier/cgi/geologicunitmorphology/geologic_body> ;
    skos:definition "An arcuate or subcircular dyke, generally associated with a volcanic centre."@en ;
    skos:historyNote "This vocabulary"@en ;
    skos:inScheme cs: ;
    skos:prefLabel "ring dike"@en ;
    skos:related <http://resource.geosciml.org/classifier/cgi/geologicunitmorphology/arcuate_sheet> ;
.

<http://resource.geosciml.org/classifier/cgi/geologicunitmorphology/rock_body_geometry_irregular>
    a skos:Concept ;
    rdfs:isDefinedBy cs: ;
    skos:broader <http://resource.geosciml.org/classifier/cgi/geologicunitmorphology/geologic_body> ;
    skos:definition "Rock body geometry is irregular and can not be characterized using terminology."@en ;
    skos:historyNote "This vocabulary"@en ;
    skos:inScheme cs: ;
    skos:prefLabel "rock body geometry irregular"@en ;
.

<http://resource.geosciml.org/classifier/cgi/geologicunitmorphology/rock_body_geometry_not_specified>
    a skos:Concept ;
    rdfs:isDefinedBy cs: ;
    skos:broader <http://resource.geosciml.org/classifier/cgi/geologicunitmorphology/geologic_body> ;
    skos:definition "Rock body geometry is not specified. Use in normative descriptions where any morphology is allowed."@en ;
    skos:historyNote "This vocabulary"@en ;
    skos:inScheme cs: ;
    skos:prefLabel "rock body geometry not specified"@en ;
.

<http://resource.geosciml.org/classifier/cgi/geologicunitmorphology/rod>
    a skos:Concept ;
    rdfs:isDefinedBy cs: ;
    skos:broader <http://resource.geosciml.org/classifier/cgi/geologicunitmorphology/cylinder> ;
    skos:definition "Cylinder with very long axis, generally circular or elliptical cross section (generating figure). H>>>W=L. Long axis may be in any orientation, and may be curved."@en ;
    skos:historyNote "This vocabulary"@en ;
    skos:inScheme cs: ;
    skos:prefLabel "rod"@en ;
.

<http://resource.geosciml.org/classifier/cgi/geologicunitmorphology/sigmoidal_vein>
    a skos:Concept ;
    rdfs:isDefinedBy cs: ;
    skos:broader <http://resource.geosciml.org/classifier/cgi/geologicunitmorphology/vein> ;
    skos:definition "Vein curved so as to resemble the letter S in section"@en ;
    skos:historyNote "This vocabulary"@en ;
    skos:inScheme cs: ;
    skos:prefLabel "sigmoidal vein"@en ;
    skos:related <http://resource.geosciml.org/classifier/cgi/geologicunitmorphology/sigmoid_sheet> ;
.

<http://resource.geosciml.org/classifier/cgi/geologicunitmorphology/sphenolith>
    a skos:Concept ;
    rdfs:isDefinedBy cs: ;
    skos:altLabel
        "Sphenolithus"@de ,
        "esfenolito"@es ,
        "sfenoliitti"@fi ,
        "sfenolite"@it ,
        "sfenolit"@ru ,
        "sfenolit"@sv ;
    skos:broader <http://resource.geosciml.org/classifier/cgi/geologicunitmorphology/geologic_body> ;
    skos:definition "Wedge-like intrusion, partly concordant, partly discordant."@en ;
    skos:historyNote "This vocabulary"@en ;
    skos:inScheme cs: ;
    skos:prefLabel "sphenolith"@en ;
    skos:related
        <http://resource.geosciml.org/classifier/cgi/geologicunitmorphology/prism> ,
        <http://resource.geosciml.org/classifier/cgi/geologicunitmorphology/wedge> ;
.

<http://resource.geosciml.org/classifier/cgi/geologicunitmorphology/spheroid>
    a skos:Concept ;
    rdfs:isDefinedBy cs: ;
    skos:broader <http://resource.geosciml.org/classifier/cgi/geologicunitmorphology/ellipsoid> ;
    skos:definition "Ellipsoid with L, W, and H dimensions all approximately equal"@en ;
    skos:historyNote "This vocabulary"@en ;
    skos:inScheme cs: ;
    skos:prefLabel "spheroid"@en ;
.

<http://resource.geosciml.org/classifier/cgi/geologicunitmorphology/square_profile>
    a skos:Concept ;
    rdfs:isDefinedBy cs: ;
    skos:broader <http://resource.geosciml.org/classifier/cgi/geologicunitmorphology/polygonal_profile> ;
    skos:definition "polygonal profile that approximates a square"@en ;
    skos:historyNote "This vocabulary"@en ;
    skos:inScheme cs: ;
    skos:prefLabel "square profile"@en ;
.

<http://resource.geosciml.org/classifier/cgi/geologicunitmorphology/tablet>
    a skos:Concept ;
    rdfs:isDefinedBy cs: ;
    skos:broader <http://resource.geosciml.org/classifier/cgi/geologicunitmorphology/polygonal_cylinder> ;
    skos:definition "Polygonal cylinder with height less than length or width, disc with edges separating side into multiple segments."@en ;
    skos:historyNote "This vocabulary"@en ;
    skos:inScheme cs: ;
    skos:prefLabel "tablet"@en ;
.

<http://resource.geosciml.org/classifier/cgi/geologicunitmorphology/trough>
    a skos:Concept ;
    rdfs:isDefinedBy cs: ;
    skos:altLabel
        "Tiefseemulde"@de ,
        "fosa abisal alargada"@es ,
        "poimupohjat"@fi ,
        "fossa abissale allungata"@it ,
        "trog"@ru ,
        "tråg"@sv ;
    skos:broader <http://resource.geosciml.org/classifier/cgi/geologicunitmorphology/geologic_body> ;
    skos:definition "Shape of a body of sedimentary rock deposited in an elongate depression filled with sediment. large size distinguishes from channel"@en ;
    skos:historyNote "This vocabulary"@en ;
    skos:inScheme cs: ;
    skos:prefLabel "trough shape"@en ;
    skos:related <http://resource.geosciml.org/classifier/cgi/geologicunitmorphology/longitudinal_section_of_cylinder> ;
.

<http://resource.geosciml.org/classifier/cgi/geologicunitmorphology/arcuate_sheet>
    a skos:Concept ;
    rdfs:isDefinedBy cs: ;
    skos:broader <http://resource.geosciml.org/classifier/cgi/geologicunitmorphology/sheet> ;
    skos:definition "Sheet in which one of L or W is a curved arc"@en ;
    skos:historyNote "This vocabulary"@en ;
    skos:inScheme cs: ;
    skos:prefLabel "arcuate sheet"@en ;
.

<http://resource.geosciml.org/classifier/cgi/geologicunitmorphology/blanket_shape>
    a skos:Concept ;
    rdfs:isDefinedBy cs: ;
    skos:broader <http://resource.geosciml.org/classifier/cgi/geologicunitmorphology/geologic_body> ;
    skos:definition "A thin, widespread body with width to thickness ratio greater than 1000 to 1 that covers an underlying substrate. A layer of known great lateral extent. Morphology equivalent to bed or layer, but implies that body forms the top of some unit, instead of occurring within a body."@en ;
    skos:historyNote "This vocabulary"@en ;
    skos:inScheme cs: ;
    skos:prefLabel "blanket shape"@en ;
    skos:related <http://resource.geosciml.org/classifier/cgi/geologicunitmorphology/sheet> ;
.

<http://resource.geosciml.org/classifier/cgi/geologicunitmorphology/blob>
    a skos:Concept ;
    rdfs:isDefinedBy cs: ;
    skos:broader <http://resource.geosciml.org/classifier/cgi/geologicunitmorphology/three_dimensional_body> ;
    skos:definition "Body with smooth surface, broadly equant shape, irregular protuberances, no symmetry axes, and a boundary that can not be separated into sides."@en ;
    skos:historyNote "This vocabulary"@en ;
    skos:inScheme cs: ;
    skos:prefLabel "blob"@en ;
.

<http://resource.geosciml.org/classifier/cgi/geologicunitmorphology/bread_loaf_ellipsoid>
    a skos:Concept ;
    rdfs:isDefinedBy cs: ;
    skos:broader <http://resource.geosciml.org/classifier/cgi/geologicunitmorphology/ellipsoid> ;
    skos:definition "Ellipsoid with L 10 times W or H"@en ;
    skos:historyNote "This vocabulary"@en ;
    skos:inScheme cs: ;
    skos:prefLabel "bread loaf ellipsoid"@en ;
.

<http://resource.geosciml.org/classifier/cgi/geologicunitmorphology/circular_cylinder>
    a skos:Concept ;
    rdfs:isDefinedBy cs: ;
    skos:broader <http://resource.geosciml.org/classifier/cgi/geologicunitmorphology/elliptical_cylinder> ;
    skos:definition "Elliptical cylinder that has circular symmetry about long axis, distinct side surfaces are not defined. Cross section is circular"@en ;
    skos:historyNote "This vocabulary"@en ;
    skos:inScheme cs: ;
    skos:prefLabel "circular cylinder"@en ;
.

<http://resource.geosciml.org/classifier/cgi/geologicunitmorphology/cone>
    a skos:Concept ;
    rdfs:isDefinedBy cs: ;
    skos:broader <http://resource.geosciml.org/classifier/cgi/geologicunitmorphology/discus> ;
    skos:definition "Discus with one planar side, and circular symmetry on axis, geologic cones typically have height <(<) diameter"@en ;
    skos:historyNote "This vocabulary"@en ;
    skos:inScheme cs: ;
    skos:prefLabel "cone shape"@en ;
.

<http://resource.geosciml.org/classifier/cgi/geologicunitmorphology/cone_segment>
    a skos:Concept ;
    rdfs:isDefinedBy cs: ;
    skos:broader <http://resource.geosciml.org/classifier/cgi/geologicunitmorphology/three_dimensional_body> ;
    skos:definition "Body that is section of a cone formed by splitting the cone along a surface parallel to the cone axis, that interesect approximately along the axis."@en ;
    skos:historyNote "This vocabulary"@en ;
    skos:inScheme cs: ;
    skos:prefLabel "cone segment"@en ;
.

<http://resource.geosciml.org/classifier/cgi/geologicunitmorphology/diapir>
    a skos:Concept ;
    rdfs:isDefinedBy cs: ;
    skos:broader <http://resource.geosciml.org/classifier/cgi/geologicunitmorphology/geologic_body> ;
    skos:definition "Broadly inverted tear drop morphology. Body of magmatic or mobile sedimentary material intruded into overlying rocks."@en ;
    skos:historyNote "This vocabulary"@en ;
    skos:inScheme cs: ;
    skos:prefLabel "diapir"@en ;
.

<http://resource.geosciml.org/classifier/cgi/geologicunitmorphology/elliptical_cylinder>
    a skos:Concept ;
    rdfs:isDefinedBy cs: ;
    skos:broader <http://resource.geosciml.org/classifier/cgi/geologicunitmorphology/cylinder> ;
    skos:definition "Cylinder that has elliptical cross section, distinct side surfaces are not defined."@en ;
    skos:historyNote "This vocabulary"@en ;
    skos:inScheme cs: ;
    skos:narrower <http://resource.geosciml.org/classifier/cgi/geologicunitmorphology/circular_cylinder> ;
    skos:prefLabel "elliptical cylinder"@en ;
.

<http://resource.geosciml.org/classifier/cgi/geologicunitmorphology/polygonal_profile>
    a skos:Concept ;
    rdfs:isDefinedBy cs: ;
    skos:broader <http://resource.geosciml.org/classifier/cgi/geologicunitmorphology/planar_profile> ;
    skos:definition "Profile for which the ratio of length of longest chord to shortest chord is greater than 1.4.profile and a boundary that can be divided into distinct straight sides separated by higher curvature corners."@en ;
    skos:historyNote "This vocabulary"@en ;
    skos:inScheme cs: ;
    skos:prefLabel "polygonal profile"@en ;
.

<http://resource.geosciml.org/classifier/cgi/geologicunitmorphology/ribbon>
    a skos:Concept ;
    rdfs:isDefinedBy cs: ;
    skos:broader <http://resource.geosciml.org/classifier/cgi/geologicunitmorphology/three_dimensional_body> ;
    skos:definition "Body that is very thin relative to width and and length. Long axis may be curved. L>(>>)W>>>H. H is typically in vertical direction."@en ;
    skos:historyNote "This vocabulary"@en ;
    skos:inScheme cs: ;
    skos:prefLabel "ribbon"@en ;
.

<http://resource.geosciml.org/classifier/cgi/geologicunitmorphology/sigmoid_sheet>
    a skos:Concept ;
    rdfs:isDefinedBy cs: ;
    skos:broader <http://resource.geosciml.org/classifier/cgi/geologicunitmorphology/sheet> ;
    skos:definition "Sheet with 's' curvature of L or W direction"@en ;
    skos:historyNote "This vocabulary"@en ;
    skos:inScheme cs: ;
    skos:prefLabel "sigmoid sheet"@en ;
.

<http://resource.geosciml.org/classifier/cgi/geologicunitmorphology/tabular_prism>
    a skos:Concept ;
    rdfs:isDefinedBy cs: ;
    skos:broader <http://resource.geosciml.org/classifier/cgi/geologicunitmorphology/prism> ;
    skos:definition "Body defined by pairs of parallel, approximately planar surfaces separated by definable edges. Grades to ellipsoid as edges lose definition, to block as axial ratios approach 1, to polygonal cylinder as L approaches W. L>>W>H. H is in vertical direction, L is horizontal."@en ;
    skos:historyNote "This vocabulary"@en ;
    skos:inScheme cs: ;
    skos:prefLabel "tabular prism"@en ;
.

<http://resource.geosciml.org/classifier/cgi/geologicunitmorphology/tear_drop>
    a skos:Concept ;
    rdfs:isDefinedBy cs: ;
    skos:broader <http://resource.geosciml.org/classifier/cgi/geologicunitmorphology/three_dimensional_body> ;
    skos:definition "Body bounded by hemispheroid on one side, cone on other, with circular symmetry around cone axis"@en ;
    skos:historyNote "This vocabulary"@en ;
    skos:inScheme cs: ;
    skos:prefLabel "tear drop"@en ;
.

<http://resource.geosciml.org/classifier/cgi/geologicunitmorphology/dike>
    a skos:Concept ;
    rdfs:isDefinedBy cs: ;
    skos:altLabel
        "Dyke"@de ,
        "dyke"@en ,
        "dique"@es ,
        "juonet"@fi ,
        "dicco"@it ,
        "dajka"@ru ,
        "gång"@sv ;
    skos:broader <http://resource.geosciml.org/classifier/cgi/geologicunitmorphology/geologic_body> ;
    skos:definition "A generally sheet-like intrusive rock body that cuts across bedding or foliation in the host rock, or intrudes massive host rock."@en ;
    skos:historyNote "This vocabulary"@en ;
    skos:inScheme cs: ;
    skos:prefLabel "dike"@en ;
    skos:related <http://resource.geosciml.org/classifier/cgi/geologicunitmorphology/sheet> ;
.

<http://resource.geosciml.org/classifier/cgi/geologicunitmorphology/equant_profile>
    a skos:Concept ;
    rdfs:isDefinedBy cs: ;
    skos:broader <http://resource.geosciml.org/classifier/cgi/geologicunitmorphology/planar_profile> ;
    skos:definition "Profile for which the ratio of length of longest chord to shortest chord is less than 1.4."@en ;
    skos:historyNote "This vocabulary"@en ;
    skos:inScheme cs: ;
    skos:narrower
        <http://resource.geosciml.org/classifier/cgi/geologicunitmorphology/circular_profile> ,
        <http://resource.geosciml.org/classifier/cgi/geologicunitmorphology/equant_polygonal_profile> ;
    skos:prefLabel "equant profile"@en ;
.

<http://resource.geosciml.org/classifier/cgi/geologicunitmorphology/sill_form>
    a skos:Concept ;
    rdfs:isDefinedBy cs: ;
    skos:broader <http://resource.geosciml.org/classifier/cgi/geologicunitmorphology/geologic_body> ;
    skos:definition "A tabular intrusive igneous body with long dimensions parallel to bedding or foliation of sedimentary or metamorphic host rock."@en ;
    skos:historyNote "This vocabulary"@en ;
    skos:inScheme cs: ;
    skos:prefLabel "sill form"@en ;
    skos:related
        <http://resource.geosciml.org/classifier/cgi/geologicunitmorphology/layer_shape> ,
        <http://resource.geosciml.org/classifier/cgi/geologicunitmorphology/sheet> ,
        <http://resource.geosciml.org/classifier/cgi/geologicunitmorphology/sheet_ellipsoid> ;
.

<http://resource.geosciml.org/classifier/cgi/geologicunitmorphology/wedge>
    a skos:Concept ;
    rdfs:isDefinedBy cs: ;
    skos:broader <http://resource.geosciml.org/classifier/cgi/geologicunitmorphology/three_dimensional_body> ;
    skos:definition "A wedge is a polyhedron defined by two triangles and three trapezoid faces. A wedge has five faces, nine edges, and six vertices. A wedge is a subclass of the prismatoids with the base and opposite ridge in two parallel planes."@en ;
    skos:inScheme cs: ;
    skos:prefLabel "wedge"@en ;
    skos:related <http://resource.geosciml.org/classifier/cgi/geologicunitmorphology/prism> ;
    schema:citation "https://en.wikipedia.org/wiki/Wedge_(geometry)"^^xsd:anyURI ;
.

<http://resource.geosciml.org/classifier/cgi/geologicunitmorphology/hemispheroid>
    a skos:Concept ;
    rdfs:isDefinedBy cs: ;
    skos:broader <http://resource.geosciml.org/classifier/cgi/geologicunitmorphology/three_dimensional_body> ;
    skos:definition "Section of a spheroid formed by removing everything on the smaller volume side of a surface that intersects the spheroid. Grades to cone as suface generator (line rotated about axis to generate volume above lower planar boundary) becomes straight."@en ;
    skos:historyNote "This vocabulary"@en ;
    skos:inScheme cs: ;
    skos:prefLabel "hemispheroid"@en ;
.

<http://resource.geosciml.org/classifier/cgi/geologicunitmorphology/layer_shape>
    a skos:Concept ;
    rdfs:isDefinedBy cs: ;
    skos:altLabel
        "Schicht"@de ,
        "estrato"@es ,
        "kerrokset"@fi ,
        "strato"@it ,
        "sloj"@ru ,
        "lager"@sv ;
    skos:broader <http://resource.geosciml.org/classifier/cgi/geologicunitmorphology/geologic_body> ;
    skos:definition "Body geometry characterized by generally thin character relative to the lateral extent of the body (on order of 1:100). Thin bodies of lesser extent are lenses. Connotes a non-intrusive body, equivalent intrusive body would be dike (or sill). Denotes that body is in a sequence of similar sheet-like bodies between other rock bodies"@en ;
    skos:historyNote "This vocabulary"@en ;
    skos:inScheme cs: ;
    skos:prefLabel "layer shape"@en ;
    skos:related
        <http://resource.geosciml.org/classifier/cgi/geologicunitmorphology/blanket_shape> ,
        <http://resource.geosciml.org/classifier/cgi/geologicunitmorphology/sill_form> ;
.

<http://resource.geosciml.org/classifier/cgi/geologicunitmorphology/polygonal_cylinder>
    a skos:Concept ;
    rdfs:isDefinedBy cs: ;
    skos:broader <http://resource.geosciml.org/classifier/cgi/geologicunitmorphology/cylinder> ;
    skos:definition "Cylinder in which the edges bounding side surfaces are parallel or subparallel to cylinder axis. Cross section is polygon. Length of axis may be called height or thickness, and is typically in the vertical direction (distinguishing polygonal cylinder from tabular prism and wedge)."@en ;
    skos:historyNote "This vocabulary"@en ;
    skos:inScheme cs: ;
    skos:narrower
        <http://resource.geosciml.org/classifier/cgi/geologicunitmorphology/block> ,
        <http://resource.geosciml.org/classifier/cgi/geologicunitmorphology/square_profile> ,
        <http://resource.geosciml.org/classifier/cgi/geologicunitmorphology/tablet> ;
    skos:prefLabel "polygonal cylinder"@en ;
.

<http://resource.geosciml.org/classifier/cgi/geologicunitmorphology/prism>
    a skos:Concept ;
    rdfs:isDefinedBy cs: ;
    skos:broader <http://resource.geosciml.org/classifier/cgi/geologicunitmorphology/three_dimensional_body> ;
    skos:definition "A polyhedron with an n-sided polygonal base, another congruent parallel base (with the same rotational orientation), and n other faces (necessarily all parallelograms) joining corresponding sides of the two bases. All cross-sections parallel to the base faces are congruent to the bases. Prisms are named for their base, so a prism with a pentagonal base is called a pentagonal prism."@en ;
    skos:inScheme cs: ;
    skos:narrower <http://resource.geosciml.org/classifier/cgi/geologicunitmorphology/tabular_prism> ;
    skos:prefLabel "prism"@en ;
    skos:related <http://resource.geosciml.org/classifier/cgi/geologicunitmorphology/wedge> ;
    schema:citation "https://en.wikipedia.org/wiki/Prism_(geometry)"^^xsd:anyURI ;
.

<http://resource.geosciml.org/classifier/cgi/geologicunitmorphology/sheet_ellipsoid>
    a skos:Concept ;
    rdfs:isDefinedBy cs: ;
    skos:broader <http://resource.geosciml.org/classifier/cgi/geologicunitmorphology/ellipsoid> ;
    skos:definition "Ellipsoid with one axis much smaller than others H on order of .001 of L or W"@en ;
    skos:historyNote "This vocabulary"@en ;
    skos:inScheme cs: ;
    skos:prefLabel "sheet ellipsoid"@en ;
.

<http://resource.geosciml.org/classifier/cgi/geologicunitmorphology/vein>
    a skos:Concept ;
    rdfs:isDefinedBy cs: ;
    skos:broader <http://resource.geosciml.org/classifier/cgi/geologicunitmorphology/geologic_body> ;
    skos:definition "A tabular or sheetlike epigenetic mineral filling of a fault or fracture"@en ;
    skos:historyNote "This vocabulary"@en ;
    skos:inScheme cs: ;
    skos:narrower
        <http://resource.geosciml.org/classifier/cgi/geologicunitmorphology/planar_vein> ,
        <http://resource.geosciml.org/classifier/cgi/geologicunitmorphology/sigmoidal_vein> ;
    skos:prefLabel "vein-shape"@en ;
    skos:related <http://resource.geosciml.org/classifier/cgi/geologicunitmorphology/sheet> ;
.

<http://resource.geosciml.org/classifier/cgi/geologicunitmorphology/cylinder>
    a skos:Concept ;
    rdfs:isDefinedBy cs: ;
    skos:broader <http://resource.geosciml.org/classifier/cgi/geologicunitmorphology/three_dimensional_body> ;
    skos:definition "Body defined by translation of a generating plane figure with approximately equant cross section (circle, ellipsoid, polygon) along a straight axial line. H>=W=L. Axis is direction normal to generating plane figure, which forms parallel top and bottom bounding surface."@en ;
    skos:historyNote "This vocabulary"@en ;
    skos:inScheme cs: ;
    skos:narrower
        <http://resource.geosciml.org/classifier/cgi/geologicunitmorphology/disc> ,
        <http://resource.geosciml.org/classifier/cgi/geologicunitmorphology/elliptical_cylinder> ,
        <http://resource.geosciml.org/classifier/cgi/geologicunitmorphology/polygonal_cylinder> ,
        <http://resource.geosciml.org/classifier/cgi/geologicunitmorphology/rod> ;
    skos:prefLabel "cylinder"@en ;
.

<http://resource.geosciml.org/classifier/cgi/geologicunitmorphology/longitudinal_section_of_cylinder>
    a skos:Concept ;
    rdfs:isDefinedBy cs: ;
    skos:broader <http://resource.geosciml.org/classifier/cgi/geologicunitmorphology/three_dimensional_body> ;
    skos:definition "Body that is section of a circular or elliptical cylinder formed by a splitting the cylinder along a surface approximately parallel to its long axis. L>>W>H."@en ;
    skos:historyNote "This vocabulary"@en ;
    skos:inScheme cs: ;
    skos:prefLabel "longitudinal section of cylinder"@en ;
.

<http://resource.geosciml.org/classifier/cgi/geologicunitmorphology/planar_profile>
    a skos:Concept ;
    rdfs:isDefinedBy cs: ;
    skos:definition "Shape is defined by intersection of body with some surface, generally either a cross section or map view"@en ;
    skos:historyNote "This vocabulary"@en ;
    skos:inScheme cs: ;
    skos:narrower
        <http://resource.geosciml.org/classifier/cgi/geologicunitmorphology/elliptical_profile> ,
        <http://resource.geosciml.org/classifier/cgi/geologicunitmorphology/equant_profile> ,
        <http://resource.geosciml.org/classifier/cgi/geologicunitmorphology/irregular_profile> ,
        <http://resource.geosciml.org/classifier/cgi/geologicunitmorphology/lenticular_profile> ,
        <http://resource.geosciml.org/classifier/cgi/geologicunitmorphology/polygonal_profile> ;
    skos:prefLabel "planar profile"@en ;
    skos:topConceptOf cs: ;
.

<http://resource.geosciml.org/classifier/cgi/geologicunitmorphology/discus>
    a skos:Concept ;
    rdfs:isDefinedBy cs: ;
    skos:broader <http://resource.geosciml.org/classifier/cgi/geologicunitmorphology/three_dimensional_body> ;
    skos:definition "Body with two sides that converge to define an edge that is circular in profile, edge separates definable top and bottom. L=W>H. Grades to oblate ellipsoid as edge separating sides loses definition, cone as one side becomes distinctly planar."@en ;
    skos:historyNote "This vocabulary"@en ;
    skos:inScheme cs: ;
    skos:narrower
        <http://resource.geosciml.org/classifier/cgi/geologicunitmorphology/cone> ,
        <http://resource.geosciml.org/classifier/cgi/geologicunitmorphology/elongate_discus> ;
    skos:prefLabel "discus"@en ;
.

<http://resource.geosciml.org/classifier/cgi/geologicunitmorphology/ellipsoid>
    a skos:Concept ;
    rdfs:isDefinedBy cs: ;
    skos:broader <http://resource.geosciml.org/classifier/cgi/geologicunitmorphology/three_dimensional_body> ;
    skos:definition "Body that contains three orthogonal axes defining three surfaces of reflection symmetry, profiles along the surfaces are elliptical. Boundary can not be separated into sides (no edges). Becomes cylinder or disc when bounding surface can be considered parallel to one of the axis. L>=W>=H"@en ;
    skos:historyNote "This vocabulary"@en ;
    skos:inScheme cs: ;
    skos:narrower
        <http://resource.geosciml.org/classifier/cgi/geologicunitmorphology/bread_loaf_ellipsoid> ,
        <http://resource.geosciml.org/classifier/cgi/geologicunitmorphology/dart_ellipsoid> ,
        <http://resource.geosciml.org/classifier/cgi/geologicunitmorphology/football_ellipsoid> ,
        <http://resource.geosciml.org/classifier/cgi/geologicunitmorphology/pancake_ellipsoid> ,
        <http://resource.geosciml.org/classifier/cgi/geologicunitmorphology/pillow_ellipsoid> ,
        <http://resource.geosciml.org/classifier/cgi/geologicunitmorphology/sheet_ellipsoid> ,
        <http://resource.geosciml.org/classifier/cgi/geologicunitmorphology/spheroid> ;
    skos:prefLabel "ellipsoid"@en ;
.

<http://resource.geosciml.org/classifier/cgi/geologicunitmorphology/sheet>
    a skos:Concept ;
    rdfs:isDefinedBy cs: ;
    skos:broader <http://resource.geosciml.org/classifier/cgi/geologicunitmorphology/three_dimensional_body> ;
    skos:definition "Body that is very thin relative to lateral extent, so thin that is considered to consist of two bounding surfaces joined at an edge. Aspect ratio is L=W>>>H. The geometry of the edge joining the surfaces is not specified in the definition. If the geometry of the edge comes into play in the definition, becomes ribbon, disc or tablet(?). Includes dike, vein, sill and bed-shaped geologic units."@en ;
    skos:historyNote "This vocabulary"@en ;
    skos:inScheme cs: ;
    skos:narrower
        <http://resource.geosciml.org/classifier/cgi/geologicunitmorphology/arcuate_sheet> ,
        <http://resource.geosciml.org/classifier/cgi/geologicunitmorphology/conical_sheet> ,
        <http://resource.geosciml.org/classifier/cgi/geologicunitmorphology/dome_sheet> ,
        <http://resource.geosciml.org/classifier/cgi/geologicunitmorphology/planar_sheet> ,
        <http://resource.geosciml.org/classifier/cgi/geologicunitmorphology/sigmoid_sheet> ;
    skos:prefLabel "sheet"@en ;
    skos:related
        <http://resource.geosciml.org/classifier/cgi/geologicunitmorphology/dike> ,
        <http://resource.geosciml.org/classifier/cgi/geologicunitmorphology/layer_shape> ,
        <http://resource.geosciml.org/classifier/cgi/geologicunitmorphology/sill_form> ,
        <http://resource.geosciml.org/classifier/cgi/geologicunitmorphology/vein> ;
.

<http://resource.geosciml.org/classifier/cgi/geologicunitmorphology/three_dimensional_body>
    a skos:Concept ;
    rdfs:isDefinedBy cs: ;
    skos:definition "Any three dimensional body"@en ;
    skos:historyNote "This vocabulary"@en ;
    skos:inScheme cs: ;
    skos:narrower
        <http://resource.geosciml.org/classifier/cgi/geologicunitmorphology/blob> ,
        <http://resource.geosciml.org/classifier/cgi/geologicunitmorphology/cone_segment> ,
        <http://resource.geosciml.org/classifier/cgi/geologicunitmorphology/cylinder> ,
        <http://resource.geosciml.org/classifier/cgi/geologicunitmorphology/discoid_anulus> ,
        <http://resource.geosciml.org/classifier/cgi/geologicunitmorphology/discus> ,
        <http://resource.geosciml.org/classifier/cgi/geologicunitmorphology/ellipsoid> ,
        <http://resource.geosciml.org/classifier/cgi/geologicunitmorphology/geologic_body> ,
        <http://resource.geosciml.org/classifier/cgi/geologicunitmorphology/hemispheroid> ,
        <http://resource.geosciml.org/classifier/cgi/geologicunitmorphology/longitudinal_section_of_cylinder> ,
        <http://resource.geosciml.org/classifier/cgi/geologicunitmorphology/prism> ,
        <http://resource.geosciml.org/classifier/cgi/geologicunitmorphology/ribbon> ,
        <http://resource.geosciml.org/classifier/cgi/geologicunitmorphology/sheet> ,
        <http://resource.geosciml.org/classifier/cgi/geologicunitmorphology/tear_drop> ,
        <http://resource.geosciml.org/classifier/cgi/geologicunitmorphology/wedge> ;
    skos:prefLabel "three dimensional body"@en ;
    skos:topConceptOf cs: ;
.

<http://resource.geosciml.org/classifier/cgi/geologicunitmorphology/geologic_body>
    a skos:Concept ;
    rdfs:isDefinedBy cs: ;
    skos:broader <http://resource.geosciml.org/classifier/cgi/geologicunitmorphology/three_dimensional_body> ;
    skos:definition "A 3 dimensional body defined based on geometric shape, with some geologic connotation or denotation."@en ;
    skos:historyNote "This vocabulary"@en ;
    skos:inScheme cs: ;
    skos:narrower
        <http://resource.geosciml.org/classifier/cgi/geologicunitmorphology/arch_morphology> ,
        <http://resource.geosciml.org/classifier/cgi/geologicunitmorphology/basin_shape> ,
        <http://resource.geosciml.org/classifier/cgi/geologicunitmorphology/blanket_shape> ,
        <http://resource.geosciml.org/classifier/cgi/geologicunitmorphology/boudin_shape> ,
        <http://resource.geosciml.org/classifier/cgi/geologicunitmorphology/channel_shape> ,
        <http://resource.geosciml.org/classifier/cgi/geologicunitmorphology/column_shape> ,
        <http://resource.geosciml.org/classifier/cgi/geologicunitmorphology/cupola> ,
        <http://resource.geosciml.org/classifier/cgi/geologicunitmorphology/diapir> ,
        <http://resource.geosciml.org/classifier/cgi/geologicunitmorphology/dike> ,
        <http://resource.geosciml.org/classifier/cgi/geologicunitmorphology/dome> ,
        <http://resource.geosciml.org/classifier/cgi/geologicunitmorphology/ductolith> ,
        <http://resource.geosciml.org/classifier/cgi/geologicunitmorphology/ethmolith> ,
        <http://resource.geosciml.org/classifier/cgi/geologicunitmorphology/fan> ,
        <http://resource.geosciml.org/classifier/cgi/geologicunitmorphology/graben_shape> ,
        <http://resource.geosciml.org/classifier/cgi/geologicunitmorphology/laccolith> ,
        <http://resource.geosciml.org/classifier/cgi/geologicunitmorphology/layer_shape> ,
        <http://resource.geosciml.org/classifier/cgi/geologicunitmorphology/lens> ,
        <http://resource.geosciml.org/classifier/cgi/geologicunitmorphology/lopolith> ,
        <http://resource.geosciml.org/classifier/cgi/geologicunitmorphology/mound> ,
        <http://resource.geosciml.org/classifier/cgi/geologicunitmorphology/phacolith> ,
        <http://resource.geosciml.org/classifier/cgi/geologicunitmorphology/pipe> ,
        <http://resource.geosciml.org/classifier/cgi/geologicunitmorphology/pod> ,
        <http://resource.geosciml.org/classifier/cgi/geologicunitmorphology/ring_dyke> ,
        <http://resource.geosciml.org/classifier/cgi/geologicunitmorphology/rock_body_geometry_irregular> ,
        <http://resource.geosciml.org/classifier/cgi/geologicunitmorphology/rock_body_geometry_not_specified> ,
        <http://resource.geosciml.org/classifier/cgi/geologicunitmorphology/sill_form> ,
        <http://resource.geosciml.org/classifier/cgi/geologicunitmorphology/sphenolith> ,
        <http://resource.geosciml.org/classifier/cgi/geologicunitmorphology/trough> ,
        <http://resource.geosciml.org/classifier/cgi/geologicunitmorphology/vein> ;
    skos:prefLabel "geologic body"@en ;
.

cs:
    a skos:ConceptScheme ;
    skos:changeNote
        "2010-02-11 Add narrower relationship links by adding skos:narrower link in Protege, defining skos:narrower as inverse of skos:broader, calculating with Pellet reasoner to add inferred axioms, and using 'file/Export inferred axioms as ontology' in Protege."@en ,
        "2010-11-28 SMR: replace URN with http URI according to CGI URI scheme (see https://www.seegrid.csiro.au/wiki/bin/view/CGIModel/PersistentIdentifiersInGeoSciMLServices) to make version 201202"@en ,
        "2012-02-07 SMR: update URI to replace numeric final token with English-language string as in original URN scheme."@en ,
        "2012-02-27 SMR: add skos:exactMatch triples to map URIs for concepts in this vocabulary to number-token URIs in 201012 version of same concepts."@en ,
        "2012-11-24 SMR: Update to 201211 version; add collection entity, check all pref labels are lower case, remove owl:NamedIndividual and Owl:Thing rdf:types."@en ,
        "2016-11-21 OLR: regenerate SKOS-RDF file as part of migration to new vocabulary server. No changes to terms. Minor corrections to hierarchy from the previous 2012 version."@en ,
        "2020-06-23 NJC: Added properties to ensure vocab matched Geoscience Australia's vocab profile (http://linked.data.gov.au/def/ga-skos-profile). Just annotation properties, no new content. Agents (creator/publisher) now not text but RDF resource. Dates (create/modified) derived from editorial notes & existing date properties."@en ,
        "2021-12-17 R.Heaven: BGS Added prefLabel and altLabel in non English languages, obtained from previously determined alignments between @en labels in CGI and Multi-lingual Thesaurus of Geosciences (MulTG) and Asian Multi-lingual Thesaurus of Geosciences (AMTG). Note that specific language packs are required to render the fonts.  Known issues: @lo and @fi labels were incorrectly encoded in the digitised source datasets; they have been included regardless of this in case the encoding can be corrected."@en ,
        "2024-10-16 NJC: update to be VocPub 4.10 valid"@en ;
    skos:definition "This scheme specifies concepts that describe the geometry or form of a geologic unit, as defined by the IUGS Commission for Geoscience Information (CGI) Geoscience Terminology Working Group. Examples include: dike (dyke), cone, fan, sheet, etc. Morphology is independent of the material that composes the geologic unit. By extension, this vocabulary includes all concepts in this conceptScheme, as well as concepts in any previous versions of the scheme."@en ;
    skos:editorialNote "This file contains the 2016 SKOS-RDF version of the CGI Geologic Unit Morphology vocabulary. Compilation and review in MS Excel spreadsheet, converted to MS Excel for SKOS generation using SKOS_for_GA_from_XLS_2016.03.xslt"@en ;
    skos:hasTopConcept
        <http://resource.geosciml.org/classifier/cgi/geologicunitmorphology/planar_profile> ,
        <http://resource.geosciml.org/classifier/cgi/geologicunitmorphology/three_dimensional_body> ;
    skos:historyNote "Original set of terms from the GeosciML standard" ;
    skos:prefLabel "Geologic Unit Morphology"@en ;
    schema:citation "http://www.opengis.net/doc/geosciml/4.1"^^xsd:anyURI ;
    schema:creator <https://linked.data.gov.au/org/cgi-gtwg> ;
    schema:dateCreated "2010-02-11"^^xsd:date ;
    schema:dateModified "2020-06-23"^^xsd:date ;
    schema:publisher <https://linked.data.gov.au/org/cgi> ;
.
