@prefix dcterms: <http://purl.org/dc/terms/> .
@prefix dt: <http://resource.geosciml.org/datatype/> .
@prefix rdf: <http://www.w3.org/1999/02/22-rdf-syntax-ns#> .
@prefix rdfs: <http://www.w3.org/2000/01/rdf-schema#> .
@prefix schema: <https://schema.org/> .
@prefix skos: <http://www.w3.org/2004/02/skos/core#> .
@prefix xml: <http://www.w3.org/XML/1998/namespace> .
@prefix xsd: <http://www.w3.org/2001/XMLSchema#> .

<https://linked.data.gov.au/org/cgi-gtwg> a schema:Organization ;
    schema:affiliation <https://linked.data.gov.au/org/cgi> ;
    schema:name "CGI Geoscience Terminology Working Group" ;
    schema:url "http://www.cgi-iugs.org/tech_collaboration/geoscience_terminology_working_group.html"^^xsd:anyURI .


<https://linked.data.gov.au/org/cgi> a schema:Organization ;
    schema:name "Commission for the Management and Application of Geoscience Information" ;
    schema:url "http://www.cgi-iugs.org"^^xsd:anyURI .


<http://resource.geosciml.org/classifierscheme/cgi/2016.01/geologicunitmorphology> a skos:ConceptScheme ;
    schema:keywords "GeoSciML" ;
    dcterms:created "2010-02-11"^^xsd:date ;
    dcterms:creator <https://linked.data.gov.au/org/cgi-gtwg> ;
    dcterms:modified "2020-06-23"^^xsd:date ;
    dcterms:provenance "Original set of terms from the GeosciML standard" ;
    dcterms:publisher <https://linked.data.gov.au/org/cgi> ;
    dcterms:source "http://www.opengis.net/doc/geosciml/4.1"^^xsd:anyURI ;
    skos:changeNote "2010-02-11 Add narrower relationship links by adding skos:narrower link in Protege, defining skos:narrower as inverse of skos:broader, calculating with Pellet reasoner to add inferred axioms, and using 'file/Export inferred axioms as ontology' in Protege."@en,
        "2010-11-28 SMR replace URN with http URI according to CGI URI scheme (see https://www.seegrid.csiro.au/wiki/bin/view/CGIModel/PersistentIdentifiersInGeoSciMLServices) to make version 201202"@en,
        "2012-02-07 SMR update URI to replace numeric final token with English-language string as in original URN scheme."@en,
        "2012-02-27 SMR add skos:exactMatch triples to map URIs for concepts in this vocabulary to number-token URIs in 201012 version of same concepts."@en,
        "2012-11-24 SMR Update to 201211 version; add collection entity, check all pref labels are lower case, remove owl:NamedIndividual and Owl:Thing rdf:types."@en,
        "2016-11-21 OLR regenerate SKOS-RDF file as part of migration to new vocabulary server. No changes to terms. Minor corrections to hierarchy from the previous 2012 version."@en,
        "2020-06-23 NJC Added properties to ensure vocab matched Geoscience Australia's vocab profile (http://linked.data.gov.au/def/ga-skos-profile). Just annotation properties, no new content. Agents (creator/publisher) now not text but RDF resource. Dates (create/modified) derived from editorial notes & existing date properties."@en,
        "2021-12-17 R.Heaven BGS Added prefLabel and altLabel in non English languages, obtained from previously determined alignments between @en labels in CGI and Multi-lingual Thesaurus of Geosciences (MulTG) and Asian Multi-lingual Thesaurus of Geosciences (AMTG). Note that specific language packs are required to render the fonts.  Known issues: @lo and @fi labels were incorrectly encoded in the digitised source datasets; they have been included regardless of this in case the encoding can be corrected."@en ;
    skos:definition "This scheme specifies concepts that describe the geometry or form of a geologic unit, as defined by the IUGS Commission for Geoscience Information (CGI) Geoscience Terminology Working Group. Examples include: dike (dyke), cone, fan, sheet, etc. Morphology is independent of the material that composes the geologic unit. By extension, this vocabulary includes all concepts in this conceptScheme, as well as concepts in any previous versions of the scheme."@en ;
    skos:editorialNote "This file contains the 2016 SKOS-RDF version of the CGI Geologic Unit Morphology vocabulary. Compilation and review in MS Excel spreadsheet, converted to MS Excel for SKOS generation using SKOS_for_GA_from_XLS_2016.03.xslt"@en ;
    skos:hasTopConcept <http://resource.geosciml.org/classifier/cgi/geologicunitmorphology/planar_profile>,
        <http://resource.geosciml.org/classifier/cgi/geologicunitmorphology/three_dimensional_body> ;
    skos:prefLabel "Geologic Unit Morphology"@en .


<http://resource.geosciml.org/classifier/cgi/geologicunitmorphology> a skos:Collection ;
    dcterms:provenance "this vocabulary" ;
    skos:definition "All Concepts in this vocabulary" ;
    skos:member <http://resource.geosciml.org/classifier/cgi/geologicunitmorphology/arch_morphology>,
        <http://resource.geosciml.org/classifier/cgi/geologicunitmorphology/arcuate_sheet>,
        <http://resource.geosciml.org/classifier/cgi/geologicunitmorphology/basin_shape>,
        <http://resource.geosciml.org/classifier/cgi/geologicunitmorphology/blanket_shape>,
        <http://resource.geosciml.org/classifier/cgi/geologicunitmorphology/blob>,
        <http://resource.geosciml.org/classifier/cgi/geologicunitmorphology/block>,
        <http://resource.geosciml.org/classifier/cgi/geologicunitmorphology/boudin_shape>,
        <http://resource.geosciml.org/classifier/cgi/geologicunitmorphology/bread_loaf_ellipsoid>,
        <http://resource.geosciml.org/classifier/cgi/geologicunitmorphology/channel_shape>,
        <http://resource.geosciml.org/classifier/cgi/geologicunitmorphology/circular_cylinder>,
        <http://resource.geosciml.org/classifier/cgi/geologicunitmorphology/circular_profile>,
        <http://resource.geosciml.org/classifier/cgi/geologicunitmorphology/column_shape>,
        <http://resource.geosciml.org/classifier/cgi/geologicunitmorphology/cone>,
        <http://resource.geosciml.org/classifier/cgi/geologicunitmorphology/cone_segment>,
        <http://resource.geosciml.org/classifier/cgi/geologicunitmorphology/conical_sheet>,
        <http://resource.geosciml.org/classifier/cgi/geologicunitmorphology/cupola>,
        <http://resource.geosciml.org/classifier/cgi/geologicunitmorphology/cylinder>,
        <http://resource.geosciml.org/classifier/cgi/geologicunitmorphology/dart_ellipsoid>,
        <http://resource.geosciml.org/classifier/cgi/geologicunitmorphology/diapir>,
        <http://resource.geosciml.org/classifier/cgi/geologicunitmorphology/dike>,
        <http://resource.geosciml.org/classifier/cgi/geologicunitmorphology/disc>,
        <http://resource.geosciml.org/classifier/cgi/geologicunitmorphology/discoid_anulus>,
        <http://resource.geosciml.org/classifier/cgi/geologicunitmorphology/discus>,
        <http://resource.geosciml.org/classifier/cgi/geologicunitmorphology/dome>,
        <http://resource.geosciml.org/classifier/cgi/geologicunitmorphology/dome_sheet>,
        <http://resource.geosciml.org/classifier/cgi/geologicunitmorphology/ductolith>,
        <http://resource.geosciml.org/classifier/cgi/geologicunitmorphology/ellipsoid>,
        <http://resource.geosciml.org/classifier/cgi/geologicunitmorphology/elliptical_cylinder>,
        <http://resource.geosciml.org/classifier/cgi/geologicunitmorphology/elliptical_profile>,
        <http://resource.geosciml.org/classifier/cgi/geologicunitmorphology/elongate_discus>,
        <http://resource.geosciml.org/classifier/cgi/geologicunitmorphology/equant_polygonal_profile>,
        <http://resource.geosciml.org/classifier/cgi/geologicunitmorphology/equant_profile>,
        <http://resource.geosciml.org/classifier/cgi/geologicunitmorphology/ethmolith>,
        <http://resource.geosciml.org/classifier/cgi/geologicunitmorphology/fan>,
        <http://resource.geosciml.org/classifier/cgi/geologicunitmorphology/football_ellipsoid>,
        <http://resource.geosciml.org/classifier/cgi/geologicunitmorphology/geologic_body>,
        <http://resource.geosciml.org/classifier/cgi/geologicunitmorphology/graben_shape>,
        <http://resource.geosciml.org/classifier/cgi/geologicunitmorphology/hemispheroid>,
        <http://resource.geosciml.org/classifier/cgi/geologicunitmorphology/irregular_profile>,
        <http://resource.geosciml.org/classifier/cgi/geologicunitmorphology/laccolith>,
        <http://resource.geosciml.org/classifier/cgi/geologicunitmorphology/layer_shape>,
        <http://resource.geosciml.org/classifier/cgi/geologicunitmorphology/lens>,
        <http://resource.geosciml.org/classifier/cgi/geologicunitmorphology/lenticular_profile>,
        <http://resource.geosciml.org/classifier/cgi/geologicunitmorphology/longitudinal_section_of_cylinder>,
        <http://resource.geosciml.org/classifier/cgi/geologicunitmorphology/lopolith>,
        <http://resource.geosciml.org/classifier/cgi/geologicunitmorphology/mound>,
        <http://resource.geosciml.org/classifier/cgi/geologicunitmorphology/pancake_ellipsoid>,
        <http://resource.geosciml.org/classifier/cgi/geologicunitmorphology/phacolith>,
        <http://resource.geosciml.org/classifier/cgi/geologicunitmorphology/pillow_ellipsoid>,
        <http://resource.geosciml.org/classifier/cgi/geologicunitmorphology/pipe>,
        <http://resource.geosciml.org/classifier/cgi/geologicunitmorphology/planar_profile>,
        <http://resource.geosciml.org/classifier/cgi/geologicunitmorphology/planar_sheet>,
        <http://resource.geosciml.org/classifier/cgi/geologicunitmorphology/planar_vein>,
        <http://resource.geosciml.org/classifier/cgi/geologicunitmorphology/pod>,
        <http://resource.geosciml.org/classifier/cgi/geologicunitmorphology/polygonal_cylinder>,
        <http://resource.geosciml.org/classifier/cgi/geologicunitmorphology/polygonal_profile>,
        <http://resource.geosciml.org/classifier/cgi/geologicunitmorphology/prism>,
        <http://resource.geosciml.org/classifier/cgi/geologicunitmorphology/ribbon>,
        <http://resource.geosciml.org/classifier/cgi/geologicunitmorphology/ring_dyke>,
        <http://resource.geosciml.org/classifier/cgi/geologicunitmorphology/rock_body_geometry_irregular>,
        <http://resource.geosciml.org/classifier/cgi/geologicunitmorphology/rock_body_geometry_not_specified>,
        <http://resource.geosciml.org/classifier/cgi/geologicunitmorphology/rod>,
        <http://resource.geosciml.org/classifier/cgi/geologicunitmorphology/sheet>,
        <http://resource.geosciml.org/classifier/cgi/geologicunitmorphology/sheet_ellipsoid>,
        <http://resource.geosciml.org/classifier/cgi/geologicunitmorphology/sigmoid_sheet>,
        <http://resource.geosciml.org/classifier/cgi/geologicunitmorphology/sigmoidal_vein>,
        <http://resource.geosciml.org/classifier/cgi/geologicunitmorphology/sill_form>,
        <http://resource.geosciml.org/classifier/cgi/geologicunitmorphology/sphenolith>,
        <http://resource.geosciml.org/classifier/cgi/geologicunitmorphology/spheroid>,
        <http://resource.geosciml.org/classifier/cgi/geologicunitmorphology/square_profile>,
        <http://resource.geosciml.org/classifier/cgi/geologicunitmorphology/tablet>,
        <http://resource.geosciml.org/classifier/cgi/geologicunitmorphology/tabular_prism>,
        <http://resource.geosciml.org/classifier/cgi/geologicunitmorphology/tear_drop>,
        <http://resource.geosciml.org/classifier/cgi/geologicunitmorphology/three_dimensional_body>,
        <http://resource.geosciml.org/classifier/cgi/geologicunitmorphology/trough>,
        <http://resource.geosciml.org/classifier/cgi/geologicunitmorphology/vein>,
        <http://resource.geosciml.org/classifier/cgi/geologicunitmorphology/wedge> ;
    skos:prefLabel "Geologic Unit Morphology - All Concepts"@en .


<http://resource.geosciml.org/classifier/cgi/geologicunitmorphology/planar_profile> a skos:Concept ;
    dcterms:provenance "This vocabulary"@en ;
    rdfs:isDefinedBy <http://resource.geosciml.org/classifierscheme/cgi/2016.01/geologicunitmorphology> ;
    skos:definition "Shape is defined by intersection of body with some surface, generally either a cross section or map view"@en ;
    skos:inScheme <http://resource.geosciml.org/classifierscheme/cgi/2016.01/geologicunitmorphology> ;
    skos:narrower <http://resource.geosciml.org/classifier/cgi/geologicunitmorphology/elliptical_profile>,
        <http://resource.geosciml.org/classifier/cgi/geologicunitmorphology/equant_profile>,
        <http://resource.geosciml.org/classifier/cgi/geologicunitmorphology/irregular_profile>,
        <http://resource.geosciml.org/classifier/cgi/geologicunitmorphology/lenticular_profile>,
        <http://resource.geosciml.org/classifier/cgi/geologicunitmorphology/polygonal_profile> ;
    skos:prefLabel "planar profile"@en ;
    skos:topConceptOf <http://resource.geosciml.org/classifierscheme/cgi/2016.01/geologicunitmorphology> .


<http://resource.geosciml.org/classifier/cgi/geologicunitmorphology/three_dimensional_body> a skos:Concept ;
    dcterms:provenance "This vocabulary"@en ;
    rdfs:isDefinedBy <http://resource.geosciml.org/classifierscheme/cgi/2016.01/geologicunitmorphology> ;
    skos:definition "Any three dimensional body"@en ;
    skos:inScheme <http://resource.geosciml.org/classifierscheme/cgi/2016.01/geologicunitmorphology> ;
    skos:narrower <http://resource.geosciml.org/classifier/cgi/geologicunitmorphology/blob>,
        <http://resource.geosciml.org/classifier/cgi/geologicunitmorphology/cone_segment>,
        <http://resource.geosciml.org/classifier/cgi/geologicunitmorphology/cylinder>,
        <http://resource.geosciml.org/classifier/cgi/geologicunitmorphology/discoid_anulus>,
        <http://resource.geosciml.org/classifier/cgi/geologicunitmorphology/discus>,
        <http://resource.geosciml.org/classifier/cgi/geologicunitmorphology/ellipsoid>,
        <http://resource.geosciml.org/classifier/cgi/geologicunitmorphology/geologic_body>,
        <http://resource.geosciml.org/classifier/cgi/geologicunitmorphology/hemispheroid>,
        <http://resource.geosciml.org/classifier/cgi/geologicunitmorphology/longitudinal_section_of_cylinder>,
        <http://resource.geosciml.org/classifier/cgi/geologicunitmorphology/prism>,
        <http://resource.geosciml.org/classifier/cgi/geologicunitmorphology/ribbon>,
        <http://resource.geosciml.org/classifier/cgi/geologicunitmorphology/sheet>,
        <http://resource.geosciml.org/classifier/cgi/geologicunitmorphology/tear_drop>,
        <http://resource.geosciml.org/classifier/cgi/geologicunitmorphology/wedge> ;
    skos:prefLabel "three dimensional body"@en ;
    skos:topConceptOf <http://resource.geosciml.org/classifierscheme/cgi/2016.01/geologicunitmorphology> .


<http://resource.geosciml.org/classifier/cgi/geologicunitmorphology/arch_morphology> a skos:Concept ;
    dcterms:provenance "This vocabulary"@en ;
    rdfs:isDefinedBy <http://resource.geosciml.org/classifierscheme/cgi/2016.01/geologicunitmorphology> ;
    skos:broader <http://resource.geosciml.org/classifier/cgi/geologicunitmorphology/geologic_body> ;
    skos:definition "A raised elongate body, morphologically equivalent to upside down channel"@en ;
    skos:inScheme <http://resource.geosciml.org/classifierscheme/cgi/2016.01/geologicunitmorphology> ;
    skos:prefLabel "arch morphology"@en ;
    skos:related <http://resource.geosciml.org/classifier/cgi/geologicunitmorphology/longitudinal_section_of_cylinder> .


<http://resource.geosciml.org/classifier/cgi/geologicunitmorphology/arcuate_sheet> a skos:Concept ;
    dcterms:provenance "This vocabulary"@en ;
    rdfs:isDefinedBy <http://resource.geosciml.org/classifierscheme/cgi/2016.01/geologicunitmorphology> ;
    skos:broader <http://resource.geosciml.org/classifier/cgi/geologicunitmorphology/sheet> ;
    skos:definition "Sheet in which one of L or W is a curved arc"@en ;
    skos:inScheme <http://resource.geosciml.org/classifierscheme/cgi/2016.01/geologicunitmorphology> ;
    skos:prefLabel "arcuate sheet"@en .


<http://resource.geosciml.org/classifier/cgi/geologicunitmorphology/basin_shape> a skos:Concept ;
    dcterms:provenance "This vocabulary"@en ;
    rdfs:isDefinedBy <http://resource.geosciml.org/classifierscheme/cgi/2016.01/geologicunitmorphology> ;
    skos:broader <http://resource.geosciml.org/classifier/cgi/geologicunitmorphology/geologic_body> ;
    skos:definition "Geometric analog is convex down discoid, term generally connotes a kilometer-scale feature. Map view may be circular, elliptical, or irregular, characteristic feature is thickening from the edges towards the center. Typically used to describe a body of sedimentary rock deposited in a low area in the Earth's crust, in which case there is an implication that the top is (or was) a surface of deposition."@en ;
    skos:inScheme <http://resource.geosciml.org/classifierscheme/cgi/2016.01/geologicunitmorphology> ;
    skos:prefLabel "basin shape"@en,
        "buffertzon"@sv ;
    skos:related <http://resource.geosciml.org/classifier/cgi/geologicunitmorphology/discus>,
        <http://resource.geosciml.org/classifier/cgi/geologicunitmorphology/hemispheroid> .


<http://resource.geosciml.org/classifier/cgi/geologicunitmorphology/blanket_shape> a skos:Concept ;
    dcterms:provenance "This vocabulary"@en ;
    rdfs:isDefinedBy <http://resource.geosciml.org/classifierscheme/cgi/2016.01/geologicunitmorphology> ;
    skos:broader <http://resource.geosciml.org/classifier/cgi/geologicunitmorphology/geologic_body> ;
    skos:definition "A thin, widespread body with width to thickness ratio greater than 1000 to 1 that covers an underlying substrate. A layer of known great lateral extent. Morphology equivalent to bed or layer, but implies that body forms the top of some unit, instead of occurring within a body."@en ;
    skos:inScheme <http://resource.geosciml.org/classifierscheme/cgi/2016.01/geologicunitmorphology> ;
    skos:prefLabel "blanket shape"@en ;
    skos:related <http://resource.geosciml.org/classifier/cgi/geologicunitmorphology/sheet> .


<http://resource.geosciml.org/classifier/cgi/geologicunitmorphology/blob> a skos:Concept ;
    dcterms:provenance "This vocabulary"@en ;
    rdfs:isDefinedBy <http://resource.geosciml.org/classifierscheme/cgi/2016.01/geologicunitmorphology> ;
    skos:broader <http://resource.geosciml.org/classifier/cgi/geologicunitmorphology/three_dimensional_body> ;
    skos:definition "Body with smooth surface, broadly equant shape, irregular protuberances, no symmetry axes, and a boundary that can not be separated into sides."@en ;
    skos:inScheme <http://resource.geosciml.org/classifierscheme/cgi/2016.01/geologicunitmorphology> ;
    skos:prefLabel "blob"@en .


<http://resource.geosciml.org/classifier/cgi/geologicunitmorphology/block> a skos:Concept ;
    dcterms:provenance "This vocabulary"@en ;
    rdfs:isDefinedBy <http://resource.geosciml.org/classifierscheme/cgi/2016.01/geologicunitmorphology> ;
    skos:altLabel "bangun bongkah"@id,
        "지괴구조"@ko ;
    skos:broader <http://resource.geosciml.org/classifier/cgi/geologicunitmorphology/polygonal_cylinder> ;
    skos:definition "Equant polygonal cylinder, L=W=H, definable edges separate bounding surfaces. Grades to tabular prism as one horizontal dimension becomes distinctly longer than the other, and tablet or polygonal cylinder as one vertical axis becomes distinctly shorter or longer than the horizontal axes."@en ;
    skos:inScheme <http://resource.geosciml.org/classifierscheme/cgi/2016.01/geologicunitmorphology> ;
    skos:prefLabel "Blockstruktur"@de,
        "block"@en,
        "estructura bloques"@es,
        "lohkorakenteet"@fi,
        "structure bloc"@fr,
        "struktur bongkah"@id,
        "struttura a blocchi"@it,
        "地塊構造"@ja,
        "rcnasm<½nCabøúk"@km,
        "암괴구조"@ko,
        "Â£¤¦É¾¤»ø®®ìñº¡"@lo,
        "struktur bongkah"@ms,
        "struktura blokovaya"@ru,
        "blockstruktur"@sv,
        "โครงสร้างบล็อก"@th,
        "cấu trúc khối"@vi,
        "块状构造"@zh .


<http://resource.geosciml.org/classifier/cgi/geologicunitmorphology/boudin_shape> a skos:Concept ;
    dcterms:provenance "This vocabulary"@en ;
    rdfs:isDefinedBy <http://resource.geosciml.org/classifierscheme/cgi/2016.01/geologicunitmorphology> ;
    skos:broader <http://resource.geosciml.org/classifier/cgi/geologicunitmorphology/geologic_body> ;
    skos:definition "Layer or bed of rock deformed into sausage-shaped segments (boudins), either separated or joined by pinched connections. Morphology generally defined in a profile view, third dimension is not denoted, use of term also implies that the body is not isolated, but is related to an original body elongate on some dimension that has been stretched and separated into separate bodies"@en ;
    skos:inScheme <http://resource.geosciml.org/classifierscheme/cgi/2016.01/geologicunitmorphology> ;
    skos:prefLabel "boudin shape"@en ;
    skos:related <http://resource.geosciml.org/classifier/cgi/geologicunitmorphology/bread_loaf_ellipsoid> .


<http://resource.geosciml.org/classifier/cgi/geologicunitmorphology/bread_loaf_ellipsoid> a skos:Concept ;
    dcterms:provenance "This vocabulary"@en ;
    rdfs:isDefinedBy <http://resource.geosciml.org/classifierscheme/cgi/2016.01/geologicunitmorphology> ;
    skos:broader <http://resource.geosciml.org/classifier/cgi/geologicunitmorphology/ellipsoid> ;
    skos:definition "Ellipsoid with L 10 times W or H"@en ;
    skos:inScheme <http://resource.geosciml.org/classifierscheme/cgi/2016.01/geologicunitmorphology> ;
    skos:prefLabel "bread loaf ellipsoid"@en .


<http://resource.geosciml.org/classifier/cgi/geologicunitmorphology/channel_shape> a skos:Concept ;
    dcterms:provenance "This vocabulary"@en ;
    rdfs:isDefinedBy <http://resource.geosciml.org/classifierscheme/cgi/2016.01/geologicunitmorphology> ;
    skos:altLabel "gully"@sv ;
    skos:broader <http://resource.geosciml.org/classifier/cgi/geologicunitmorphology/geologic_body> ;
    skos:definition "Strongly elongate lens or ribbon with a convex downward lower surface, near planar upper surface. Morphology is equivalent to upside down arch."@en ;
    skos:inScheme <http://resource.geosciml.org/classifierscheme/cgi/2016.01/geologicunitmorphology> ;
    skos:prefLabel "Rinne"@de,
        "channel shape"@en,
        "canal natural"@es,
        "uomat"@fi,
        "canale"@it,
        "ruslo"@ru,
        "kanal"@sv ;
    skos:related <http://resource.geosciml.org/classifier/cgi/geologicunitmorphology/longitudinal_section_of_cylinder>,
        <http://resource.geosciml.org/classifier/cgi/geologicunitmorphology/ribbon> .


<http://resource.geosciml.org/classifier/cgi/geologicunitmorphology/circular_cylinder> a skos:Concept ;
    dcterms:provenance "This vocabulary"@en ;
    rdfs:isDefinedBy <http://resource.geosciml.org/classifierscheme/cgi/2016.01/geologicunitmorphology> ;
    skos:broader <http://resource.geosciml.org/classifier/cgi/geologicunitmorphology/elliptical_cylinder> ;
    skos:definition "Elliptical cylinder that has circular symmetry about long axis, distinct side surfaces are not defined. Cross section is circular"@en ;
    skos:inScheme <http://resource.geosciml.org/classifierscheme/cgi/2016.01/geologicunitmorphology> ;
    skos:prefLabel "circular cylinder"@en .


<http://resource.geosciml.org/classifier/cgi/geologicunitmorphology/circular_profile> a skos:Concept ;
    dcterms:provenance "This vocabulary"@en ;
    rdfs:isDefinedBy <http://resource.geosciml.org/classifierscheme/cgi/2016.01/geologicunitmorphology> ;
    skos:broader <http://resource.geosciml.org/classifier/cgi/geologicunitmorphology/equant_profile> ;
    skos:definition "equant profile with arcuate boundary"@en ;
    skos:inScheme <http://resource.geosciml.org/classifierscheme/cgi/2016.01/geologicunitmorphology> ;
    skos:prefLabel "circular profile"@en .


<http://resource.geosciml.org/classifier/cgi/geologicunitmorphology/column_shape> a skos:Concept ;
    dcterms:provenance "This vocabulary"@en ;
    rdfs:isDefinedBy <http://resource.geosciml.org/classifierscheme/cgi/2016.01/geologicunitmorphology> ;
    skos:broader <http://resource.geosciml.org/classifier/cgi/geologicunitmorphology/geologic_body> ;
    skos:definition "Cylindrical body, equant cross section, long in direction normal to equant cross section. Morphology equivalent to pipe, without denotation of transport function."@en ;
    skos:inScheme <http://resource.geosciml.org/classifierscheme/cgi/2016.01/geologicunitmorphology> ;
    skos:prefLabel "column shape"@en ;
    skos:related <http://resource.geosciml.org/classifier/cgi/geologicunitmorphology/circular_cylinder>,
        <http://resource.geosciml.org/classifier/cgi/geologicunitmorphology/polygonal_cylinder> .


<http://resource.geosciml.org/classifier/cgi/geologicunitmorphology/cone> a skos:Concept ;
    dcterms:provenance "This vocabulary"@en ;
    rdfs:isDefinedBy <http://resource.geosciml.org/classifierscheme/cgi/2016.01/geologicunitmorphology> ;
    skos:broader <http://resource.geosciml.org/classifier/cgi/geologicunitmorphology/discus> ;
    skos:definition "Discus with one planar side, and circular symmetry on axis, geologic cones typically have height <(<) diameter"@en ;
    skos:inScheme <http://resource.geosciml.org/classifierscheme/cgi/2016.01/geologicunitmorphology> ;
    skos:prefLabel "cone shape"@en .


<http://resource.geosciml.org/classifier/cgi/geologicunitmorphology/cone_segment> a skos:Concept ;
    dcterms:provenance "This vocabulary"@en ;
    rdfs:isDefinedBy <http://resource.geosciml.org/classifierscheme/cgi/2016.01/geologicunitmorphology> ;
    skos:broader <http://resource.geosciml.org/classifier/cgi/geologicunitmorphology/three_dimensional_body> ;
    skos:definition "Body that is section of a cone formed by splitting the cone along a surface parallel to the cone axis, that interesect approximately along the axis."@en ;
    skos:inScheme <http://resource.geosciml.org/classifierscheme/cgi/2016.01/geologicunitmorphology> ;
    skos:prefLabel "cone segment"@en .


<http://resource.geosciml.org/classifier/cgi/geologicunitmorphology/conical_sheet> a skos:Concept ;
    dcterms:provenance "This vocabulary"@en ;
    rdfs:isDefinedBy <http://resource.geosciml.org/classifierscheme/cgi/2016.01/geologicunitmorphology> ;
    skos:broader <http://resource.geosciml.org/classifier/cgi/geologicunitmorphology/sheet> ;
    skos:definition "Sheet that conforms to surface of a cone."@en ;
    skos:inScheme <http://resource.geosciml.org/classifierscheme/cgi/2016.01/geologicunitmorphology> ;
    skos:prefLabel "conical sheet"@en .


<http://resource.geosciml.org/classifier/cgi/geologicunitmorphology/cupola> a skos:Concept ;
    dcterms:provenance "This vocabulary"@en ;
    rdfs:isDefinedBy <http://resource.geosciml.org/classifierscheme/cgi/2016.01/geologicunitmorphology> ;
    skos:broader <http://resource.geosciml.org/classifier/cgi/geologicunitmorphology/geologic_body> ;
    skos:definition "Large upward projection of the roof of an igneous intrusion into the country rock above. A possibly irregular dome like or columnar body rooted in a larger body."@en ;
    skos:inScheme <http://resource.geosciml.org/classifierscheme/cgi/2016.01/geologicunitmorphology> ;
    skos:prefLabel "cupola"@en ;
    skos:related <http://resource.geosciml.org/classifier/cgi/geologicunitmorphology/hemispheroid> .


<http://resource.geosciml.org/classifier/cgi/geologicunitmorphology/cylinder> a skos:Concept ;
    dcterms:provenance "This vocabulary"@en ;
    rdfs:isDefinedBy <http://resource.geosciml.org/classifierscheme/cgi/2016.01/geologicunitmorphology> ;
    skos:broader <http://resource.geosciml.org/classifier/cgi/geologicunitmorphology/three_dimensional_body> ;
    skos:definition "Body defined by translation of a generating plane figure with approximately equant cross section (circle, ellipsoid, polygon) along a straight axial line. H>=W=L. Axis is direction normal to generating plane figure, which forms parallel top and bottom bounding surface."@en ;
    skos:inScheme <http://resource.geosciml.org/classifierscheme/cgi/2016.01/geologicunitmorphology> ;
    skos:narrower <http://resource.geosciml.org/classifier/cgi/geologicunitmorphology/disc>,
        <http://resource.geosciml.org/classifier/cgi/geologicunitmorphology/elliptical_cylinder>,
        <http://resource.geosciml.org/classifier/cgi/geologicunitmorphology/polygonal_cylinder>,
        <http://resource.geosciml.org/classifier/cgi/geologicunitmorphology/rod> ;
    skos:prefLabel "cylinder"@en .


<http://resource.geosciml.org/classifier/cgi/geologicunitmorphology/dart_ellipsoid> a skos:Concept ;
    dcterms:provenance "This vocabulary"@en ;
    rdfs:isDefinedBy <http://resource.geosciml.org/classifierscheme/cgi/2016.01/geologicunitmorphology> ;
    skos:broader <http://resource.geosciml.org/classifier/cgi/geologicunitmorphology/ellipsoid> ;
    skos:definition "Ellipsoid with L more than 50 times W or H"@en ;
    skos:inScheme <http://resource.geosciml.org/classifierscheme/cgi/2016.01/geologicunitmorphology> ;
    skos:prefLabel "dart ellipsoid"@en .


<http://resource.geosciml.org/classifier/cgi/geologicunitmorphology/diapir> a skos:Concept ;
    dcterms:provenance "This vocabulary"@en ;
    rdfs:isDefinedBy <http://resource.geosciml.org/classifierscheme/cgi/2016.01/geologicunitmorphology> ;
    skos:broader <http://resource.geosciml.org/classifier/cgi/geologicunitmorphology/geologic_body> ;
    skos:definition "Broadly inverted tear drop morphology. Body of magmatic or mobile sedimentary material intruded into overlying rocks."@en ;
    skos:inScheme <http://resource.geosciml.org/classifierscheme/cgi/2016.01/geologicunitmorphology> ;
    skos:prefLabel "diapir"@en .


<http://resource.geosciml.org/classifier/cgi/geologicunitmorphology/dike> a skos:Concept ;
    dcterms:provenance "This vocabulary"@en ;
    rdfs:isDefinedBy <http://resource.geosciml.org/classifierscheme/cgi/2016.01/geologicunitmorphology> ;
    skos:altLabel "dyke"@en ;
    skos:broader <http://resource.geosciml.org/classifier/cgi/geologicunitmorphology/geologic_body> ;
    skos:definition "A generally sheet-like intrusive rock body that cuts across bedding or foliation in the host rock, or intrudes massive host rock."@en ;
    skos:inScheme <http://resource.geosciml.org/classifierscheme/cgi/2016.01/geologicunitmorphology> ;
    skos:prefLabel "Dyke"@de,
        "dike"@en,
        "dique"@es,
        "juonet"@fi,
        "dicco"@it,
        "dajka"@ru,
        "gång"@sv ;
    skos:related <http://resource.geosciml.org/classifier/cgi/geologicunitmorphology/sheet> .


<http://resource.geosciml.org/classifier/cgi/geologicunitmorphology/disc> a skos:Concept ;
    dcterms:provenance "This vocabulary"@en ;
    rdfs:isDefinedBy <http://resource.geosciml.org/classifierscheme/cgi/2016.01/geologicunitmorphology> ;
    skos:broader <http://resource.geosciml.org/classifier/cgi/geologicunitmorphology/cylinder> ;
    skos:definition "Cylinder with height less than diameter. L=W>H, edges separates side from top and bottom. Grades to oblate ellipsoid as edges lose definition."@en ;
    skos:inScheme <http://resource.geosciml.org/classifierscheme/cgi/2016.01/geologicunitmorphology> ;
    skos:prefLabel "disc"@en .


<http://resource.geosciml.org/classifier/cgi/geologicunitmorphology/discoid_anulus> a skos:Concept ;
    dcterms:provenance "This vocabulary"@en ;
    rdfs:isDefinedBy <http://resource.geosciml.org/classifierscheme/cgi/2016.01/geologicunitmorphology> ;
    skos:broader <http://resource.geosciml.org/classifier/cgi/geologicunitmorphology/three_dimensional_body> ;
    skos:definition "Cone with central part removed along cylindrical volume approximately along the cone axis"@en ;
    skos:inScheme <http://resource.geosciml.org/classifierscheme/cgi/2016.01/geologicunitmorphology> ;
    skos:prefLabel "discoid anulus"@en .


<http://resource.geosciml.org/classifier/cgi/geologicunitmorphology/discus> a skos:Concept ;
    dcterms:provenance "This vocabulary"@en ;
    rdfs:isDefinedBy <http://resource.geosciml.org/classifierscheme/cgi/2016.01/geologicunitmorphology> ;
    skos:broader <http://resource.geosciml.org/classifier/cgi/geologicunitmorphology/three_dimensional_body> ;
    skos:definition "Body with two sides that converge to define an edge that is circular in profile, edge separates definable top and bottom. L=W>H. Grades to oblate ellipsoid as edge separating sides loses definition, cone as one side becomes distinctly planar."@en ;
    skos:inScheme <http://resource.geosciml.org/classifierscheme/cgi/2016.01/geologicunitmorphology> ;
    skos:narrower <http://resource.geosciml.org/classifier/cgi/geologicunitmorphology/cone>,
        <http://resource.geosciml.org/classifier/cgi/geologicunitmorphology/elongate_discus> ;
    skos:prefLabel "discus"@en .


<http://resource.geosciml.org/classifier/cgi/geologicunitmorphology/dome> a skos:Concept ;
    dcterms:provenance "This vocabulary"@en ;
    rdfs:isDefinedBy <http://resource.geosciml.org/classifierscheme/cgi/2016.01/geologicunitmorphology> ;
    skos:broader <http://resource.geosciml.org/classifier/cgi/geologicunitmorphology/geologic_body> ;
    skos:definition "Steep-sided disk-like body, for example and accumulation of high viscosity lava above and around a volcanic vent. A structure in which the top of the body dips gently away in all directions e.g. salt dome, extrusion dome"@en ;
    skos:inScheme <http://resource.geosciml.org/classifierscheme/cgi/2016.01/geologicunitmorphology> ;
    skos:prefLabel "Dom"@de,
        "dome"@en,
        "domo"@es,
        "doomit"@fi,
        "duomo"@it,
        "kupol"@ru,
        "dom"@sv ;
    skos:related <http://resource.geosciml.org/classifier/cgi/geologicunitmorphology/hemispheroid> .


<http://resource.geosciml.org/classifier/cgi/geologicunitmorphology/dome_sheet> a skos:Concept ;
    dcterms:provenance "This vocabulary"@en ;
    rdfs:isDefinedBy <http://resource.geosciml.org/classifierscheme/cgi/2016.01/geologicunitmorphology> ;
    skos:broader <http://resource.geosciml.org/classifier/cgi/geologicunitmorphology/sheet> ;
    skos:definition "Sheet in which L and W are curved arcs."@en ;
    skos:inScheme <http://resource.geosciml.org/classifierscheme/cgi/2016.01/geologicunitmorphology> ;
    skos:prefLabel "dome sheet"@en .


<http://resource.geosciml.org/classifier/cgi/geologicunitmorphology/ductolith> a skos:Concept ;
    dcterms:provenance "This vocabulary"@en ;
    rdfs:isDefinedBy <http://resource.geosciml.org/classifierscheme/cgi/2016.01/geologicunitmorphology> ;
    skos:broader <http://resource.geosciml.org/classifier/cgi/geologicunitmorphology/geologic_body> ;
    skos:definition "Concordant intrusion, teardrop-shaped in cross section."@en ;
    skos:inScheme <http://resource.geosciml.org/classifierscheme/cgi/2016.01/geologicunitmorphology> ;
    skos:prefLabel "ductolith"@en ;
    skos:related <http://resource.geosciml.org/classifier/cgi/geologicunitmorphology/diapir>,
        <http://resource.geosciml.org/classifier/cgi/geologicunitmorphology/tear_drop> .


<http://resource.geosciml.org/classifier/cgi/geologicunitmorphology/ellipsoid> a skos:Concept ;
    dcterms:provenance "This vocabulary"@en ;
    rdfs:isDefinedBy <http://resource.geosciml.org/classifierscheme/cgi/2016.01/geologicunitmorphology> ;
    skos:broader <http://resource.geosciml.org/classifier/cgi/geologicunitmorphology/three_dimensional_body> ;
    skos:definition "Body that contains three orthogonal axes defining three surfaces of reflection symmetry, profiles along the surfaces are elliptical. Boundary can not be separated into sides (no edges). Becomes cylinder or disc when bounding surface can be considered parallel to one of the axis. L>=W>=H"@en ;
    skos:inScheme <http://resource.geosciml.org/classifierscheme/cgi/2016.01/geologicunitmorphology> ;
    skos:narrower <http://resource.geosciml.org/classifier/cgi/geologicunitmorphology/bread_loaf_ellipsoid>,
        <http://resource.geosciml.org/classifier/cgi/geologicunitmorphology/dart_ellipsoid>,
        <http://resource.geosciml.org/classifier/cgi/geologicunitmorphology/football_ellipsoid>,
        <http://resource.geosciml.org/classifier/cgi/geologicunitmorphology/pancake_ellipsoid>,
        <http://resource.geosciml.org/classifier/cgi/geologicunitmorphology/pillow_ellipsoid>,
        <http://resource.geosciml.org/classifier/cgi/geologicunitmorphology/sheet_ellipsoid>,
        <http://resource.geosciml.org/classifier/cgi/geologicunitmorphology/spheroid> ;
    skos:prefLabel "ellipsoid"@en .


<http://resource.geosciml.org/classifier/cgi/geologicunitmorphology/elliptical_cylinder> a skos:Concept ;
    dcterms:provenance "This vocabulary"@en ;
    rdfs:isDefinedBy <http://resource.geosciml.org/classifierscheme/cgi/2016.01/geologicunitmorphology> ;
    skos:broader <http://resource.geosciml.org/classifier/cgi/geologicunitmorphology/cylinder> ;
    skos:definition "Cylinder that has elliptical cross section, distinct side surfaces are not defined."@en ;
    skos:inScheme <http://resource.geosciml.org/classifierscheme/cgi/2016.01/geologicunitmorphology> ;
    skos:narrower <http://resource.geosciml.org/classifier/cgi/geologicunitmorphology/circular_cylinder> ;
    skos:prefLabel "elliptical cylinder"@en .


<http://resource.geosciml.org/classifier/cgi/geologicunitmorphology/elliptical_profile> a skos:Concept ;
    dcterms:provenance "This vocabulary"@en ;
    rdfs:isDefinedBy <http://resource.geosciml.org/classifierscheme/cgi/2016.01/geologicunitmorphology> ;
    skos:broader <http://resource.geosciml.org/classifier/cgi/geologicunitmorphology/planar_profile> ;
    skos:definition "Profile approximates an ellipse, ratio of long axis to short axis is greater than 1.4"@en ;
    skos:inScheme <http://resource.geosciml.org/classifierscheme/cgi/2016.01/geologicunitmorphology> ;
    skos:prefLabel "elliptical profile"@en .


<http://resource.geosciml.org/classifier/cgi/geologicunitmorphology/elongate_discus> a skos:Concept ;
    dcterms:provenance "This vocabulary"@en ;
    rdfs:isDefinedBy <http://resource.geosciml.org/classifierscheme/cgi/2016.01/geologicunitmorphology> ;
    skos:broader <http://resource.geosciml.org/classifier/cgi/geologicunitmorphology/discus> ;
    skos:definition "Discus for which the profile defined by the bounding edge is longer in one direction than other. L>W>>H"@en ;
    skos:inScheme <http://resource.geosciml.org/classifierscheme/cgi/2016.01/geologicunitmorphology> ;
    skos:prefLabel "elongate discus"@en .


<http://resource.geosciml.org/classifier/cgi/geologicunitmorphology/equant_polygonal_profile> a skos:Concept ;
    dcterms:provenance "This vocabulary"@en ;
    rdfs:isDefinedBy <http://resource.geosciml.org/classifierscheme/cgi/2016.01/geologicunitmorphology> ;
    skos:broader <http://resource.geosciml.org/classifier/cgi/geologicunitmorphology/equant_profile> ;
    skos:definition "Aquant profile with boundary that can be divided into distinct straight sides separated by higher curvature corners."@en ;
    skos:inScheme <http://resource.geosciml.org/classifierscheme/cgi/2016.01/geologicunitmorphology> ;
    skos:prefLabel "equant polygonal profile"@en .


<http://resource.geosciml.org/classifier/cgi/geologicunitmorphology/equant_profile> a skos:Concept ;
    dcterms:provenance "This vocabulary"@en ;
    rdfs:isDefinedBy <http://resource.geosciml.org/classifierscheme/cgi/2016.01/geologicunitmorphology> ;
    skos:broader <http://resource.geosciml.org/classifier/cgi/geologicunitmorphology/planar_profile> ;
    skos:definition "Profile for which the ratio of length of longest chord to shortest chord is less than 1.4."@en ;
    skos:inScheme <http://resource.geosciml.org/classifierscheme/cgi/2016.01/geologicunitmorphology> ;
    skos:narrower <http://resource.geosciml.org/classifier/cgi/geologicunitmorphology/circular_profile>,
        <http://resource.geosciml.org/classifier/cgi/geologicunitmorphology/equant_polygonal_profile> ;
    skos:prefLabel "equant profile"@en .


<http://resource.geosciml.org/classifier/cgi/geologicunitmorphology/ethmolith> a skos:Concept ;
    dcterms:provenance "This vocabulary"@en ;
    rdfs:isDefinedBy <http://resource.geosciml.org/classifierscheme/cgi/2016.01/geologicunitmorphology> ;
    skos:broader <http://resource.geosciml.org/classifier/cgi/geologicunitmorphology/geologic_body> ;
    skos:definition "Discordant, funnel-shaped intrusion, tapers downward"@en ;
    skos:inScheme <http://resource.geosciml.org/classifierscheme/cgi/2016.01/geologicunitmorphology> ;
    skos:prefLabel "ethmolith"@en ;
    skos:related <http://resource.geosciml.org/classifier/cgi/geologicunitmorphology/cone> .


<http://resource.geosciml.org/classifier/cgi/geologicunitmorphology/fan> a skos:Concept ;
    dcterms:provenance "This vocabulary"@en ;
    rdfs:isDefinedBy <http://resource.geosciml.org/classifierscheme/cgi/2016.01/geologicunitmorphology> ;
    skos:broader <http://resource.geosciml.org/classifier/cgi/geologicunitmorphology/geologic_body> ;
    skos:definition "A cone segment, generally applied to surface morphology of sedimentary deposit with a gentle surface slope, radiating from a localized sediment source."@en ;
    skos:inScheme <http://resource.geosciml.org/classifierscheme/cgi/2016.01/geologicunitmorphology> ;
    skos:prefLabel "Faecher"@de,
        "fan"@en,
        "cono"@es,
        "keilat"@fi,
        "conoide"@it,
        "vynos veeroobraznyj"@ru,
        "kon"@sv ;
    skos:related <http://resource.geosciml.org/classifier/cgi/geologicunitmorphology/cone_segment> .


<http://resource.geosciml.org/classifier/cgi/geologicunitmorphology/football_ellipsoid> a skos:Concept ;
    dcterms:provenance "This vocabulary"@en ;
    rdfs:isDefinedBy <http://resource.geosciml.org/classifierscheme/cgi/2016.01/geologicunitmorphology> ;
    skos:broader <http://resource.geosciml.org/classifier/cgi/geologicunitmorphology/ellipsoid> ;
    skos:definition "Ellipsoid with L 2 to 5 times W or H"@en ;
    skos:inScheme <http://resource.geosciml.org/classifierscheme/cgi/2016.01/geologicunitmorphology> ;
    skos:prefLabel "football ellipsoid"@en .


<http://resource.geosciml.org/classifier/cgi/geologicunitmorphology/geologic_body> a skos:Concept ;
    dcterms:provenance "This vocabulary"@en ;
    rdfs:isDefinedBy <http://resource.geosciml.org/classifierscheme/cgi/2016.01/geologicunitmorphology> ;
    skos:broader <http://resource.geosciml.org/classifier/cgi/geologicunitmorphology/three_dimensional_body> ;
    skos:definition "A 3 dimensional body defined based on geometric shape, with some geologic connotation or denotation."@en ;
    skos:inScheme <http://resource.geosciml.org/classifierscheme/cgi/2016.01/geologicunitmorphology> ;
    skos:narrower <http://resource.geosciml.org/classifier/cgi/geologicunitmorphology/arch_morphology>,
        <http://resource.geosciml.org/classifier/cgi/geologicunitmorphology/basin_shape>,
        <http://resource.geosciml.org/classifier/cgi/geologicunitmorphology/blanket_shape>,
        <http://resource.geosciml.org/classifier/cgi/geologicunitmorphology/boudin_shape>,
        <http://resource.geosciml.org/classifier/cgi/geologicunitmorphology/channel_shape>,
        <http://resource.geosciml.org/classifier/cgi/geologicunitmorphology/column_shape>,
        <http://resource.geosciml.org/classifier/cgi/geologicunitmorphology/cupola>,
        <http://resource.geosciml.org/classifier/cgi/geologicunitmorphology/diapir>,
        <http://resource.geosciml.org/classifier/cgi/geologicunitmorphology/dike>,
        <http://resource.geosciml.org/classifier/cgi/geologicunitmorphology/dome>,
        <http://resource.geosciml.org/classifier/cgi/geologicunitmorphology/ductolith>,
        <http://resource.geosciml.org/classifier/cgi/geologicunitmorphology/ethmolith>,
        <http://resource.geosciml.org/classifier/cgi/geologicunitmorphology/fan>,
        <http://resource.geosciml.org/classifier/cgi/geologicunitmorphology/graben_shape>,
        <http://resource.geosciml.org/classifier/cgi/geologicunitmorphology/laccolith>,
        <http://resource.geosciml.org/classifier/cgi/geologicunitmorphology/layer_shape>,
        <http://resource.geosciml.org/classifier/cgi/geologicunitmorphology/lens>,
        <http://resource.geosciml.org/classifier/cgi/geologicunitmorphology/lopolith>,
        <http://resource.geosciml.org/classifier/cgi/geologicunitmorphology/mound>,
        <http://resource.geosciml.org/classifier/cgi/geologicunitmorphology/phacolith>,
        <http://resource.geosciml.org/classifier/cgi/geologicunitmorphology/pipe>,
        <http://resource.geosciml.org/classifier/cgi/geologicunitmorphology/pod>,
        <http://resource.geosciml.org/classifier/cgi/geologicunitmorphology/ring_dyke>,
        <http://resource.geosciml.org/classifier/cgi/geologicunitmorphology/rock_body_geometry_irregular>,
        <http://resource.geosciml.org/classifier/cgi/geologicunitmorphology/rock_body_geometry_not_specified>,
        <http://resource.geosciml.org/classifier/cgi/geologicunitmorphology/sill_form>,
        <http://resource.geosciml.org/classifier/cgi/geologicunitmorphology/sphenolith>,
        <http://resource.geosciml.org/classifier/cgi/geologicunitmorphology/trough>,
        <http://resource.geosciml.org/classifier/cgi/geologicunitmorphology/vein> ;
    skos:prefLabel "geologic body"@en .


<http://resource.geosciml.org/classifier/cgi/geologicunitmorphology/graben_shape> a skos:Concept ;
    dcterms:provenance "This vocabulary"@en ;
    rdfs:isDefinedBy <http://resource.geosciml.org/classifierscheme/cgi/2016.01/geologicunitmorphology> ;
    skos:broader <http://resource.geosciml.org/classifier/cgi/geologicunitmorphology/geologic_body> ;
    skos:definition "an elongate body bounded on both sides by normal faults that dip toward each other"@en ;
    skos:inScheme <http://resource.geosciml.org/classifierscheme/cgi/2016.01/geologicunitmorphology> ;
    skos:prefLabel "Graben"@de,
        "graben shape"@en,
        "graben"@es,
        "hautavajoamat"@fi,
        "graben"@it,
        "graben"@ru,
        "gravsänka"@sv ;
    skos:related <http://resource.geosciml.org/classifier/cgi/geologicunitmorphology/tabular_prism> .


<http://resource.geosciml.org/classifier/cgi/geologicunitmorphology/hemispheroid> a skos:Concept ;
    dcterms:provenance "This vocabulary"@en ;
    rdfs:isDefinedBy <http://resource.geosciml.org/classifierscheme/cgi/2016.01/geologicunitmorphology> ;
    skos:broader <http://resource.geosciml.org/classifier/cgi/geologicunitmorphology/three_dimensional_body> ;
    skos:definition "Section of a spheroid formed by removing everything on the smaller volume side of a surface that intersects the spheroid. Grades to cone as suface generator (line rotated about axis to generate volume above lower planar boundary) becomes straight."@en ;
    skos:inScheme <http://resource.geosciml.org/classifierscheme/cgi/2016.01/geologicunitmorphology> ;
    skos:prefLabel "hemispheroid"@en .


<http://resource.geosciml.org/classifier/cgi/geologicunitmorphology/irregular_profile> a skos:Concept ;
    dcterms:provenance "This vocabulary"@en ;
    rdfs:isDefinedBy <http://resource.geosciml.org/classifierscheme/cgi/2016.01/geologicunitmorphology> ;
    skos:broader <http://resource.geosciml.org/classifier/cgi/geologicunitmorphology/planar_profile> ;
    skos:definition "Profile does not conform to any of the regular geometries associated with other categories in the vocabulary."@en ;
    skos:inScheme <http://resource.geosciml.org/classifierscheme/cgi/2016.01/geologicunitmorphology> ;
    skos:prefLabel "irregular profile"@en .


<http://resource.geosciml.org/classifier/cgi/geologicunitmorphology/laccolith> a skos:Concept ;
    dcterms:provenance "This vocabulary"@en ;
    rdfs:isDefinedBy <http://resource.geosciml.org/classifierscheme/cgi/2016.01/geologicunitmorphology> ;
    skos:altLabel "¹ó­-ºñ¡-£½-­ó-»ø®-À¹ñ©"@lo,
        "岩盘"@zh,
        "菌形穹隆"@zh ;
    skos:broader <http://resource.geosciml.org/classifier/cgi/geologicunitmorphology/geologic_body> ;
    skos:definition "A tabular or lenticular igneous body whose long dimensions parallel layering in the host rock, and which as a convex-up roof and a known or assumed flat floor"@en ;
    skos:inScheme <http://resource.geosciml.org/classifierscheme/cgi/2016.01/geologicunitmorphology> ;
    skos:prefLabel "Lakkolith"@de,
        "laccolith"@en,
        "lacolito"@es,
        "lakkoliitit"@fi,
        "laccolite"@fr,
        "lakolit"@id,
        "laccolite"@it,
        "ラコリス"@ja,
        "Lk;kUlIt"@km,
        "병반"@ko,
        "¹ó­Áìñ¡-Â£-ìò©"@lo,
        "lakolitos"@ms,
        "lakkolit"@ru,
        "lakkolit"@sv,
        "หินอัคนีรูปเห็ด"@th,
        "thể nấm"@vi,
        "岩盖"@zh ;
    skos:related <http://resource.geosciml.org/classifier/cgi/geologicunitmorphology/discus>,
        <http://resource.geosciml.org/classifier/cgi/geologicunitmorphology/sheet_ellipsoid> .


<http://resource.geosciml.org/classifier/cgi/geologicunitmorphology/layer_shape> a skos:Concept ;
    dcterms:provenance "This vocabulary"@en ;
    rdfs:isDefinedBy <http://resource.geosciml.org/classifierscheme/cgi/2016.01/geologicunitmorphology> ;
    skos:broader <http://resource.geosciml.org/classifier/cgi/geologicunitmorphology/geologic_body> ;
    skos:definition "Body geometry characterized by generally thin character relative to the lateral extent of the body (on order of 1:100). Thin bodies of lesser extent are lenses. Connotes a non-intrusive body, equivalent intrusive body would be dike (or sill). Denotes that body is in a sequence of similar sheet-like bodies between other rock bodies"@en ;
    skos:inScheme <http://resource.geosciml.org/classifierscheme/cgi/2016.01/geologicunitmorphology> ;
    skos:prefLabel "Schicht"@de,
        "layer shape"@en,
        "estrato"@es,
        "kerrokset"@fi,
        "strato"@it,
        "sloj"@ru,
        "lager"@sv ;
    skos:related <http://resource.geosciml.org/classifier/cgi/geologicunitmorphology/blanket_shape>,
        <http://resource.geosciml.org/classifier/cgi/geologicunitmorphology/sill_form> .


<http://resource.geosciml.org/classifier/cgi/geologicunitmorphology/lens> a skos:Concept ;
    dcterms:provenance "This vocabulary"@en ;
    rdfs:isDefinedBy <http://resource.geosciml.org/classifierscheme/cgi/2016.01/geologicunitmorphology> ;
    skos:broader <http://resource.geosciml.org/classifier/cgi/geologicunitmorphology/geologic_body> ;
    skos:definition "A body bounded by converging surfaces (at least one of which is curved), thick in the middle and thinning out toward the edges, resembling a convex lens."@en ;
    skos:inScheme <http://resource.geosciml.org/classifierscheme/cgi/2016.01/geologicunitmorphology> ;
    skos:prefLabel "Linse"@de,
        "lens"@en,
        "lentejón"@es,
        "linssit"@fi,
        "lente"@it,
        "linza"@ru,
        "lins"@sv ;
    skos:related <http://resource.geosciml.org/classifier/cgi/geologicunitmorphology/discus> .


<http://resource.geosciml.org/classifier/cgi/geologicunitmorphology/lenticular_profile> a skos:Concept ;
    dcterms:provenance "This vocabulary"@en ;
    rdfs:isDefinedBy <http://resource.geosciml.org/classifierscheme/cgi/2016.01/geologicunitmorphology> ;
    skos:broader <http://resource.geosciml.org/classifier/cgi/geologicunitmorphology/planar_profile> ;
    skos:definition "Profile with ratio of long axis length to short axis length greater than 5 with sides that taper to a point, shaped like the profile of an optical lense."@en ;
    skos:inScheme <http://resource.geosciml.org/classifierscheme/cgi/2016.01/geologicunitmorphology> ;
    skos:prefLabel "lenticular profile"@en .


<http://resource.geosciml.org/classifier/cgi/geologicunitmorphology/longitudinal_section_of_cylinder> a skos:Concept ;
    dcterms:provenance "This vocabulary"@en ;
    rdfs:isDefinedBy <http://resource.geosciml.org/classifierscheme/cgi/2016.01/geologicunitmorphology> ;
    skos:broader <http://resource.geosciml.org/classifier/cgi/geologicunitmorphology/three_dimensional_body> ;
    skos:definition "Body that is section of a circular or elliptical cylinder formed by a splitting the cylinder along a surface approximately parallel to its long axis. L>>W>H."@en ;
    skos:inScheme <http://resource.geosciml.org/classifierscheme/cgi/2016.01/geologicunitmorphology> ;
    skos:prefLabel "longitudinal section of cylinder"@en .


<http://resource.geosciml.org/classifier/cgi/geologicunitmorphology/lopolith> a skos:Concept ;
    dcterms:provenance "This vocabulary"@en ;
    rdfs:isDefinedBy <http://resource.geosciml.org/classifierscheme/cgi/2016.01/geologicunitmorphology> ;
    skos:broader <http://resource.geosciml.org/classifier/cgi/geologicunitmorphology/geologic_body> ;
    skos:definition "A large, concordant, typically layered igneous intrusion whose floor is convex-down and whose roof may be convex-down or flat."@en ;
    skos:inScheme <http://resource.geosciml.org/classifierscheme/cgi/2016.01/geologicunitmorphology> ;
    skos:prefLabel "Lopolith"@de,
        "lopolith"@en,
        "lopolito"@es,
        "lopoliitit"@fi,
        "lopolite"@fr,
        "lopolit"@id,
        "lopolite"@it,
        "ロポリス"@ja,
        "silaEdllatsn§wgkñúgtMbn;"@km,
        "분상암체"@ko,
        "ÂìÂ²ìò©"@lo,
        "lopolitos"@ms,
        "lopolit"@ru,
        "lopolit"@sv,
        "หินอัคนีรูปฝักบัว"@th,
        "thể chậu"@vi,
        "岩盆"@zh ;
    skos:related <http://resource.geosciml.org/classifier/cgi/geologicunitmorphology/discus>,
        <http://resource.geosciml.org/classifier/cgi/geologicunitmorphology/sheet_ellipsoid> .


<http://resource.geosciml.org/classifier/cgi/geologicunitmorphology/mound> a skos:Concept ;
    dcterms:provenance "This vocabulary"@en ;
    rdfs:isDefinedBy <http://resource.geosciml.org/classifierscheme/cgi/2016.01/geologicunitmorphology> ;
    skos:broader <http://resource.geosciml.org/classifier/cgi/geologicunitmorphology/geologic_body> ;
    skos:definition "Lense like body of rock, lateral extent less than 100m, generally flat at bottom, with stratigraphic pinch out of beds (onlap) along upper sides."@en ;
    skos:inScheme <http://resource.geosciml.org/classifierscheme/cgi/2016.01/geologicunitmorphology> ;
    skos:prefLabel "Kuppe"@de,
        "mound"@en,
        "cerro"@es,
        "kumpareet"@fi,
        "mound"@it,
        "kholm zemlyanoj"@ru,
        "kulle"@sv ;
    skos:related <http://resource.geosciml.org/classifier/cgi/geologicunitmorphology/discus> .


<http://resource.geosciml.org/classifier/cgi/geologicunitmorphology/pancake_ellipsoid> a skos:Concept ;
    dcterms:provenance "This vocabulary"@en ;
    rdfs:isDefinedBy <http://resource.geosciml.org/classifierscheme/cgi/2016.01/geologicunitmorphology> ;
    skos:broader <http://resource.geosciml.org/classifier/cgi/geologicunitmorphology/ellipsoid> ;
    skos:definition "Ellipsoid with H on order of .01 of L or W"@en ;
    skos:inScheme <http://resource.geosciml.org/classifierscheme/cgi/2016.01/geologicunitmorphology> ;
    skos:prefLabel "pancake ellipsoid"@en .


<http://resource.geosciml.org/classifier/cgi/geologicunitmorphology/phacolith> a skos:Concept ;
    dcterms:provenance "This vocabulary"@en ;
    rdfs:isDefinedBy <http://resource.geosciml.org/classifierscheme/cgi/2016.01/geologicunitmorphology> ;
    skos:broader <http://resource.geosciml.org/classifier/cgi/geologicunitmorphology/geologic_body> ;
    skos:definition "Concordant, lenticular intrusion, emplaced along a fold axis"@en ;
    skos:inScheme <http://resource.geosciml.org/classifierscheme/cgi/2016.01/geologicunitmorphology> ;
    skos:prefLabel "phacolith"@en ;
    skos:related <http://resource.geosciml.org/classifier/cgi/geologicunitmorphology/longitudinal_section_of_cylinder> .


<http://resource.geosciml.org/classifier/cgi/geologicunitmorphology/pillow_ellipsoid> a skos:Concept ;
    dcterms:provenance "This vocabulary"@en ;
    rdfs:isDefinedBy <http://resource.geosciml.org/classifierscheme/cgi/2016.01/geologicunitmorphology> ;
    skos:broader <http://resource.geosciml.org/classifier/cgi/geologicunitmorphology/ellipsoid> ;
    skos:definition "Ellipsoid with H on order of 0.1 of L or W"@en ;
    skos:inScheme <http://resource.geosciml.org/classifierscheme/cgi/2016.01/geologicunitmorphology> ;
    skos:prefLabel "pillow ellipsoid"@en .


<http://resource.geosciml.org/classifier/cgi/geologicunitmorphology/pipe> a skos:Concept ;
    dcterms:provenance "This vocabulary"@en ;
    rdfs:isDefinedBy <http://resource.geosciml.org/classifierscheme/cgi/2016.01/geologicunitmorphology> ;
    skos:broader <http://resource.geosciml.org/classifier/cgi/geologicunitmorphology/geologic_body> ;
    skos:definition "Rock body that has a length to width ratio greater than 10 to 1, with two sub equal width dimensions."@en ;
    skos:inScheme <http://resource.geosciml.org/classifierscheme/cgi/2016.01/geologicunitmorphology> ;
    skos:prefLabel "Pipe"@de,
        "pipe"@en,
        "pipa"@es,
        "piiput"@fi,
        "tubo"@it,
        "trubka"@ru,
        "pipe"@sv .


<http://resource.geosciml.org/classifier/cgi/geologicunitmorphology/planar_sheet> a skos:Concept ;
    dcterms:provenance "This vocabulary"@en ;
    rdfs:isDefinedBy <http://resource.geosciml.org/classifierscheme/cgi/2016.01/geologicunitmorphology> ;
    skos:broader <http://resource.geosciml.org/classifier/cgi/geologicunitmorphology/sheet> ;
    skos:definition "Sheet in which L and W axes are straight lines"@en ;
    skos:inScheme <http://resource.geosciml.org/classifierscheme/cgi/2016.01/geologicunitmorphology> ;
    skos:prefLabel "planar sheet"@en .


<http://resource.geosciml.org/classifier/cgi/geologicunitmorphology/planar_vein> a skos:Concept ;
    dcterms:provenance "This vocabulary"@en ;
    rdfs:isDefinedBy <http://resource.geosciml.org/classifierscheme/cgi/2016.01/geologicunitmorphology> ;
    skos:broader <http://resource.geosciml.org/classifier/cgi/geologicunitmorphology/vein> ;
    skos:definition "Vein with length and width significantly greater than its thickness, giving the vein a tabular form"@en ;
    skos:inScheme <http://resource.geosciml.org/classifierscheme/cgi/2016.01/geologicunitmorphology> ;
    skos:prefLabel "planar vein"@en ;
    skos:related <http://resource.geosciml.org/classifier/cgi/geologicunitmorphology/dike>,
        <http://resource.geosciml.org/classifier/cgi/geologicunitmorphology/layer_shape> .


<http://resource.geosciml.org/classifier/cgi/geologicunitmorphology/pod> a skos:Concept ;
    dcterms:provenance "This vocabulary"@en ;
    rdfs:isDefinedBy <http://resource.geosciml.org/classifierscheme/cgi/2016.01/geologicunitmorphology> ;
    skos:broader <http://resource.geosciml.org/classifier/cgi/geologicunitmorphology/geologic_body> ;
    skos:definition "A small intrusion of elongate or lenticular form"@en ;
    skos:inScheme <http://resource.geosciml.org/classifierscheme/cgi/2016.01/geologicunitmorphology> ;
    skos:prefLabel "pod"@en ;
    skos:related <http://resource.geosciml.org/classifier/cgi/geologicunitmorphology/blob> .


<http://resource.geosciml.org/classifier/cgi/geologicunitmorphology/polygonal_cylinder> a skos:Concept ;
    dcterms:provenance "This vocabulary"@en ;
    rdfs:isDefinedBy <http://resource.geosciml.org/classifierscheme/cgi/2016.01/geologicunitmorphology> ;
    skos:broader <http://resource.geosciml.org/classifier/cgi/geologicunitmorphology/cylinder> ;
    skos:definition "Cylinder in which the edges bounding side surfaces are parallel or subparallel to cylinder axis. Cross section is polygon. Length of axis may be called height or thickness, and is typically in the vertical direction (distinguishing polygonal cylinder from tabular prism and wedge)."@en ;
    skos:inScheme <http://resource.geosciml.org/classifierscheme/cgi/2016.01/geologicunitmorphology> ;
    skos:narrower <http://resource.geosciml.org/classifier/cgi/geologicunitmorphology/block>,
        <http://resource.geosciml.org/classifier/cgi/geologicunitmorphology/square_profile>,
        <http://resource.geosciml.org/classifier/cgi/geologicunitmorphology/tablet> ;
    skos:prefLabel "polygonal cylinder"@en .


<http://resource.geosciml.org/classifier/cgi/geologicunitmorphology/polygonal_profile> a skos:Concept ;
    dcterms:provenance "This vocabulary"@en ;
    rdfs:isDefinedBy <http://resource.geosciml.org/classifierscheme/cgi/2016.01/geologicunitmorphology> ;
    skos:broader <http://resource.geosciml.org/classifier/cgi/geologicunitmorphology/planar_profile> ;
    skos:definition "Profile for which the ratio of length of longest chord to shortest chord is greater than 1.4.profile and a boundary that can be divided into distinct straight sides separated by higher curvature corners."@en ;
    skos:inScheme <http://resource.geosciml.org/classifierscheme/cgi/2016.01/geologicunitmorphology> ;
    skos:prefLabel "polygonal profile"@en .


<http://resource.geosciml.org/classifier/cgi/geologicunitmorphology/prism> a skos:Concept ;
    dcterms:source "https://en.wikipedia.org/wiki/Prism_(geometry)"^^xsd:anyURI ;
    rdfs:isDefinedBy <http://resource.geosciml.org/classifierscheme/cgi/2016.01/geologicunitmorphology> ;
    skos:broader <http://resource.geosciml.org/classifier/cgi/geologicunitmorphology/three_dimensional_body> ;
    skos:definition "A polyhedron with an n-sided polygonal base, another congruent parallel base (with the same rotational orientation), and n other faces (necessarily all parallelograms) joining corresponding sides of the two bases. All cross-sections parallel to the base faces are congruent to the bases. Prisms are named for their base, so a prism with a pentagonal base is called a pentagonal prism."@en ;
    skos:inScheme <http://resource.geosciml.org/classifierscheme/cgi/2016.01/geologicunitmorphology> ;
    skos:narrower <http://resource.geosciml.org/classifier/cgi/geologicunitmorphology/tabular_prism> ;
    skos:prefLabel "prism"@en ;
    skos:related <http://resource.geosciml.org/classifier/cgi/geologicunitmorphology/wedge> .


<http://resource.geosciml.org/classifier/cgi/geologicunitmorphology/ribbon> a skos:Concept ;
    dcterms:provenance "This vocabulary"@en ;
    rdfs:isDefinedBy <http://resource.geosciml.org/classifierscheme/cgi/2016.01/geologicunitmorphology> ;
    skos:broader <http://resource.geosciml.org/classifier/cgi/geologicunitmorphology/three_dimensional_body> ;
    skos:definition "Body that is very thin relative to width and and length. Long axis may be curved. L>(>>)W>>>H. H is typically in vertical direction."@en ;
    skos:inScheme <http://resource.geosciml.org/classifierscheme/cgi/2016.01/geologicunitmorphology> ;
    skos:prefLabel "ribbon"@en .


<http://resource.geosciml.org/classifier/cgi/geologicunitmorphology/ring_dyke> a skos:Concept ;
    dcterms:provenance "This vocabulary"@en ;
    rdfs:isDefinedBy <http://resource.geosciml.org/classifierscheme/cgi/2016.01/geologicunitmorphology> ;
    skos:altLabel "retas melingkar"@id,
        "リングダイク"@ja ;
    skos:broader <http://resource.geosciml.org/classifier/cgi/geologicunitmorphology/geologic_body> ;
    skos:definition "An arcuate or subcircular dyke, generally associated with a volcanic centre."@en ;
    skos:inScheme <http://resource.geosciml.org/classifierscheme/cgi/2016.01/geologicunitmorphology> ;
    skos:prefLabel "Ringdyke"@de,
        "ring dike"@en,
        "dique anular"@es,
        "rengasjuonet"@fi,
        "ring dyke"@fr,
        "retas cincin"@id,
        "filone ad anello"@it,
        "環状岩脈"@ja,
        "TMnb;TwkB½T§CuMvij"@km,
        "환상암맥"@ko,
        "²½Îñ¤¸ö¤Á¹¸­"@lo,
        "korok gelang"@ms,
        "dajka kol'tsevaya"@ru,
        "ringgång"@sv,
        "พนังวงแหวน"@th,
        "thể tường dạng vòng"@vi,
        "环状岩墙"@zh ;
    skos:related <http://resource.geosciml.org/classifier/cgi/geologicunitmorphology/arcuate_sheet> .


<http://resource.geosciml.org/classifier/cgi/geologicunitmorphology/rock_body_geometry_irregular> a skos:Concept ;
    dcterms:provenance "This vocabulary"@en ;
    rdfs:isDefinedBy <http://resource.geosciml.org/classifierscheme/cgi/2016.01/geologicunitmorphology> ;
    skos:broader <http://resource.geosciml.org/classifier/cgi/geologicunitmorphology/geologic_body> ;
    skos:definition "Rock body geometry is irregular and can not be characterized using terminology."@en ;
    skos:inScheme <http://resource.geosciml.org/classifierscheme/cgi/2016.01/geologicunitmorphology> ;
    skos:prefLabel "rock body geometry irregular"@en .


<http://resource.geosciml.org/classifier/cgi/geologicunitmorphology/rock_body_geometry_not_specified> a skos:Concept ;
    dcterms:provenance "This vocabulary"@en ;
    rdfs:isDefinedBy <http://resource.geosciml.org/classifierscheme/cgi/2016.01/geologicunitmorphology> ;
    skos:broader <http://resource.geosciml.org/classifier/cgi/geologicunitmorphology/geologic_body> ;
    skos:definition "Rock body geometry is not specified. Use in normative descriptions where any morphology is allowed."@en ;
    skos:inScheme <http://resource.geosciml.org/classifierscheme/cgi/2016.01/geologicunitmorphology> ;
    skos:prefLabel "rock body geometry not specified"@en .


<http://resource.geosciml.org/classifier/cgi/geologicunitmorphology/rod> a skos:Concept ;
    dcterms:provenance "This vocabulary"@en ;
    rdfs:isDefinedBy <http://resource.geosciml.org/classifierscheme/cgi/2016.01/geologicunitmorphology> ;
    skos:broader <http://resource.geosciml.org/classifier/cgi/geologicunitmorphology/cylinder> ;
    skos:definition "Cylinder with very long axis, generally circular or elliptical cross section (generating figure). H>>>W=L. Long axis may be in any orientation, and may be curved."@en ;
    skos:inScheme <http://resource.geosciml.org/classifierscheme/cgi/2016.01/geologicunitmorphology> ;
    skos:prefLabel "rod"@en .


<http://resource.geosciml.org/classifier/cgi/geologicunitmorphology/sheet> a skos:Concept ;
    dcterms:provenance "This vocabulary"@en ;
    rdfs:isDefinedBy <http://resource.geosciml.org/classifierscheme/cgi/2016.01/geologicunitmorphology> ;
    skos:broader <http://resource.geosciml.org/classifier/cgi/geologicunitmorphology/three_dimensional_body> ;
    skos:definition "Body that is very thin relative to lateral extent, so thin that is considered to consist of two bounding surfaces joined at an edge. Aspect ratio is L=W>>>H. The geometry of the edge joining the surfaces is not specified in the definition. If the geometry of the edge comes into play in the definition, becomes ribbon, disc or tablet(?). Includes dike, vein, sill and bed-shaped geologic units."@en ;
    skos:inScheme <http://resource.geosciml.org/classifierscheme/cgi/2016.01/geologicunitmorphology> ;
    skos:narrower <http://resource.geosciml.org/classifier/cgi/geologicunitmorphology/arcuate_sheet>,
        <http://resource.geosciml.org/classifier/cgi/geologicunitmorphology/conical_sheet>,
        <http://resource.geosciml.org/classifier/cgi/geologicunitmorphology/dome_sheet>,
        <http://resource.geosciml.org/classifier/cgi/geologicunitmorphology/planar_sheet>,
        <http://resource.geosciml.org/classifier/cgi/geologicunitmorphology/sigmoid_sheet> ;
    skos:prefLabel "sheet"@en ;
    skos:related <http://resource.geosciml.org/classifier/cgi/geologicunitmorphology/dike>,
        <http://resource.geosciml.org/classifier/cgi/geologicunitmorphology/layer_shape>,
        <http://resource.geosciml.org/classifier/cgi/geologicunitmorphology/sill_form>,
        <http://resource.geosciml.org/classifier/cgi/geologicunitmorphology/vein> .


<http://resource.geosciml.org/classifier/cgi/geologicunitmorphology/sheet_ellipsoid> a skos:Concept ;
    dcterms:provenance "This vocabulary"@en ;
    rdfs:isDefinedBy <http://resource.geosciml.org/classifierscheme/cgi/2016.01/geologicunitmorphology> ;
    skos:broader <http://resource.geosciml.org/classifier/cgi/geologicunitmorphology/ellipsoid> ;
    skos:definition "Ellipsoid with one axis much smaller than others H on order of .001 of L or W"@en ;
    skos:inScheme <http://resource.geosciml.org/classifierscheme/cgi/2016.01/geologicunitmorphology> ;
    skos:prefLabel "sheet ellipsoid"@en .


<http://resource.geosciml.org/classifier/cgi/geologicunitmorphology/sigmoid_sheet> a skos:Concept ;
    dcterms:provenance "This vocabulary"@en ;
    rdfs:isDefinedBy <http://resource.geosciml.org/classifierscheme/cgi/2016.01/geologicunitmorphology> ;
    skos:broader <http://resource.geosciml.org/classifier/cgi/geologicunitmorphology/sheet> ;
    skos:definition "Sheet with 's' curvature of L or W direction"@en ;
    skos:inScheme <http://resource.geosciml.org/classifierscheme/cgi/2016.01/geologicunitmorphology> ;
    skos:prefLabel "sigmoid sheet"@en .


<http://resource.geosciml.org/classifier/cgi/geologicunitmorphology/sigmoidal_vein> a skos:Concept ;
    dcterms:provenance "This vocabulary"@en ;
    rdfs:isDefinedBy <http://resource.geosciml.org/classifierscheme/cgi/2016.01/geologicunitmorphology> ;
    skos:broader <http://resource.geosciml.org/classifier/cgi/geologicunitmorphology/vein> ;
    skos:definition "Vein curved so as to resemble the letter S in section"@en ;
    skos:inScheme <http://resource.geosciml.org/classifierscheme/cgi/2016.01/geologicunitmorphology> ;
    skos:prefLabel "sigmoidal vein"@en ;
    skos:related <http://resource.geosciml.org/classifier/cgi/geologicunitmorphology/sigmoid_sheet> .


<http://resource.geosciml.org/classifier/cgi/geologicunitmorphology/sill_form> a skos:Concept ;
    dcterms:provenance "This vocabulary"@en ;
    rdfs:isDefinedBy <http://resource.geosciml.org/classifierscheme/cgi/2016.01/geologicunitmorphology> ;
    skos:broader <http://resource.geosciml.org/classifier/cgi/geologicunitmorphology/geologic_body> ;
    skos:definition "A tabular intrusive igneous body with long dimensions parallel to bedding or foliation of sedimentary or metamorphic host rock."@en ;
    skos:inScheme <http://resource.geosciml.org/classifierscheme/cgi/2016.01/geologicunitmorphology> ;
    skos:prefLabel "sill form"@en ;
    skos:related <http://resource.geosciml.org/classifier/cgi/geologicunitmorphology/layer_shape>,
        <http://resource.geosciml.org/classifier/cgi/geologicunitmorphology/sheet>,
        <http://resource.geosciml.org/classifier/cgi/geologicunitmorphology/sheet_ellipsoid> .


<http://resource.geosciml.org/classifier/cgi/geologicunitmorphology/sphenolith> a skos:Concept ;
    dcterms:provenance "This vocabulary"@en ;
    rdfs:isDefinedBy <http://resource.geosciml.org/classifierscheme/cgi/2016.01/geologicunitmorphology> ;
    skos:broader <http://resource.geosciml.org/classifier/cgi/geologicunitmorphology/geologic_body> ;
    skos:definition "Wedge-like intrusion, partly concordant, partly discordant."@en ;
    skos:inScheme <http://resource.geosciml.org/classifierscheme/cgi/2016.01/geologicunitmorphology> ;
    skos:prefLabel "Sphenolithus"@de,
        "sphenolith"@en,
        "esfenolito"@es,
        "sfenoliitti"@fi,
        "sfenolite"@it,
        "sfenolit"@ru,
        "sfenolit"@sv ;
    skos:related <http://resource.geosciml.org/classifier/cgi/geologicunitmorphology/prism>,
        <http://resource.geosciml.org/classifier/cgi/geologicunitmorphology/wedge> .


<http://resource.geosciml.org/classifier/cgi/geologicunitmorphology/spheroid> a skos:Concept ;
    dcterms:provenance "This vocabulary"@en ;
    rdfs:isDefinedBy <http://resource.geosciml.org/classifierscheme/cgi/2016.01/geologicunitmorphology> ;
    skos:broader <http://resource.geosciml.org/classifier/cgi/geologicunitmorphology/ellipsoid> ;
    skos:definition "Ellipsoid with L, W, and H dimensions all approximately equal"@en ;
    skos:inScheme <http://resource.geosciml.org/classifierscheme/cgi/2016.01/geologicunitmorphology> ;
    skos:prefLabel "spheroid"@en .


<http://resource.geosciml.org/classifier/cgi/geologicunitmorphology/square_profile> a skos:Concept ;
    dcterms:provenance "This vocabulary"@en ;
    rdfs:isDefinedBy <http://resource.geosciml.org/classifierscheme/cgi/2016.01/geologicunitmorphology> ;
    skos:broader <http://resource.geosciml.org/classifier/cgi/geologicunitmorphology/polygonal_profile> ;
    skos:definition "polygonal profile that approximates a square"@en ;
    skos:inScheme <http://resource.geosciml.org/classifierscheme/cgi/2016.01/geologicunitmorphology> ;
    skos:prefLabel "square profile"@en .


<http://resource.geosciml.org/classifier/cgi/geologicunitmorphology/tablet> a skos:Concept ;
    dcterms:provenance "This vocabulary"@en ;
    rdfs:isDefinedBy <http://resource.geosciml.org/classifierscheme/cgi/2016.01/geologicunitmorphology> ;
    skos:broader <http://resource.geosciml.org/classifier/cgi/geologicunitmorphology/polygonal_cylinder> ;
    skos:definition "Polygonal cylinder with height less than length or width, disc with edges separating side into multiple segments."@en ;
    skos:inScheme <http://resource.geosciml.org/classifierscheme/cgi/2016.01/geologicunitmorphology> ;
    skos:prefLabel "tablet"@en .


<http://resource.geosciml.org/classifier/cgi/geologicunitmorphology/tabular_prism> a skos:Concept ;
    dcterms:provenance "This vocabulary"@en ;
    rdfs:isDefinedBy <http://resource.geosciml.org/classifierscheme/cgi/2016.01/geologicunitmorphology> ;
    skos:broader <http://resource.geosciml.org/classifier/cgi/geologicunitmorphology/prism> ;
    skos:definition "Body defined by pairs of parallel, approximately planar surfaces separated by definable edges. Grades to ellipsoid as edges lose definition, to block as axial ratios approach 1, to polygonal cylinder as L approaches W. L>>W>H. H is in vertical direction, L is horizontal."@en ;
    skos:inScheme <http://resource.geosciml.org/classifierscheme/cgi/2016.01/geologicunitmorphology> ;
    skos:prefLabel "tabular prism"@en .


<http://resource.geosciml.org/classifier/cgi/geologicunitmorphology/tear_drop> a skos:Concept ;
    dcterms:provenance "This vocabulary"@en ;
    rdfs:isDefinedBy <http://resource.geosciml.org/classifierscheme/cgi/2016.01/geologicunitmorphology> ;
    skos:broader <http://resource.geosciml.org/classifier/cgi/geologicunitmorphology/three_dimensional_body> ;
    skos:definition "Body bounded by hemispheroid on one side, cone on other, with circular symmetry around cone axis"@en ;
    skos:inScheme <http://resource.geosciml.org/classifierscheme/cgi/2016.01/geologicunitmorphology> ;
    skos:prefLabel "tear drop"@en .


<http://resource.geosciml.org/classifier/cgi/geologicunitmorphology/trough> a skos:Concept ;
    dcterms:provenance "This vocabulary"@en ;
    rdfs:isDefinedBy <http://resource.geosciml.org/classifierscheme/cgi/2016.01/geologicunitmorphology> ;
    skos:broader <http://resource.geosciml.org/classifier/cgi/geologicunitmorphology/geologic_body> ;
    skos:definition "Shape of a body of sedimentary rock deposited in an elongate depression filled with sediment. large size distinguishes from channel"@en ;
    skos:inScheme <http://resource.geosciml.org/classifierscheme/cgi/2016.01/geologicunitmorphology> ;
    skos:prefLabel "Tiefseemulde"@de,
        "trough shape"@en,
        "fosa abisal alargada"@es,
        "poimupohjat"@fi,
        "fossa abissale allungata"@it,
        "trog"@ru,
        "tråg"@sv ;
    skos:related <http://resource.geosciml.org/classifier/cgi/geologicunitmorphology/longitudinal_section_of_cylinder> .


<http://resource.geosciml.org/classifier/cgi/geologicunitmorphology/vein> a skos:Concept ;
    dcterms:provenance "This vocabulary"@en ;
    rdfs:isDefinedBy <http://resource.geosciml.org/classifierscheme/cgi/2016.01/geologicunitmorphology> ;
    skos:broader <http://resource.geosciml.org/classifier/cgi/geologicunitmorphology/geologic_body> ;
    skos:definition "A tabular or sheetlike epigenetic mineral filling of a fault or fracture"@en ;
    skos:inScheme <http://resource.geosciml.org/classifierscheme/cgi/2016.01/geologicunitmorphology> ;
    skos:narrower <http://resource.geosciml.org/classifier/cgi/geologicunitmorphology/planar_vein>,
        <http://resource.geosciml.org/classifier/cgi/geologicunitmorphology/sigmoidal_vein> ;
    skos:prefLabel "vein-shape"@en ;
    skos:related <http://resource.geosciml.org/classifier/cgi/geologicunitmorphology/sheet> .


<http://resource.geosciml.org/classifier/cgi/geologicunitmorphology/wedge> a skos:Concept ;
    dcterms:source "https://en.wikipedia.org/wiki/Wedge_(geometry)"^^xsd:anyURI ;
    rdfs:isDefinedBy <http://resource.geosciml.org/classifierscheme/cgi/2016.01/geologicunitmorphology> ;
    skos:broader <http://resource.geosciml.org/classifier/cgi/geologicunitmorphology/three_dimensional_body> ;
    skos:definition "A wedge is a polyhedron defined by two triangles and three trapezoid faces. A wedge has five faces, nine edges, and six vertices. A wedge is a subclass of the prismatoids with the base and opposite ridge in two parallel planes."@en ;
    skos:inScheme <http://resource.geosciml.org/classifierscheme/cgi/2016.01/geologicunitmorphology> ;
    skos:prefLabel "wedge"@en ;
    skos:related <http://resource.geosciml.org/classifier/cgi/geologicunitmorphology/prism> .

