PREFIX : <http://resource.geosciml.org/classifierscheme/cgi/2016.01/stratigraphicrank>
PREFIX cs: <http://resource.geosciml.org/classifierscheme/cgi/2016.01/stratigraphicrank>
PREFIX dt: <http://resource.geosciml.org/datatype/>
PREFIX rdf: <http://www.w3.org/1999/02/22-rdf-syntax-ns#>
PREFIX rdfs: <http://www.w3.org/2000/01/rdf-schema#>
PREFIX schema: <https://schema.org/>
PREFIX skos: <http://www.w3.org/2004/02/skos/core#>
PREFIX xsd: <http://www.w3.org/2001/XMLSchema#>

<http://resource.geosciml.org/classifierscheme/cgi/2016.01/stratigraphicrank> a skos:ConceptScheme ;
    schema:keywords "GeoSciML" ;
    schema:dateCreated "2009-07-14"^^xsd:date ;
    schema:creator <https://linked.data.gov.au/org/cgi-gtwg> ;
    schema:dateModified "2025-06-04"^^xsd:date ;
    schema:citation "Original set of terms from the GeosciML standard" ;
    schema:publisher <https://linked.data.gov.au/org/cgi> ;
    schema:citation "http://www.opengis.net/doc/geosciml/4.1"^^xsd:anyURI ;
    skos:changeNote "2009-07-14 Generate SKOS encoding of vocabulary from Excel spreadsheet."@en,
        "2009-12-07 SMR Update metadata properties for version, creator, title, and format. Change skos:HistoryNote to dc:source for information on origin of terms and definitions."@en,
        "2010-02-08 SMR Clean up namespace declarations so concept URI's follow CGI URN scheme; concepts have URN, are not document fragments."@en,
        "2010-11-28 SMR replace URN with http URI constructed according to CGI URI scheme (see https://www.seegrid.csiro.au/wiki/bin/view/CGIModel/PersistentIdentifiersInGeoSciMLServices)"@en,
        "2011-02-16 SMR Add broader/narrower relations according to stratigraphic code. These are not meant to be formal isA or PartOf relations, rather should be read something like 'broader in local intention' or 'may be part of'. Add term 'complex' to vocabulary"@en,
        "2012-02-07 SMR update URI to replace numeric final token with English-language string as in original URN scheme."@en,
        "2012-02-27 SMR add skos:exactMatch triples to map URIs for concepts in this vocabulary to number-token URIs in 201012 version of same concepts."@en,
        "2012-11-24 SMR Update to 201211 version; add collection entity, check all pref labels are lower case, remove owl:NamedIndividual and Owl:Thing rdf:types."@en,
        "2016-07-15 OLR - reformat SKOS-RDF for new repository"@en,
        "2020-06-23 NJC Added properties to ensure vocab matched Geoscience Australia's vocab profile (http://linked.data.gov.au/def/ga-skos-profile). Just annotation properties, no new content. Agents (creator/publisher) now not text but RDF resource. Dates (create/modified) derived from editorial notes & existing date properties."@en ,
        "2025-06-04 NJC Updates metadata to meet the VocPub 5.1 profile"@en ;
    skos:definition "This scheme specifies concepts used to categorize the stratigraphic rank of geologic units, as compiled by the IUGS Commission for Geoscience Information (CGI) Geoscience Terminology Working Group. By extension, it includes all concepts in this conceptScheme, as well as concepts in any previous versions of the scheme."@en ;
    skos:editorialNote "This file contains the 2016.01 SKOS-RDF version of the CGI Stratigraphic Rank vocabulary. Compilation and review in MS Excel spreadsheet, converted to MS Excel for SKOS generation using GSML_SKOS_fromXLS_2016.02.xslt."@en ;
    skos:hasTopConcept <http://resource.geosciml.org/classifier/cgi/stratigraphicrank/complex>,
        <http://resource.geosciml.org/classifier/cgi/stratigraphicrank/megasequence>,
        <http://resource.geosciml.org/classifier/cgi/stratigraphicrank/rank_not_specified>,
        <http://resource.geosciml.org/classifier/cgi/stratigraphicrank/supergroup>,
        <http://resource.geosciml.org/classifier/cgi/stratigraphicrank/supersuite> ;
    skos:prefLabel "Stratigraphic Rank"@en .


<http://resource.geosciml.org/classifier/cgi/stratigraphicrank> a skos:Collection ;
    schema:citation "this vocabulary" ;
    skos:definition "All Concepts in this vocabulary" ;
    skos:member <http://resource.geosciml.org/classifier/cgi/stratigraphicrank/bed>,
        <http://resource.geosciml.org/classifier/cgi/stratigraphicrank/complex>,
        <http://resource.geosciml.org/classifier/cgi/stratigraphicrank/formation>,
        <http://resource.geosciml.org/classifier/cgi/stratigraphicrank/group>,
        <http://resource.geosciml.org/classifier/cgi/stratigraphicrank/lithodeme>,
        <http://resource.geosciml.org/classifier/cgi/stratigraphicrank/megasequence>,
        <http://resource.geosciml.org/classifier/cgi/stratigraphicrank/member>,
        <http://resource.geosciml.org/classifier/cgi/stratigraphicrank/rank_not_specified>,
        <http://resource.geosciml.org/classifier/cgi/stratigraphicrank/sequence>,
        <http://resource.geosciml.org/classifier/cgi/stratigraphicrank/subgroup>,
        <http://resource.geosciml.org/classifier/cgi/stratigraphicrank/suite>,
        <http://resource.geosciml.org/classifier/cgi/stratigraphicrank/supergroup>,
        <http://resource.geosciml.org/classifier/cgi/stratigraphicrank/supersequence>,
        <http://resource.geosciml.org/classifier/cgi/stratigraphicrank/supersuite> ;
    skos:prefLabel "Stratigraphic Rank - All Concepts"@en .


<http://resource.geosciml.org/classifier/cgi/stratigraphicrank/complex> a skos:Concept ;
    schema:citation "Salvador; A.; ed. 1994. International Stratigraphic Guide: International Union of Geological Sciences; Trondheim; NO; 214 p."@en ;
    rdfs:isDefinedBy <http://resource.geosciml.org/classifierscheme/cgi/2016.01/stratigraphicrank> ;
    skos:definition "A lithostratigraphic unit composed of diverse types of any class or classes of rock (sedimentary; igneous; metamorphic); and characterized by irregularly mixed lithology or by hightly complicated structure relations to the extent that the original sequence of the component rocks may be obscured and the individual rocks or rock sequence cannot be readily mapped."@en ;
    skos:inScheme <http://resource.geosciml.org/classifierscheme/cgi/2016.01/stratigraphicrank> ;
    skos:prefLabel "complex"@en ;
    skos:related <http://resource.geosciml.org/classifier/cgi/stratigraphicrank/lithodeme> ;
    skos:topConceptOf <http://resource.geosciml.org/classifierscheme/cgi/2016.01/stratigraphicrank> .


<http://resource.geosciml.org/classifier/cgi/stratigraphicrank/megasequence> a skos:Concept ;
    schema:citation "Haq; B.U.hardenbol; J.; and Vail; P.R.; 1988; Mesozoic and Cenozoic chronostratigraphy an dcycles of sea-level changes; in Wilgus; C.K.; et al.; eds; Sea-level Changes: an Integrated Approach: Society of Sedimentary Geology Special Publication 42; p. 71-108."@en ;
    rdfs:isDefinedBy <http://resource.geosciml.org/classifierscheme/cgi/2016.01/stratigraphicrank> ;
    skos:definition "A succession of strata comprising two or more supersequences. A large-scale sequence-stratigraphic unit deposited during one distinct phase of basin evolution; separated by major unconformities that mark a change in fundamental basin-controlling processes."@en ;
    skos:inScheme <http://resource.geosciml.org/classifierscheme/cgi/2016.01/stratigraphicrank> ;
    skos:narrower <http://resource.geosciml.org/classifier/cgi/stratigraphicrank/supersequence> ;
    skos:prefLabel "megasequence"@en ;
    skos:related <http://resource.geosciml.org/classifier/cgi/stratigraphicrank/supersuite> ;
    skos:topConceptOf <http://resource.geosciml.org/classifierscheme/cgi/2016.01/stratigraphicrank> .


<http://resource.geosciml.org/classifier/cgi/stratigraphicrank/rank_not_specified> a skos:Concept ;
    schema:citation "this vocabulary"@en ;
    rdfs:isDefinedBy <http://resource.geosciml.org/classifierscheme/cgi/2016.01/stratigraphicrank> ;
    skos:definition "unit is not part of a defined stratigraphic hierarchy."@en ;
    skos:inScheme <http://resource.geosciml.org/classifierscheme/cgi/2016.01/stratigraphicrank> ;
    skos:prefLabel "not specified"@en ;
    skos:topConceptOf <http://resource.geosciml.org/classifierscheme/cgi/2016.01/stratigraphicrank> .


<http://resource.geosciml.org/classifier/cgi/stratigraphicrank/supergroup> a skos:Concept ;
    schema:citation "North American Commission on Stratigraphic Nomenclature; 2005; Salvador; 1994"@en ;
    rdfs:isDefinedBy <http://resource.geosciml.org/classifierscheme/cgi/2016.01/stratigraphicrank> ;
    skos:definition "A supergroup is a formal assemblage of related or superposed groups or of groups and formations"@en ;
    skos:inScheme <http://resource.geosciml.org/classifierscheme/cgi/2016.01/stratigraphicrank> ;
    skos:narrower <http://resource.geosciml.org/classifier/cgi/stratigraphicrank/group> ;
    skos:prefLabel "supergroup"@en ;
    skos:related <http://resource.geosciml.org/classifier/cgi/stratigraphicrank/supersuite> ;
    skos:topConceptOf <http://resource.geosciml.org/classifierscheme/cgi/2016.01/stratigraphicrank> .


<http://resource.geosciml.org/classifier/cgi/stratigraphicrank/supersuite> a skos:Concept ;
    schema:citation "North American Commission on Stratigraphic Nomenclature; 2005"@en ;
    rdfs:isDefinedBy <http://resource.geosciml.org/classifierscheme/cgi/2016.01/stratigraphicrank> ;
    skos:definition "A formal lithodemic unit next higher in rank to suite. It comprises two or more suites having a degree of natural relationship to one another"@en ;
    skos:inScheme <http://resource.geosciml.org/classifierscheme/cgi/2016.01/stratigraphicrank> ;
    skos:narrower <http://resource.geosciml.org/classifier/cgi/stratigraphicrank/suite> ;
    skos:prefLabel "supersuite"@en ;
    skos:related <http://resource.geosciml.org/classifier/cgi/stratigraphicrank/megasequence>,
        <http://resource.geosciml.org/classifier/cgi/stratigraphicrank/supergroup> ;
    skos:topConceptOf <http://resource.geosciml.org/classifierscheme/cgi/2016.01/stratigraphicrank> .


<http://resource.geosciml.org/classifier/cgi/stratigraphicrank/bed> a skos:Concept ;
    schema:citation "North American Commission on Stratigraphic Nomenclature; 2005; Salvador; 1994"@en ;
    rdfs:isDefinedBy <http://resource.geosciml.org/classifierscheme/cgi/2016.01/stratigraphicrank> ;
    skos:broader <http://resource.geosciml.org/classifier/cgi/stratigraphicrank/member> ;
    skos:definition "The smallest formal lithostratigraphic unit; usually a distinctive lithic entity which can be distinguished from adjacent rocks by one or more physical characteristics."@en ;
    skos:inScheme <http://resource.geosciml.org/classifierscheme/cgi/2016.01/stratigraphicrank> ;
    skos:prefLabel "bed"@en .


<http://resource.geosciml.org/classifier/cgi/stratigraphicrank/formation> a skos:Concept ;
    schema:citation "North American Commission on Stratigraphic Nomenclature; 2005; Salvador; 1994"@en ;
    rdfs:isDefinedBy <http://resource.geosciml.org/classifierscheme/cgi/2016.01/stratigraphicrank> ;
    skos:broader <http://resource.geosciml.org/classifier/cgi/stratigraphicrank/subgroup> ;
    skos:definition "A body of rock identified by lithic characteristics and stratigraphic position; it is usually but not necessarily tabular and is mappable at the Earth's surface or traceable in the subsurface."@en ;
    skos:inScheme <http://resource.geosciml.org/classifierscheme/cgi/2016.01/stratigraphicrank> ;
    skos:narrower <http://resource.geosciml.org/classifier/cgi/stratigraphicrank/member> ;
    skos:prefLabel "formation"@en ;
    skos:related <http://resource.geosciml.org/classifier/cgi/stratigraphicrank/lithodeme> .


<http://resource.geosciml.org/classifier/cgi/stratigraphicrank/group> a skos:Concept ;
    schema:citation "North American Commission on Stratigraphic Nomenclature; 2005; Salvador; 1994"@en ;
    rdfs:isDefinedBy <http://resource.geosciml.org/classifierscheme/cgi/2016.01/stratigraphicrank> ;
    skos:broader <http://resource.geosciml.org/classifier/cgi/stratigraphicrank/supergroup> ;
    skos:definition "A group is the lithostratigraphic unit next higher in rank to either subgroup or formation. A groups may consist of two or more subgroups or two or more formations or a combination of both."@en ;
    skos:inScheme <http://resource.geosciml.org/classifierscheme/cgi/2016.01/stratigraphicrank> ;
    skos:narrower <http://resource.geosciml.org/classifier/cgi/stratigraphicrank/subgroup> ;
    skos:prefLabel "group"@en ;
    skos:related <http://resource.geosciml.org/classifier/cgi/stratigraphicrank/suite> .


<http://resource.geosciml.org/classifier/cgi/stratigraphicrank/lithodeme> a skos:Concept ;
    schema:citation "North American Commission on Stratigraphic Nomenclature; 2005"@en ;
    rdfs:isDefinedBy <http://resource.geosciml.org/classifierscheme/cgi/2016.01/stratigraphicrank> ;
    skos:broader <http://resource.geosciml.org/classifier/cgi/stratigraphicrank/suite> ;
    skos:definition "A body of predominantly intrusivehighly deformed and/or highly metamorphosed rock; distinguished and delimited on the basis of rock characteristics."@en ;
    skos:inScheme <http://resource.geosciml.org/classifierscheme/cgi/2016.01/stratigraphicrank> ;
    skos:prefLabel "lithodeme"@en ;
    skos:related <http://resource.geosciml.org/classifier/cgi/stratigraphicrank/complex>,
        <http://resource.geosciml.org/classifier/cgi/stratigraphicrank/formation>,
        <http://resource.geosciml.org/classifier/cgi/stratigraphicrank/sequence> .


<http://resource.geosciml.org/classifier/cgi/stratigraphicrank/member> a skos:Concept ;
    schema:citation "North American Commission on Stratigraphic Nomenclature; 2005; Salvador; 1994"@en ;
    rdfs:isDefinedBy <http://resource.geosciml.org/classifierscheme/cgi/2016.01/stratigraphicrank> ;
    skos:broader <http://resource.geosciml.org/classifier/cgi/stratigraphicrank/formation> ;
    skos:definition "A formal lithostratigraphic unit next in rank below a formation; and always part of a formation. It is a named entity within a formation because it possesses characteristics distinguishing it from adjacent parts of the formation."@en ;
    skos:inScheme <http://resource.geosciml.org/classifierscheme/cgi/2016.01/stratigraphicrank> ;
    skos:narrower <http://resource.geosciml.org/classifier/cgi/stratigraphicrank/bed> ;
    skos:prefLabel "member"@en .


<http://resource.geosciml.org/classifier/cgi/stratigraphicrank/sequence> a skos:Concept ;
    schema:citation "Van Wagoner; J.C.; Posamentierh.W.; Mitchum; R.M.; Vail; P.R.; Sarg; J.F.; Loutit; T.S.hardenbol; J.; 1988; An overview of sequence stratigraphy and key definitions. In: Wilgus; C.K.hastings; B.S.; Kendall; C.G.St.C.; Posamentierh.W.; Ross; C.A.; Van Wagoner; J.C. (Eds.); Sea Level Changes––An Integrated Approach; vol. 42. SEPM Special Publication; pp. 39–45."@en ;
    rdfs:isDefinedBy <http://resource.geosciml.org/classifierscheme/cgi/2016.01/stratigraphicrank> ;
    skos:broader <http://resource.geosciml.org/classifier/cgi/stratigraphicrank/supersequence> ;
    skos:definition "A genetically related succession of strata bounded by unconformites or their correlative conformable contacts; and typically having a thickness of 10-100 metres."@en ;
    skos:inScheme <http://resource.geosciml.org/classifierscheme/cgi/2016.01/stratigraphicrank> ;
    skos:prefLabel "sequence"@en ;
    skos:related <http://resource.geosciml.org/classifier/cgi/stratigraphicrank/lithodeme> .


<http://resource.geosciml.org/classifier/cgi/stratigraphicrank/subgroup> a skos:Concept ;
    schema:citation "Salvador; 1994"@en ;
    rdfs:isDefinedBy <http://resource.geosciml.org/classifierscheme/cgi/2016.01/stratigraphicrank> ;
    skos:broader <http://resource.geosciml.org/classifier/cgi/stratigraphicrank/group> ;
    skos:definition "A subgroup is the lithostratigraphic unit next higher in rank to formation. A subgroup usually consists of several formations."@en ;
    skos:inScheme <http://resource.geosciml.org/classifierscheme/cgi/2016.01/stratigraphicrank> ;
    skos:narrower <http://resource.geosciml.org/classifier/cgi/stratigraphicrank/formation> ;
    skos:prefLabel "subgroup"@en .


<http://resource.geosciml.org/classifier/cgi/stratigraphicrank/suite> a skos:Concept ;
    schema:citation "North American Commission on Stratigraphic Nomenclature; 2005"@en ;
    rdfs:isDefinedBy <http://resource.geosciml.org/classifierscheme/cgi/2016.01/stratigraphicrank> ;
    skos:broader <http://resource.geosciml.org/classifier/cgi/stratigraphicrank/supersuite> ;
    skos:definition "A formal lithodemic unit next higher in rank to lithodeme. It comprises two or more associated lithodemes of the same class (e.g.; plutonic; metamorphic)."@en ;
    skos:inScheme <http://resource.geosciml.org/classifierscheme/cgi/2016.01/stratigraphicrank> ;
    skos:narrower <http://resource.geosciml.org/classifier/cgi/stratigraphicrank/lithodeme> ;
    skos:prefLabel "suite"@en ;
    skos:related <http://resource.geosciml.org/classifier/cgi/stratigraphicrank/group>,
        <http://resource.geosciml.org/classifier/cgi/stratigraphicrank/supersequence> .


<http://resource.geosciml.org/classifier/cgi/stratigraphicrank/supersequence> a skos:Concept ;
    schema:citation "Haq; B.U.hardenbol; J.; and Vail; P.R.; 1988; Mesozoic and Cenozoic chronostratigraphy an dcycles of sea-level changes; in Wilgus; C.K.; et al.; eds; Sea-level Changes: an Integrated Approach: Society of Sedimentary Geology Special Publication 42; p. 71-108."@en ;
    rdfs:isDefinedBy <http://resource.geosciml.org/classifierscheme/cgi/2016.01/stratigraphicrank> ;
    skos:broader <http://resource.geosciml.org/classifier/cgi/stratigraphicrank/megasequence> ;
    skos:definition "A succession of strata comprising two or more sequences"@en ;
    skos:inScheme <http://resource.geosciml.org/classifierscheme/cgi/2016.01/stratigraphicrank> ;
    skos:narrower <http://resource.geosciml.org/classifier/cgi/stratigraphicrank/sequence> ;
    skos:prefLabel "supersequence"@en ;
    skos:related <http://resource.geosciml.org/classifier/cgi/stratigraphicrank/suite> .

